@prefix : <http://purl.org/td/transportdisruption#> .
@prefix dc: <http://purl.org/dc/elements/1.1/> .
@prefix owl: <http://www.w3.org/2002/07/owl#> .
@prefix rdf: <http://www.w3.org/1999/02/22-rdf-syntax-ns#> .
@prefix xml: <http://www.w3.org/XML/1998/namespace> .
@prefix xsd: <http://www.w3.org/2001/XMLSchema#> .
@prefix rdfs: <http://www.w3.org/2000/01/rdf-schema#> .
@prefix skos: <http://www.w3.org/2004/02/skos/core#> .
@prefix terms: <http://purl.org/dc/terms/> .
@base <http://purl.org/td/transportdisruption> .

<http://purl.org/td/transportdisruption> rdf:type owl:Ontology ;
                                         
                                         rdfs:label "The Transport Disruption ontology"^^xsd:string ;
                                         
                                         dc:date "2015-07-16"^^xsd:date ;
                                         
                                         dc:creator "David Corsar"^^xsd:string ;
                                         
                                         dc:rights "Licensed under the Lesser General Public Licence (LGPL) Version 2.1 (http://www.gnu.org/licenses/lgpl-2.1.html)"^^xsd:string ;
                                         
                                         dc:creator "Milan Markovic"^^xsd:string ;
                                         
                                         owl:versionInfo "Revision: 1.0.1"^^xsd:string ;
                                         
                                         dc:title "The Transport Disruption ontology"^^xsd:string ;
                                         
                                         dc:description """The Transport Disruption ontology is a formal framework for modelling events related to travel and transport that may disrupt the travel plans of an agent.  Such events typically disrupt the supply or cost of transport, can affect single or multiple transport links in an area, and cause greater disruption to an agent’s travel plans than they would typically experience due to everyday travel variability.  

The ontology is based around the DisruptiveImpact class, which captures the action of one or more events causing or tending to prevent an agent’s planned travel continuing as expected.  An Event becomes a DisruptiveEvent which is the causeOf at least one DisruptiveImpact.  It is the intention that the DisruptiveImpact class is extended to define the type(s) of impact relevant to each usage, such as a delayed journey or cancelled ferry crossing.  The Plan class is another extension point for providing details of an agent's plan that an event may have impacted upon, such as an agent’s journey itinerary. 

The ontology defines several subclass of Event, describing events that may disrupt an agent's travel plans. These are based on the analysis of published disruption information and the road disruptions described in the DATEX II (http://www.datex2.eu/) specification.   Each Event is defined in terms of its time of occurrence and place (location).   The sub_event property allows compound relationships between events to be modelled; for example, that a RoadClosure occurs as part of a Roadworks event. The factor property can be used to define further relationships between events, such as a SeriousAccident contributing to PublicTransportDelay."""^^xsd:string ;
                                         
                                         rdfs:comment """The Transport Disruption ontology provides a formal framework for modelling travel and transport related events that have a disruptive impact on an agent's planned travel.

This document describes the Transport Disruption ontology, automatically generated by the LODE service (http://www.essepuntato.it/lode)"""^^xsd:string ;
                                         
                                         owl:imports <http://purl.org/NET/c4dm/event.owl> ,
                                                     <http://xmlns.com/foaf/0.1/> ;
                                         
                                         dc:description <https://raw.githubusercontent.com/transportdisruption/transportdisruption.github.io/master/TransportDisruptionOntologyOutline.png> .


#################################################################
#
#    Annotation properties
#
#################################################################


###  http://purl.org/dc/elements/1.1/creator

dc:creator rdfs:label "Creator"@en ;
           
           terms:issued "1999-07-02"^^xsd:date ;
           
           terms:modified "2008-01-14"^^xsd:date ;
           
           skos:note "A second property with the same name as this property has been declared in the dcterms: namespace (http://purl.org/dc/terms/).  See the Introduction to the document \"DCMI Metadata Terms\" (http://dublincore.org/documents/dcmi-terms/) for an explanation."@en ;
           
           rdfs:comment "An entity primarily responsible for making the resource."@en ,
                        "Examples of a Creator include a person, an organization, or a service. Typically, the name of a Creator should be used to indicate the entity."@en ;
           
           terms:hasVersion <http://dublincore.org/usage/terms/history/#creator-006> ;
           
           rdfs:isDefinedBy dc: .



###  http://purl.org/dc/elements/1.1/date

dc:date rdfs:label "Date"@en ;
        
        terms:issued "1999-07-02"^^xsd:date ;
        
        terms:modified "2008-01-14"^^xsd:date ;
        
        rdfs:comment "A point or period of time associated with an event in the lifecycle of the resource."@en ;
        
        skos:note "A second property with the same name as this property has been declared in the dcterms: namespace (http://purl.org/dc/terms/).  See the Introduction to the document \"DCMI Metadata Terms\" (http://dublincore.org/documents/dcmi-terms/) for an explanation."@en ;
        
        rdfs:comment "Date may be used to express temporal information at any level of granularity.  Recommended best practice is to use an encoding scheme, such as the W3CDTF profile of ISO 8601 [W3CDTF]."@en ;
        
        terms:hasVersion <http://dublincore.org/usage/terms/history/#date-006> ;
        
        rdfs:isDefinedBy dc: .



###  http://purl.org/dc/elements/1.1/description

dc:description rdfs:label "Description"@en ;
               
               terms:issued "1999-07-02"^^xsd:date ;
               
               terms:modified "2008-01-14"^^xsd:date ;
               
               skos:note "A second property with the same name as this property has been declared in the dcterms: namespace (http://purl.org/dc/terms/).  See the Introduction to the document \"DCMI Metadata Terms\" (http://dublincore.org/documents/dcmi-terms/) for an explanation."@en ;
               
               rdfs:comment "An account of the resource."@en ,
                            "Description may include but is not limited to: an abstract, a table of contents, a graphical representation, or a free-text account of the resource."@en ;
               
               terms:hasVersion <http://dublincore.org/usage/terms/history/#description-006> ;
               
               rdfs:isDefinedBy dc: .



###  http://purl.org/dc/elements/1.1/rights

dc:rights rdfs:label "Rights"@en ;
          
          terms:issued "1999-07-02"^^xsd:date ;
          
          terms:modified "2008-01-14"^^xsd:date ;
          
          skos:note "A second property with the same name as this property has been declared in the dcterms: namespace (http://purl.org/dc/terms/).  See the Introduction to the document \"DCMI Metadata Terms\" (http://dublincore.org/documents/dcmi-terms/) for an explanation."@en ;
          
          rdfs:comment "Information about rights held in and over the resource."@en ,
                       "Typically, rights information includes a statement about various property rights associated with the resource, including intellectual property rights."@en ;
          
          terms:hasVersion <http://dublincore.org/usage/terms/history/#rights-006> ;
          
          rdfs:isDefinedBy dc: .



###  http://purl.org/dc/elements/1.1/title

dc:title rdfs:label "Title"@en ;
         
         terms:issued "1999-07-02"^^xsd:date ;
         
         terms:modified "2008-01-14"^^xsd:date ;
         
         rdfs:comment "A name given to the resource."@en ;
         
         skos:note "A second property with the same name as this property has been declared in the dcterms: namespace (http://purl.org/dc/terms/).  See the Introduction to the document \"DCMI Metadata Terms\" (http://dublincore.org/documents/dcmi-terms/) for an explanation."@en ;
         
         terms:hasVersion <http://dublincore.org/usage/terms/history/#title-006> ;
         
         rdfs:isDefinedBy dc: .



###  http://purl.org/dc/terms/description

terms:description rdf:type owl:AnnotationProperty .



###  http://purl.org/dc/terms/hasVersion

terms:hasVersion rdf:type owl:AnnotationProperty .



###  http://purl.org/dc/terms/issued

terms:issued rdf:type owl:AnnotationProperty .



###  http://purl.org/dc/terms/modified

terms:modified rdf:type owl:AnnotationProperty .



###  http://purl.org/dc/terms/publisher

terms:publisher rdf:type owl:AnnotationProperty .



###  http://purl.org/dc/terms/title

terms:title rdf:type owl:AnnotationProperty .



###  http://www.w3.org/2004/02/skos/core#note

skos:note rdf:type owl:AnnotationProperty .





#################################################################
#
#    Datatypes
#
#################################################################


###  http://www.w3.org/2001/XMLSchema#date

xsd:date rdf:type rdfs:Datatype .





#################################################################
#
#    Object Properties
#
#################################################################


###  http://purl.org/td/transportdisruption#causeOf

:causeOf rdf:type owl:ObjectProperty ;
         
         rdfs:label "cause of"^^xsd:string ;
         
         rdfs:comment "Indicates that a Disruptive Event is a cause of a Disruptive Impact."^^xsd:string ;
         
         rdfs:domain <http://purl.org/NET/c4dm/event.owl#Event> ;
         
         rdfs:range :DisruptiveImpact ;
         
         owl:inverseOf :hasCause .



###  http://purl.org/td/transportdisruption#hasCause

:hasCause rdf:type owl:ObjectProperty ;
          
          rdfs:label "has cause"^^xsd:string ;
          
          rdfs:comment "Indicates that a Disruptive Impact is caused by an Event."^^xsd:string ;
          
          rdfs:range <http://purl.org/NET/c4dm/event.owl#Event> ;
          
          rdfs:domain :DisruptiveImpact .



###  http://purl.org/td/transportdisruption#hasPlan

:hasPlan rdf:type owl:ObjectProperty ;
         
         rdfs:label "has plan"^^xsd:string ;
         
         rdfs:comment "Indicates a Plan that a foaf:Agent has."^^xsd:string ;
         
         rdfs:range :Plan ;
         
         rdfs:domain <http://xmlns.com/foaf/0.1/Agent> .



###  http://purl.org/td/transportdisruption#impactsOn

:impactsOn rdf:type owl:ObjectProperty ;
           
           rdfs:label "impacts on"^^xsd:string ;
           
           rdfs:comment "Indicates a Plan that a Disruptive Impact affects."^^xsd:string ;
           
           rdfs:domain :DisruptiveImpact ;
           
           rdfs:range :Plan .



###  http://purl.org/td/transportdisruption#relevantTo

:relevantTo rdf:type owl:ObjectProperty ;
            
            rdfs:label "Indicates a foaf:Agent that a Disruptive Impact is relevant to."^^xsd:string ,
                       "relevant to"^^xsd:string ;
            
            rdfs:domain :DisruptiveImpact ;
            
            rdfs:range <http://xmlns.com/foaf/0.1/Agent> .





#################################################################
#
#    Classes
#
#################################################################


###  http://purl.org/NET/c4dm/event.owl#Event

<http://purl.org/NET/c4dm/event.owl#Event> rdf:type owl:Class .



###  http://purl.org/td/transportdisruption#AbandonedVehicle

:AbandonedVehicle rdf:type owl:Class ;
                  
                  rdfs:label "Abandoned Vehicle"^^xsd:string ;
                  
                  rdfs:subClassOf :VehicleObstruction ;
                  
                  rdfs:comment "Abandoned vehicle(s) which may cause traffic disruption. This concept and description are a generalised version of the DATEX II concept abandonedVehicle."^^xsd:string ;
                  
                  rdfs:seeAlso "http://datex2.eu/schema/2/2_0#AbandonedVehicle" .



###  http://purl.org/td/transportdisruption#AbnormalLoad

:AbnormalLoad rdf:type owl:Class ;
              
              rdfs:label "Abnormal Load"^^xsd:string ;
              
              rdfs:subClassOf :VehicleObstruction ;
              
              rdfs:comment "Vehicle(s) carrying exceptional load(s) which may cause traffic disruption. This concept and description are from the DATEX II concept abnormalLoad."^^xsd:string ;
              
              rdfs:seeAlso "http://datex2.eu/schema/2/2_0#AbnormalLoad" .



###  http://purl.org/td/transportdisruption#AbnormalTraffic

:AbnormalTraffic rdf:type owl:Class ;
                 
                 rdfs:label "Abnormal Traffic"^^xsd:string ;
                 
                 rdfs:subClassOf :TrafficElementEvent ;
                 
                 rdfs:comment "A traffic condition which is not normal. This concept and description are from the DATEX II concept AbnormalTraffic."^^xsd:string ;
                 
                 rdfs:seeAlso "http://datex2.eu/schema/2/2_0#AbnormalTraffic" .



###  http://purl.org/td/transportdisruption#Accident

:Accident rdf:type owl:Class ;
          
          rdfs:label "Accident"^^xsd:string ;
          
          rdfs:subClassOf :TrafficElementEvent ;
          
          rdfs:comment "Accidents are situations in which one or more vehicles lose control and do not recover.  They include collisions between vehicle(s) or other network user(s), between vehicle(s) and fixed obstacle(s), or they result from a vehicle running off the network infrastructure. This concept and description are a generalised version of the DATEX II concept accident."^^xsd:string ;
          
          rdfs:seeAlso "http://datex2.eu/schema/2/2_0#Accident" .



###  http://purl.org/td/transportdisruption#AccidentInvestigationWork

:AccidentInvestigationWork rdf:type owl:Class ;
                           
                           rdfs:label "Accident Investigation Work"^^xsd:string ;
                           
                           rdfs:subClassOf :AuthorityOperation ;
                           
                           rdfs:comment "An operation involving authorised investigation work connected to an earlier reported accident. This concept and description are from the DATEX II concept accidentInvestigationWork."^^xsd:string ;
                           
                           rdfs:seeAlso "http://datex2.eu/schema/2/2_0#AccidentInvestigationWork" .



###  http://purl.org/td/transportdisruption#AccidentInvolvingBicycles

:AccidentInvolvingBicycles rdf:type owl:Class ;
                           
                           rdfs:label "Accident Involving Bicycles"^^xsd:string ;
                           
                           rdfs:subClassOf :AccidentInvolvingObject ;
                           
                           rdfs:comment "Includes all accidents involving at least one bicycle. This concept and description are from the DATEX II concept accidentInvolvingBicycles."^^xsd:string ;
                           
                           rdfs:seeAlso "http://datex2.eu/schema/2/2_0#AccidentInvolvingBicycles" .



###  http://purl.org/td/transportdisruption#AccidentInvolvingBuses

:AccidentInvolvingBuses rdf:type owl:Class ;
                        
                        rdfs:label "Accident Involving Buses"^^xsd:string ;
                        
                        rdfs:subClassOf :AccidentInvolvingObject ;
                        
                        rdfs:comment "Includes all accidents involving at least one passenger vehicle. This concept and description are from the DATEX II concept accidentInvolvingBuses."^^xsd:string ;
                        
                        rdfs:seeAlso "http://datex2.eu/schema/2/2_0#AccidentInvolvingBuses" .



###  http://purl.org/td/transportdisruption#AccidentInvolvingHazardousMaterials

:AccidentInvolvingHazardousMaterials rdf:type owl:Class ;
                                     
                                     rdfs:label "Accident Involving Hazardous Materials"^^xsd:string ;
                                     
                                     rdfs:subClassOf :AccidentInvolvingObject ;
                                     
                                     rdfs:comment "Includes all accidents involving at least one vehicle believed to be carrying materials, which could present an additional hazard to others. This concept and description are a generalised version of the DATEX II concept accidentInvolvingHazardousMaterials."^^xsd:string ;
                                     
                                     rdfs:seeAlso "http://datex2.eu/schema/2/2_0#AccidentInvolvingHazardousMaterials" .



###  http://purl.org/td/transportdisruption#AccidentInvolvingHeavyLorries

:AccidentInvolvingHeavyLorries rdf:type owl:Class ;
                               
                               rdfs:label "Accident Involving Heavy Lorries"^^xsd:string ;
                               
                               rdfs:subClassOf :AccidentInvolvingObject ;
                               
                               rdfs:comment "Includes all accidents involving at least one heavy goods vehicle. This concept and description are from the DATEX II concept accidentInvolvingHeavyLorries."^^xsd:string ;
                               
                               rdfs:seeAlso "http://datex2.eu/schema/2/2_0#AccidentInvolvingHeavyLorries" .



###  http://purl.org/td/transportdisruption#AccidentInvolvingMassTransitVehicle

:AccidentInvolvingMassTransitVehicle rdf:type owl:Class ;
                                     
                                     rdfs:label "Accident Involving Mass Transit Vehicle"^^xsd:string ;
                                     
                                     rdfs:subClassOf :AccidentInvolvingObject ;
                                     
                                     rdfs:comment "Includes all accidents involving at least one mass transit vehicle. This concept and description are from the DATEX II concept accidentInvolvingMassTransitVehicle."^^xsd:string ;
                                     
                                     rdfs:seeAlso "http://datex2.eu/schema/2/2_0#AccidentInvolvingMassTransitVehicle" .



###  http://purl.org/td/transportdisruption#AccidentInvolvingMopeds

:AccidentInvolvingMopeds rdf:type owl:Class ;
                         
                         rdfs:label "Accident Involving Mopeds"^^xsd:string ;
                         
                         rdfs:subClassOf :AccidentInvolvingObject ;
                         
                         rdfs:comment "Includes all accidents involving at least one moped. This concept and description are from the DATEX II concept accidentInvolvingMopeds."^^xsd:string ;
                         
                         rdfs:seeAlso "http://datex2.eu/schema/2/2_0#AccidentInvolvingMopeds" .



###  http://purl.org/td/transportdisruption#AccidentInvolvingMotorcycles

:AccidentInvolvingMotorcycles rdf:type owl:Class ;
                              
                              rdfs:label "Accident Involving Motorcycles"^^xsd:string ;
                              
                              rdfs:subClassOf :AccidentInvolvingObject ;
                              
                              rdfs:comment "Includes all accidents involving at least one motorcycle. This concept and description are from the DATEX II concept accidentInvolvingMotorcycles."^^xsd:string ;
                              
                              rdfs:seeAlso "http://datex2.eu/schema/2/2_0#AccidentInvolvingMotorcycles" .



###  http://purl.org/td/transportdisruption#AccidentInvolvingObject

:AccidentInvolvingObject rdf:type owl:Class ;
                         
                         rdfs:label "Accident Involving Object"^^xsd:string ;
                         
                         rdfs:subClassOf :Accident ;
                         
                         rdfs:comment "Includes all accidents involving a vehicle or other type of object."^^xsd:string .



###  http://purl.org/td/transportdisruption#AccidentInvolvingRadioactiveMaterial

:AccidentInvolvingRadioactiveMaterial rdf:type owl:Class ;
                                      
                                      rdfs:label "Accident Involving Radioactive Material"^^xsd:string ;
                                      
                                      rdfs:subClassOf :AccidentInvolvingObject ;
                                      
                                      rdfs:comment "Accident involving radioactive material. This concept and description are from the DATEX II concept accidentInvolvingRadioactiveMaterial."^^xsd:string ;
                                      
                                      rdfs:seeAlso "http://datex2.eu/schema/2/2_0#AccidentInvolvingRadioactiveMaterial" .



###  http://purl.org/td/transportdisruption#AccidentInvolvingTrain

:AccidentInvolvingTrain rdf:type owl:Class ;
                        
                        rdfs:label "Accident Involving Train"^^xsd:string ;
                        
                        rdfs:subClassOf :AccidentInvolvingObject ;
                        
                        rdfs:comment "Includes all accidents involving collision with a train. This concept and description are from the DATEX II concept accidentInvolvingTrain."^^xsd:string ;
                        
                        rdfs:seeAlso "http://datex2.eu/schema/2/2_0#AccidentInvolvingTrain" .



###  http://purl.org/td/transportdisruption#ActiveSpeedControlInOperation

:ActiveSpeedControlInOperation rdf:type owl:Class ;
                               
                               rdfs:label "Active Speed Control In Operation"^^xsd:string ;
                               
                               rdfs:subClassOf :SpeedManagement ;
                               
                               rdfs:comment "Automatic speed control measures are in place at the specified location, whereby speed limits are set by an automatic system which is triggered by traffic sensing equipment. This concept and description are from the DATEX II concept activeSpeedControlInOperation."^^xsd:string ;
                               
                               rdfs:seeAlso "http://datex2.eu/schema/2/2_0#ActiveSpeedControlInOperation" .



###  http://purl.org/td/transportdisruption#Activity

:Activity rdf:type owl:Class ;
          
          rdfs:label "Activity"^^xsd:string ;
          
          rdfs:subClassOf :TrafficElementEvent ;
          
          rdfs:comment "Deliberate human action external to the traffic stream or infrastructure which could disrupt traffic. This concept and description are an adaptation of the DATEX II concept Activity."^^xsd:string ;
          
          rdfs:seeAlso "http://datex2.eu/schema/2/2_0#Activity" .



###  http://purl.org/td/transportdisruption#AdverseInfrastructureConditions

:AdverseInfrastructureConditions rdf:type owl:Class ;
                                 
                                 rdfs:label "Non Weather Related Road Condition Type Enum"^^xsd:string ;
                                 
                                 rdfs:subClassOf :Conditions ;
                                 
                                 rdfs:comment "Types of road surface conditions which are not related to the weather. This concept and description are from the DATEX II concept NonWeatherRelatedRoadConditionTypeEnum."^^xsd:string ;
                                 
                                 rdfs:seeAlso "http://datex2.eu/schema/2/2_0#NonWeatherRelatedRoadConditionTypeEnum" .



###  http://purl.org/td/transportdisruption#AgriculturalShow

:AgriculturalShow rdf:type owl:Class ;
                  
                  rdfs:label "Agricultural Show"^^xsd:string ;
                  
                  rdfs:subClassOf :PublicEvent ;
                  
                  rdfs:comment "Agricultural show or event which could disrupt traffic. This concept and description are from the DATEX II concept agriculturalShow."^^xsd:string ;
                  
                  rdfs:seeAlso "http://datex2.eu/schema/2/2_0#AgriculturalShow" .



###  http://purl.org/td/transportdisruption#AirAmbulance

:AirAmbulance rdf:type owl:Class ;
              
              rdfs:label "Air Ambulance"^^xsd:string ;
              
              rdfs:subClassOf :InfrastructureSideAssistance ;
              
              rdfs:comment "Air ambulance assistance. This concept and description are from the DATEX II concept airAmbulance."^^xsd:string ;
              
              rdfs:seeAlso "http://datex2.eu/schema/2/2_0#AirAmbulance" .



###  http://purl.org/td/transportdisruption#AirRaid

:AirRaid rdf:type owl:Class ;
         
         rdfs:label "Air Raid"^^xsd:string ;
         
         rdfs:subClassOf :DisturbanceActivity ;
         
         rdfs:comment "A situation relating to any threat from foreign air power. This concept and description are from the DATEX II concept airRaid."^^xsd:string ;
         
         rdfs:seeAlso "http://datex2.eu/schema/2/2_0#AirRaid" .



###  http://purl.org/td/transportdisruption#AirShow

:AirShow rdf:type owl:Class ;
         
         rdfs:label "Air Show"^^xsd:string ;
         
         rdfs:subClassOf :PublicEvent ;
         
         rdfs:comment "Air show or other aeronautical event which could disrupt traffic. This concept and description are from the DATEX II concept airShow."^^xsd:string ;
         
         rdfs:seeAlso "http://datex2.eu/schema/2/2_0#AirShow" .



###  http://purl.org/td/transportdisruption#AircraftOffInfrastructure

:AircraftOffInfrastructure rdf:type owl:Class ;
                           
                           rdfs:label "Aircraft Off Infrastructure"^^xsd:string ;
                           
                           rdfs:subClassOf :VehicleOffInfrastructure ;
                           
                           rdfs:comment "Includes all accidents where one or more aircraft have left the runway, taxiway, etc."^^xsd:string .



###  http://purl.org/td/transportdisruption#AltercationOfVehicleOccupants

:AltercationOfVehicleOccupants rdf:type owl:Class ;
                               
                               rdfs:label "Altercation Of Vehicle Occupants"^^xsd:string ;
                               
                               rdfs:subClassOf :DisturbanceActivity ;
                               
                               rdfs:comment "An altercation (argument, dispute or fight) between two or more vehicle occupants. This concept and description are from the DATEX II concept altercationOfVehicleOccupants."^^xsd:string ;
                               
                               rdfs:seeAlso "http://datex2.eu/schema/2/2_0#AltercationOfVehicleOccupants" .



###  http://purl.org/td/transportdisruption#AnimalPresenceObstruction

:AnimalPresenceObstruction rdf:type owl:Class ;
                           
                           rdfs:label "Animal Presence Obstruction"^^xsd:string ;
                           
                           rdfs:subClassOf :Obstruction ;
                           
                           rdfs:comment "An obstruction resulting from the presence of animals. This concept and description are a generalised version of the DATEX II concept AnimalPresenceObstruction."^^xsd:string ;
                           
                           rdfs:seeAlso "http://datex2.eu/schema/2/2_0#AnimalPresenceObstruction" .



###  http://purl.org/td/transportdisruption#AnimalsOnTheInfrastructure

:AnimalsOnTheInfrastructure rdf:type owl:Class ;
                            
                            rdfs:label "Animals On The Infrastructure"^^xsd:string ;
                            
                            rdfs:subClassOf :AnimalPresenceObstruction ;
                            
                            rdfs:comment "Traffic may be disrupted due to animals on transport infrastructure. This concept and description are a generalised version of the DATEX II concept animalsOnTheRoad."^^xsd:string ;
                            
                            rdfs:seeAlso "http://datex2.eu/schema/2/2_0#AnimalsOnTheRoad" .



###  http://purl.org/td/transportdisruption#AnprCameraFailure

:AnprCameraFailure rdf:type owl:Class ;
                   
                   rdfs:label "Anpr Camera Failure"^^xsd:string ;
                   
                   rdfs:subClassOf :InfrastructureFailure ;
                   
                   rdfs:comment "Failure of automatic number plate recognition cameras. This concept and description are based on the DATEX II concept anprCameras."^^xsd:string ;
                   
                   rdfs:seeAlso "http://datex2.eu/schema/2/2_0#AnprCameras" .



###  http://purl.org/td/transportdisruption#AnprCamerasFault

:AnprCamerasFault rdf:type owl:Class ;
                  
                  rdfs:label "Anpr Camera Fault"^^xsd:string ;
                  
                  rdfs:subClassOf :InfrastructureFault ;
                  
                  rdfs:comment "Faulty or malfunctioning automatic number plate recognition cameras. This concept and description are based on the DATEX II concept anprCameras."^^xsd:string ;
                  
                  rdfs:seeAlso "http://datex2.eu/schema/2/2_0#AnprCameras" .



###  http://purl.org/td/transportdisruption#Assault

:Assault rdf:type owl:Class ;
         
         rdfs:label "Assault"^^xsd:string ;
         
         rdfs:subClassOf :DisturbanceActivity ;
         
         rdfs:comment "A situation where an assault has taken place on one or more persons. This concept and description are from the DATEX II concept assault."^^xsd:string ;
         
         rdfs:seeAlso "http://datex2.eu/schema/2/2_0#Assault" .



###  http://purl.org/td/transportdisruption#AssetDestruction

:AssetDestruction rdf:type owl:Class ;
                  
                  rdfs:label "Asset Destruction"^^xsd:string ;
                  
                  rdfs:subClassOf :DisturbanceActivity ;
                  
                  rdfs:comment "A situation where assets of one or more persons or authorities have been destroyed. This concept and description are from the DATEX II concept assetDestruction."^^xsd:string ;
                  
                  rdfs:seeAlso "http://datex2.eu/schema/2/2_0#AssetDestruction" .



###  http://purl.org/td/transportdisruption#AthleticsMeeting

:AthleticsMeeting rdf:type owl:Class ;
                  
                  rdfs:label "Athletics Meeting"^^xsd:string ;
                  
                  rdfs:subClassOf :PublicEvent ;
                  
                  rdfs:comment "Athletics event that could disrupt traffic. This concept and description are from the DATEX II concept athleticsMeeting."^^xsd:string ;
                  
                  rdfs:seeAlso "http://datex2.eu/schema/2/2_0#AthleticsMeeting" .



###  http://purl.org/td/transportdisruption#Attack

:Attack rdf:type owl:Class ;
        
        rdfs:label "Attack"^^xsd:string ;
        
        rdfs:subClassOf :DisturbanceActivity ;
        
        rdfs:comment "A situation where an attack on a group of people or properties has taken place. This concept and description are from the DATEX II concept attack."^^xsd:string ;
        
        rdfs:seeAlso "http://datex2.eu/schema/2/2_0#Attack" .



###  http://purl.org/td/transportdisruption#AttackOnVehicle

:AttackOnVehicle rdf:type owl:Class ;
                 
                 rdfs:label "Attack On Vehicle"^^xsd:string ;
                 
                 rdfs:subClassOf :DisturbanceActivity ;
                 
                 rdfs:comment "A situation where an attack on a vehicle or its occupants has taken place. This concept and description are from the DATEX II concept attackOnVehicle."^^xsd:string ;
                 
                 rdfs:seeAlso "http://datex2.eu/schema/2/2_0#AttackOnVehicle" .



###  http://purl.org/td/transportdisruption#AuthorityOperation

:AuthorityOperation rdf:type owl:Class ;
                    
                    rdfs:label "Authority Operation"^^xsd:string ;
                    
                    rdfs:subClassOf :Activity ;
                    
                    rdfs:comment "Authority initiated operation or activity that could disrupt traffic. This concept and description are from the DATEX II concept AuthorityOperation."^^xsd:string ;
                    
                    rdfs:seeAlso "http://datex2.eu/schema/2/2_0#AuthorityOperation" .



###  http://purl.org/td/transportdisruption#AutomatedTollSystemFailure

:AutomatedTollSystemFailure rdf:type owl:Class ;
                            
                            rdfs:label "Automated Toll System Failure"^^xsd:string ;
                            
                            rdfs:subClassOf :InfrastructureFailure ;
                            
                            rdfs:comment "Failure of an automated toll system. This concept and description are based on the DATEX II concept automatedTollSystem."^^xsd:string ;
                            
                            rdfs:seeAlso "http://datex2.eu/schema/2/2_0#AutomatedTollSystem" .



###  http://purl.org/td/transportdisruption#AutomatedTollSystemFault

:AutomatedTollSystemFault rdf:type owl:Class ;
                          
                          rdfs:label "Automated Toll System Fault"^^xsd:string ;
                          
                          rdfs:subClassOf :InfrastructureFault ;
                          
                          rdfs:comment "Faulty or malfunctioning automated toll system. This concept and description are based on the DATEX II concept automatedTollSystem."^^xsd:string ;
                          
                          rdfs:seeAlso "http://datex2.eu/schema/2/2_0#AutomatedTollSystem" .



###  http://purl.org/td/transportdisruption#Avalanches

:Avalanches rdf:type owl:Class ;
            
            rdfs:label "Avalanches"^^xsd:string ;
            
            rdfs:subClassOf :EnvironmentalObstruction ;
            
            rdfs:comment "The transport infrastructure obstructed or partially obstructed due to snow slides. This concept and description are a generalised version of the DATEX II concept avalanches."^^xsd:string ;
            
            rdfs:seeAlso "http://datex2.eu/schema/2/2_0#Avalanches" .



###  http://purl.org/td/transportdisruption#BadWeather

:BadWeather rdf:type owl:Class ;
            
            rdfs:label "Bad Weather"^^xsd:string ;
            
            rdfs:subClassOf :EnvironmentalConditions ;
            
            rdfs:comment "Adverse weather conditions are affecting the transport network. This concept and description are a generalised version of the DATEX II concept badWeather."^^xsd:string ;
            
            rdfs:seeAlso "http://datex2.eu/schema/2/2_0#BadWeather" .



###  http://purl.org/td/transportdisruption#BallGame

:BallGame rdf:type owl:Class ;
          
          rdfs:label "Ball Game"^^xsd:string ;
          
          rdfs:subClassOf :PublicEvent ;
          
          rdfs:comment "Ball game event that could disrupt traffic. This concept and description are from the DATEX II concept ballGame."^^xsd:string ;
          
          rdfs:seeAlso "http://datex2.eu/schema/2/2_0#BallGame" .



###  http://purl.org/td/transportdisruption#BaseballGame

:BaseballGame rdf:type owl:Class ;
              
              rdfs:label "Baseball Game"^^xsd:string ;
              
              rdfs:subClassOf :PublicEvent ;
              
              rdfs:comment "Baseball game event that could disrupt traffic. This concept and description are from the DATEX II concept baseballGame."^^xsd:string ;
              
              rdfs:seeAlso "http://datex2.eu/schema/2/2_0#BaseballGame" .



###  http://purl.org/td/transportdisruption#BasketballGame

:BasketballGame rdf:type owl:Class ;
                
                rdfs:label "Basketball Game"^^xsd:string ;
                
                rdfs:subClassOf :PublicEvent ;
                
                rdfs:comment "Basketball game event that could disrupt traffic. This concept and description are from the DATEX II concept basketballGame."^^xsd:string ;
                
                rdfs:seeAlso "http://datex2.eu/schema/2/2_0#BasketballGame" .



###  http://purl.org/td/transportdisruption#BicycleRace

:BicycleRace rdf:type owl:Class ;
             
             rdfs:label "Bicycle Race"^^xsd:string ;
             
             rdfs:subClassOf :PublicEvent ;
             
             rdfs:comment "Bicycle race that could disrupt traffic. This concept and description are from the DATEX II concept bicycleRace."^^xsd:string ;
             
             rdfs:seeAlso "http://datex2.eu/schema/2/2_0#BicycleRace" .



###  http://purl.org/td/transportdisruption#BlackIce

:BlackIce rdf:type owl:Class ;
          
          rdfs:label "Black Ice"^^xsd:string ;
          
          rdfs:subClassOf :WeatherRelatedConditions ;
          
          rdfs:comment "Black ice (i.e. clear ice, which is impossible or very difficult to see). This concept and description are adaptations the DATEX II concept blackIce."^^xsd:string ;
          
          rdfs:seeAlso "http://datex2.eu/schema/2/2_0#BlackIce" .



###  http://purl.org/td/transportdisruption#BlastingWork

:BlastingWork rdf:type owl:Class ;
              
              rdfs:label "Blasting Work"^^xsd:string ;
              
              rdfs:subClassOf :InfrastructureConstruction ;
              
              rdfs:comment "Blasting or quarrying work at the specified location. This concept and description are from the DATEX II concept blastingWork."^^xsd:string ;
              
              rdfs:seeAlso "http://datex2.eu/schema/2/2_0#BlastingWork" .



###  http://purl.org/td/transportdisruption#Blizzard

:Blizzard rdf:type owl:Class ;
          
          rdfs:label "Blizzard"^^xsd:string ;
          
          rdfs:subClassOf :EnvironmentalConditions ;
          
          rdfs:comment "Heavy snowfall in combination with strong winds, limiting visibility to 50m or less. This concept and description are from the DATEX II concept blizzard."^^xsd:string ;
          
          rdfs:seeAlso "http://datex2.eu/schema/2/2_0#Blizzard" .



###  http://purl.org/td/transportdisruption#BlockadeOrBarrier

:BlockadeOrBarrier rdf:type owl:Class ;
                   
                   rdfs:label "Blockade Or Barrier"^^xsd:string ;
                   
                   rdfs:subClassOf :DisturbanceActivity ;
                   
                   rdfs:comment "A manned blockade or barrier across a road stopping vehicles passing. This concept and description are from the DATEX II concept blockadeOrBarrier."^^xsd:string ;
                   
                   rdfs:seeAlso "http://datex2.eu/schema/2/2_0#BlockadeOrBarrier" .



###  http://purl.org/td/transportdisruption#BlowingDust

:BlowingDust rdf:type owl:Class ;
             
             rdfs:label "Blowing Dust"^^xsd:string ;
             
             rdfs:subClassOf :EnvironmentalConditions ;
             
             rdfs:comment "Dust blowing causing significantly reduced visibility. This concept and description are a generalised version of the DATEX II concept blowingDust."^^xsd:string ;
             
             rdfs:seeAlso "http://datex2.eu/schema/2/2_0#BlowingDust" .



###  http://purl.org/td/transportdisruption#BlowingSnow

:BlowingSnow rdf:type owl:Class ;
             
             rdfs:label "Blowing Snow"^^xsd:string ;
             
             rdfs:subClassOf :EnvironmentalConditions ;
             
             rdfs:comment "Fallen snow moving due to the forces of wind. This concept and description are from the DATEX II concept blowingSnow."^^xsd:string ;
             
             rdfs:seeAlso "http://datex2.eu/schema/2/2_0#BlowingSnow" .



###  http://purl.org/td/transportdisruption#BoatRace

:BoatRace rdf:type owl:Class ;
          
          rdfs:label "Boat Race"^^xsd:string ;
          
          rdfs:subClassOf :PublicEvent ;
          
          rdfs:comment "Regatta (boat race event of sailing, powerboat or rowing) that could disrupt traffic. This concept and description are from the DATEX II concept boatRace."^^xsd:string ;
          
          rdfs:seeAlso "http://datex2.eu/schema/2/2_0#BoatRace" .



###  http://purl.org/td/transportdisruption#BoatShow

:BoatShow rdf:type owl:Class ;
          
          rdfs:label "Boat Show"^^xsd:string ;
          
          rdfs:subClassOf :PublicEvent ;
          
          rdfs:comment "Boat show which could disrupt traffic. This concept and description are from the DATEX II concept boatShow."^^xsd:string ;
          
          rdfs:seeAlso "http://datex2.eu/schema/2/2_0#BoatShow" .



###  http://purl.org/td/transportdisruption#BombAlert

:BombAlert rdf:type owl:Class ;
           
           rdfs:label "Bomb Alert"^^xsd:string ;
           
           rdfs:subClassOf :DisturbanceActivity ;
           
           rdfs:comment "An alert to a situation where suspected or actual explosive or incendiary devices may cause disruption to traffic. This concept and description are from the DATEX II concept bombAlert."^^xsd:string ;
           
           rdfs:seeAlso "http://datex2.eu/schema/2/2_0#BombAlert" .



###  http://purl.org/td/transportdisruption#BombSquadInAction

:BombSquadInAction rdf:type owl:Class ;
                   
                   rdfs:label "Bomb Squad In Action"^^xsd:string ;
                   
                   rdfs:subClassOf :AuthorityOperation ;
                   
                   rdfs:comment "An operation where a bomb squad is in action to deal with suspected or actual explosive or incendiary devices which may cause disruption to traffic. This concept and description are from the DATEX II concept bombSquadInAction."^^xsd:string ;
                   
                   rdfs:seeAlso "http://datex2.eu/schema/2/2_0#BombSquadInAction" .



###  http://purl.org/td/transportdisruption#BoxingTournament

:BoxingTournament rdf:type owl:Class ;
                  
                  rdfs:label "Boxing Tournament"^^xsd:string ;
                  
                  rdfs:subClassOf :PublicEvent ;
                  
                  rdfs:comment "Boxing event that could disrupt traffic. This concept and description are from the DATEX II concept boxingTournament."^^xsd:string ;
                  
                  rdfs:seeAlso "http://datex2.eu/schema/2/2_0#BoxingTournament" .



###  http://purl.org/td/transportdisruption#BridgeSwingInOperation

:BridgeSwingInOperation rdf:type owl:Class ;
                        
                        rdfs:label "Bridge Swing In Operation"^^xsd:string ;
                        
                        rdfs:subClassOf :GeneralNetworkManagement ;
                        
                        rdfs:comment "The bridge at the specified location has swung or lifted and is therefore temporarily closed to traffic. This concept and description are from the DATEX II concept bridgeSwingInOperation."^^xsd:string ;
                        
                        rdfs:seeAlso "http://datex2.eu/schema/2/2_0#BridgeSwingInOperation" .



###  http://purl.org/td/transportdisruption#BrokenDownBus

:BrokenDownBus rdf:type owl:Class ;
               
               rdfs:label "Broken Down Bus"^^xsd:string ;
               
               rdfs:subClassOf :BrokenDownVehicle ;
               
               rdfs:comment "Broken down passenger vehicle(s) on the carriageway which may cause traffic disruption. This concept and description are from the DATEX II concept brokenDownBus."^^xsd:string ;
               
               rdfs:seeAlso "http://datex2.eu/schema/2/2_0#BrokenDownBus" .



###  http://purl.org/td/transportdisruption#BrokenDownHeavyLorry

:BrokenDownHeavyLorry rdf:type owl:Class ;
                      
                      rdfs:label "Broken Down Heavy Lorry"^^xsd:string ;
                      
                      rdfs:subClassOf :BrokenDownVehicle ;
                      
                      rdfs:comment "Broken down heavy lorry/lorries on the carriageway which may cause traffic disruption. This concept and description are from the DATEX II concept brokenDownHeavyLorry."^^xsd:string ;
                      
                      rdfs:seeAlso "http://datex2.eu/schema/2/2_0#BrokenDownHeavyLorry" .



###  http://purl.org/td/transportdisruption#BrokenDownTrain

:BrokenDownTrain rdf:type owl:Class ;
                 
                 rdfs:label "Broken Down Train"^^xsd:string ;
                 
                 rdfs:subClassOf :BrokenDownVehicle ;
                 
                 rdfs:comment "Broken down passenger vehicle(s) on the railway which may cause traffic disruption."^^xsd:string .



###  http://purl.org/td/transportdisruption#BrokenDownVehicle

:BrokenDownVehicle rdf:type owl:Class ;
                   
                   rdfs:label "Broken Down Vehicle"^^xsd:string ;
                   
                   rdfs:subClassOf :VehicleObstruction ;
                   
                   rdfs:comment "Broken down vehicle(s) which may cause traffic disruption. This concept and description are a generalised version of the DATEX II concept brokenDownVehicle."^^xsd:string ;
                   
                   rdfs:seeAlso "http://datex2.eu/schema/2/2_0#BrokenDownVehicle" .



###  http://purl.org/td/transportdisruption#BullFight

:BullFight rdf:type owl:Class ;
           
           rdfs:label "Bull Fight"^^xsd:string ;
           
           rdfs:subClassOf :PublicEvent ;
           
           rdfs:comment "Bull fighting event that could disrupt traffic. This concept and description are from the DATEX II concept bullFight."^^xsd:string ;
           
           rdfs:seeAlso "http://datex2.eu/schema/2/2_0#BullFight" .



###  http://purl.org/td/transportdisruption#BurstPipe

:BurstPipe rdf:type owl:Class ;
           
           rdfs:label "Burst Pipe"^^xsd:string ;
           
           rdfs:subClassOf :InfrastructureDamageObstruction ;
           
           rdfs:comment "The infrastructure surface has sunken or collapsed in places due to burst pipes. This concept and description are a generalised version of the DATEX II concept burstPipe."^^xsd:string ;
           
           rdfs:seeAlso "http://datex2.eu/schema/2/2_0#BurstPipe" .



###  http://purl.org/td/transportdisruption#BurstWaterMain

:BurstWaterMain rdf:type owl:Class ;
                
                rdfs:label "Burst Water Main"^^xsd:string ;
                
                rdfs:subClassOf :InfrastructureDamageObstruction ;
                
                rdfs:comment "Traffic may be disrupted due to local flooding and/or subsidence because of a broken water main. This concept and description are from the DATEX II concept burstWaterMain."^^xsd:string ;
                
                rdfs:seeAlso "http://datex2.eu/schema/2/2_0#BurstWaterMain" .



###  http://purl.org/td/transportdisruption#CarPoolLaneInOperation

:CarPoolLaneInOperation rdf:type owl:Class ;
                        
                        rdfs:label "Car Pool Lane In Operation"^^xsd:string ;
                        
                        rdfs:subClassOf :RoadOrCarriagewayOrLaneManagement ;
                        
                        rdfs:comment "Dedicated car pool lane(s) are in operation for vehicles carrying at least the specified number of occupants. This concept and description are from the DATEX II concept carPoolLaneInOperation."^^xsd:string ;
                        
                        rdfs:seeAlso "http://datex2.eu/schema/2/2_0#CarPoolLaneInOperation" .



###  http://purl.org/td/transportdisruption#CarriagewayClosures

:CarriagewayClosures rdf:type owl:Class ;
                     
                     rdfs:label "Carriageway Closures"^^xsd:string ;
                     
                     rdfs:subClassOf :RoadOrCarriagewayOrLaneManagement ;
                     
                     rdfs:comment "Carriageway closures are in operation at the specified location. This concept and description are from the DATEX II concept carriagewayClosures."^^xsd:string ;
                     
                     rdfs:seeAlso "http://datex2.eu/schema/2/2_0#CarriagewayClosures" .



###  http://purl.org/td/transportdisruption#CctvCamerasFailure

:CctvCamerasFailure rdf:type owl:Class ;
                    
                    rdfs:label "Cctv Camera Failure"^^xsd:string ;
                    
                    rdfs:subClassOf :InfrastructureFailure ;
                    
                    rdfs:comment "Failure of closed-circuit television cameras. This concept and description are based on the DATEX II concept cctvCameras."^^xsd:string ;
                    
                    rdfs:seeAlso "http://datex2.eu/schema/2/2_0#CctvCameras" .



###  http://purl.org/td/transportdisruption#CctvCamerasFault

:CctvCamerasFault rdf:type owl:Class ;
                  
                  rdfs:label "Cctv Camera Fault"^^xsd:string ;
                  
                  rdfs:subClassOf :InfrastructureFault ;
                  
                  rdfs:comment "Faulty or malfunctioning closed-circuit television cameras. This concept and description are based on the DATEX II concept cctvCameras."^^xsd:string ;
                  
                  rdfs:seeAlso "http://datex2.eu/schema/2/2_0#CctvCameras" .



###  http://purl.org/td/transportdisruption#CeremonialEvent

:CeremonialEvent rdf:type owl:Class ;
                 
                 rdfs:label "Ceremonial Event"^^xsd:string ;
                 
                 rdfs:subClassOf :PublicEvent ;
                 
                 rdfs:comment "Formal or religious act, rite or ceremony that could disrupt traffic. This concept and description are from the DATEX II concept ceremonialEvent."^^xsd:string ;
                 
                 rdfs:seeAlso "http://datex2.eu/schema/2/2_0#CeremonialEvent" .



###  http://purl.org/td/transportdisruption#ChemicalSpillageAccident

:ChemicalSpillageAccident rdf:type owl:Class ;
                          
                          rdfs:label "Chemical Spillage Accident"^^xsd:string ;
                          
                          rdfs:subClassOf :SpillageAccident ;
                          
                          rdfs:comment "Includes all situations resulting in a spillage of chemicals. This concept and description are a generalised version of the DATEX II concept chemicalSpillageAccident."^^xsd:string ;
                          
                          rdfs:seeAlso "http://datex2.eu/schema/2/2_0#ChemicalSpillageAccident" .



###  http://purl.org/td/transportdisruption#CivilEmergency

:CivilEmergency rdf:type owl:Class ;
                
                rdfs:label "Civil Emergency"^^xsd:string ;
                
                rdfs:subClassOf :AuthorityOperation ;
                
                rdfs:comment "A situation, perceived or actual, relating to a civil emergency which could disrupt traffic.  This includes large scale destruction, through events such as earthquakes, insurrection, and civil disobedience. This concept and description are from the DATEX II concept civilEmergency."^^xsd:string ;
                
                rdfs:seeAlso "http://datex2.eu/schema/2/2_0#CivilEmergency" .



###  http://purl.org/td/transportdisruption#ClearanceWork

:ClearanceWork rdf:type owl:Class ;
               
               rdfs:label "Clearance Work"^^xsd:string ;
               
               rdfs:subClassOf :InfrastructureMaintenance ;
               
               rdfs:comment "Clearance work of an unspecified nature. This concept and description are from the DATEX II concept clearanceWork."^^xsd:string ;
               
               rdfs:seeAlso "http://datex2.eu/schema/2/2_0#ClearanceWork" .



###  http://purl.org/td/transportdisruption#ClosedPermanentlyForTheWinter

:ClosedPermanentlyForTheWinter rdf:type owl:Class ;
                               
                               rdfs:label "Closed Permanently For The Winter"^^xsd:string ;
                               
                               rdfs:subClassOf :RoadOrCarriagewayOrLaneManagement ;
                               
                               rdfs:comment "The road is closed to vehicles for the duration of the winter. This concept and description are adaptations of the DATEX II concept closedPermanentlyForTheWinter."^^xsd:string ;
                               
                               rdfs:seeAlso "http://datex2.eu/schema/2/2_0#ClosedPermanentlyForTheWinter" .



###  http://purl.org/td/transportdisruption#CollapsedBridge

:CollapsedBridge rdf:type owl:Class ;
                 
                 rdfs:label "Collapsed Bridge"^^xsd:string ;
                 
                 rdfs:subClassOf :InfrastructureFailure ;
                 
                 rdfs:comment "A bridge that has collapsed."^^xsd:string .



###  http://purl.org/td/transportdisruption#CollapsedSewer

:CollapsedSewer rdf:type owl:Class ;
                
                rdfs:label "Collapsed Sewer"^^xsd:string ;
                
                rdfs:subClassOf :InfrastructureDamageObstruction ;
                
                rdfs:comment "The infrastructure surface has sunken or collapsed in places due to sewer failure. This concept and description are a generalised version of the DATEX II concept collapsedSewer."^^xsd:string ;
                
                rdfs:seeAlso "http://datex2.eu/schema/2/2_0#CollapsedSewer" .



###  http://purl.org/td/transportdisruption#CollapsedTunnel

:CollapsedTunnel rdf:type owl:Class ;
                 
                 rdfs:label "Collapsed Tunnel"^^xsd:string ;
                 
                 rdfs:subClassOf :InfrastructureFailure ;
                 
                 rdfs:comment "Collapse of a entire or section of a tunnel."^^xsd:string .



###  http://purl.org/td/transportdisruption#Collision

:Collision rdf:type owl:Class ;
           
           rdfs:label "Collision"^^xsd:string ;
           
           rdfs:subClassOf :Accident ;
           
           rdfs:comment "Collision of vehicle with another object of unspecified type. This concept and description are from the DATEX II concept collision."^^xsd:string ;
           
           rdfs:seeAlso "http://datex2.eu/schema/2/2_0#Collision" .



###  http://purl.org/td/transportdisruption#CollisionWithAnimal

:CollisionWithAnimal rdf:type owl:Class ;
                     
                     rdfs:label "Collision With Animal"^^xsd:string ;
                     
                     rdfs:subClassOf :Collision ;
                     
                     rdfs:comment "Collision of vehicle with one or more animals. This concept and description are from the DATEX II concept collisionWithAnimal."^^xsd:string ;
                     
                     rdfs:seeAlso "http://datex2.eu/schema/2/2_0#CollisionWithAnimal" .



###  http://purl.org/td/transportdisruption#CollisionWithObstruction

:CollisionWithObstruction rdf:type owl:Class ;
                          
                          rdfs:label "Collision With Obstruction"^^xsd:string ;
                          
                          rdfs:subClassOf :Collision ;
                          
                          rdfs:comment "Collision of vehicle with an object of a stationary nature. This concept and description are from the DATEX II concept collisionWithObstruction."^^xsd:string ;
                          
                          rdfs:seeAlso "http://datex2.eu/schema/2/2_0#CollisionWithObstruction" .



###  http://purl.org/td/transportdisruption#CollisionWithPerson

:CollisionWithPerson rdf:type owl:Class ;
                     
                     rdfs:label "Collision With Person"^^xsd:string ;
                     
                     rdfs:subClassOf :Collision ;
                     
                     rdfs:comment "Collision of vehicle with one or more pedestrians. This concept and description are from the DATEX II concept collisionWithPerson."^^xsd:string ;
                     
                     rdfs:seeAlso "http://datex2.eu/schema/2/2_0#CollisionWithPerson" .



###  http://purl.org/td/transportdisruption#CommercialEvent

:CommercialEvent rdf:type owl:Class ;
                 
                 rdfs:label "Commercial Event"^^xsd:string ;
                 
                 rdfs:subClassOf :PublicEvent ;
                 
                 rdfs:comment "Commercial event which could disrupt traffic. This concept and description are from the DATEX II concept commercialEvent."^^xsd:string ;
                 
                 rdfs:seeAlso "http://datex2.eu/schema/2/2_0#CommercialEvent" .



###  http://purl.org/td/transportdisruption#Concert

:Concert rdf:type owl:Class ;
         
         rdfs:label "Concert"^^xsd:string ;
         
         rdfs:subClassOf :PublicEvent ;
         
         rdfs:comment "Concert event that could disrupt traffic. This concept and description are from the DATEX II concept concert."^^xsd:string ;
         
         rdfs:seeAlso "http://datex2.eu/schema/2/2_0#Concert" .



###  http://purl.org/td/transportdisruption#Conditions

:Conditions rdf:type owl:Class ;
            
            rdfs:label "Conditions"^^xsd:string ;
            
            rdfs:subClassOf :TrafficElementEvent ;
            
            rdfs:comment "Any conditions which have the potential to degrade normal driving conditions. This concept and description are from the DATEX II concept Conditions."^^xsd:string ;
            
            rdfs:seeAlso "http://datex2.eu/schema/2/2_0#Conditions" .



###  http://purl.org/td/transportdisruption#ConstructionWork

:ConstructionWork rdf:type owl:Class ;
                  
                  rdfs:label "Construction Work"^^xsd:string ;
                  
                  rdfs:subClassOf :InfrastructureConstruction ;
                  
                  rdfs:comment "Construction work of a general nature at the specified location. This concept and description are from the DATEX II concept constructionWork."^^xsd:string ;
                  
                  rdfs:seeAlso "http://datex2.eu/schema/2/2_0#ConstructionWork" .



###  http://purl.org/td/transportdisruption#Contraflow

:Contraflow rdf:type owl:Class ;
            
            rdfs:label "Contraflow"^^xsd:string ;
            
            rdfs:subClassOf :RoadOrCarriagewayOrLaneManagement ;
            
            rdfs:comment "Two-way traffic is temporarily sharing a single carriageway. This concept and description are from the DATEX II concept contraflow."^^xsd:string ;
            
            rdfs:seeAlso "http://datex2.eu/schema/2/2_0#Contraflow" .



###  http://purl.org/td/transportdisruption#ControlledAvalanche

:ControlledAvalanche rdf:type owl:Class ;
                     
                     rdfs:label "Controlled Avalanche"^^xsd:string ;
                     
                     rdfs:subClassOf :InfrastructureMaintenance ;
                     
                     rdfs:comment "Controlled avalanche work. This concept and description are from the DATEX II concept controlledAvalanche."^^xsd:string ;
                     
                     rdfs:seeAlso "http://datex2.eu/schema/2/2_0#ControlledAvalanche" .



###  http://purl.org/td/transportdisruption#Convoy

:Convoy rdf:type owl:Class ;
        
        rdfs:label "Convoy"^^xsd:string ;
        
        rdfs:subClassOf :VehicleObstruction ;
        
        rdfs:comment "A group of vehicles moving together in formation which may cause traffic disruption. This concept and description are from the DATEX II concept convoy."^^xsd:string ;
        
        rdfs:seeAlso "http://datex2.eu/schema/2/2_0#Convoy" .



###  http://purl.org/td/transportdisruption#ConvoyService

:ConvoyService rdf:type owl:Class ;
               
               rdfs:label "Convoy Service"^^xsd:string ;
               
               rdfs:subClassOf :GeneralNetworkManagement ;
               
               rdfs:comment "A convoy service is in operation. This concept and description are from the DATEX II concept convoyService."^^xsd:string ;
               
               rdfs:seeAlso "http://datex2.eu/schema/2/2_0#ConvoyService" .



###  http://purl.org/td/transportdisruption#CricketMatch

:CricketMatch rdf:type owl:Class ;
              
              rdfs:label "Cricket Match"^^xsd:string ;
              
              rdfs:subClassOf :PublicEvent ;
              
              rdfs:comment "Cricket match that could disrupt traffic. This concept and description are from the DATEX II concept cricketMatch."^^xsd:string ;
              
              rdfs:seeAlso "http://datex2.eu/schema/2/2_0#CricketMatch" .



###  http://purl.org/td/transportdisruption#Crosswinds

:Crosswinds rdf:type owl:Class ;
            
            rdfs:label "Crosswinds"^^xsd:string ;
            
            rdfs:subClassOf :EnvironmentalConditions ;
            
            rdfs:comment "Strong cross winds across the direction of a piece of transport infrastructure (e.g.. on a ridge or bridge). This concept and description are a generalised version of the DATEX II concept crosswinds."^^xsd:string ;
            
            rdfs:seeAlso "http://datex2.eu/schema/2/2_0#Crosswinds" .



###  http://purl.org/td/transportdisruption#Crowd

:Crowd rdf:type owl:Class ;
       
       rdfs:label "Crowd"^^xsd:string ;
       
       rdfs:subClassOf :DisturbanceActivity ;
       
       rdfs:comment "A major gathering of people that could disrupt traffic. This concept and description are from the DATEX II concept crowd."^^xsd:string ;
       
       rdfs:seeAlso "http://datex2.eu/schema/2/2_0#Crowd" .



###  http://purl.org/td/transportdisruption#CulturalEvent

:CulturalEvent rdf:type owl:Class ;
               
               rdfs:label "Cultural Event"^^xsd:string ;
               
               rdfs:subClassOf :PublicEvent ;
               
               rdfs:comment "Cultural event which could disrupt traffic. This concept and description are from the DATEX II concept culturalEvent."^^xsd:string ;
               
               rdfs:seeAlso "http://datex2.eu/schema/2/2_0#CulturalEvent" .



###  http://purl.org/td/transportdisruption#CustomsOperation

:CustomsOperation rdf:type owl:Class ;
                  
                  rdfs:label "Customs Operation"^^xsd:string ;
                  
                  rdfs:subClassOf :AuthorityOperation ;
                  
                  rdfs:comment "A permanent or temporary operation established by customs and excise authorities withi, on or adjacent to transport infrastructure. This concept and description are a generalised version of the DATEX II concept customsOperation."^^xsd:string ;
                  
                  rdfs:seeAlso "http://datex2.eu/schema/2/2_0#CustomsOperation" .



###  http://purl.org/td/transportdisruption#DamagedBridge

:DamagedBridge rdf:type owl:Class ;
               
               rdfs:label "Damaged Bridge"^^xsd:string ;
               
               rdfs:subClassOf :InfrastructureDamageObstruction ;
               
               rdfs:comment "Damage to a bridge that may cause traffic disruption. This concept and description are from the DATEX II concept damagedBridge."^^xsd:string ;
               
               rdfs:seeAlso "http://datex2.eu/schema/2/2_0#DamagedBridge" .



###  http://purl.org/td/transportdisruption#DamagedCrashBarrier

:DamagedCrashBarrier rdf:type owl:Class ;
                     
                     rdfs:label "Damaged Crash Barrier"^^xsd:string ;
                     
                     rdfs:subClassOf :InfrastructureDamageObstruction ;
                     
                     rdfs:comment "Damage to a crash barrier that may cause traffic disruption. This concept and description are from the DATEX II concept damagedCrashBarrier."^^xsd:string ;
                     
                     rdfs:seeAlso "http://datex2.eu/schema/2/2_0#DamagedCrashBarrier" .



###  http://purl.org/td/transportdisruption#DamagedFlyover

:DamagedFlyover rdf:type owl:Class ;
                
                rdfs:label "Damaged Flyover"^^xsd:string ;
                
                rdfs:subClassOf :InfrastructureDamageObstruction ;
                
                rdfs:comment "Damage to an elevated section of the carriageway over another carriageway that may cause traffic disruption. This concept and description are from the DATEX II concept damagedFlyover."^^xsd:string ;
                
                rdfs:seeAlso "http://datex2.eu/schema/2/2_0#DamagedFlyover" .



###  http://purl.org/td/transportdisruption#DamagedGallery

:DamagedGallery rdf:type owl:Class ;
                
                rdfs:label "Damaged Gallery"^^xsd:string ;
                
                rdfs:subClassOf :InfrastructureDamageObstruction ;
                
                rdfs:comment "Damage to a gallery that may cause traffic disruption. This concept and description are from the DATEX II concept damagedGallery."^^xsd:string ;
                
                rdfs:seeAlso "http://datex2.eu/schema/2/2_0#DamagedGallery" .



###  http://purl.org/td/transportdisruption#DamagedGantry

:DamagedGantry rdf:type owl:Class ;
               
               rdfs:label "Damaged Gantry"^^xsd:string ;
               
               rdfs:subClassOf :InfrastructureDamageObstruction ;
               
               rdfs:comment "Damage to a gantry above the infrastructure that may cause traffic disruption. This concept and description are a generalised version of the DATEX II concept damagedGantry."^^xsd:string ;
               
               rdfs:seeAlso "http://datex2.eu/schema/2/2_0#DamagedGantry" .



###  http://purl.org/td/transportdisruption#DamagedRoadSurface

:DamagedRoadSurface rdf:type owl:Class ;
                    
                    rdfs:label "Damaged Road Surface"^^xsd:string ;
                    
                    rdfs:subClassOf :InfrastructureDamageObstruction ;
                    
                    rdfs:comment "Damage to the road surface that may cause traffic disruption. This concept and description are from the DATEX II concept damagedRoadSurface."^^xsd:string ;
                    
                    rdfs:seeAlso "http://datex2.eu/schema/2/2_0#DamagedRoadSurface" .



###  http://purl.org/td/transportdisruption#DamagedTunnel

:DamagedTunnel rdf:type owl:Class ;
               
               rdfs:label "Damaged Tunnel"^^xsd:string ;
               
               rdfs:subClassOf :InfrastructureDamageObstruction ;
               
               rdfs:comment "Damage to a tunnel that may cause traffic disruption. This concept and description are from the DATEX II concept damagedTunnel."^^xsd:string ;
               
               rdfs:seeAlso "http://datex2.eu/schema/2/2_0#DamagedTunnel" .



###  http://purl.org/td/transportdisruption#DamagedVehicle

:DamagedVehicle rdf:type owl:Class ;
                
                rdfs:label "Damaged Vehicle"^^xsd:string ;
                
                rdfs:subClassOf :VehicleObstruction ;
                
                rdfs:comment "Damaged vehicle(s) which may cause traffic disruption. This concept and description are a generalised version of the DATEX II concept damagedVehicle."^^xsd:string ;
                
                rdfs:seeAlso "http://datex2.eu/schema/2/2_0#DamagedVehicle" .



###  http://purl.org/td/transportdisruption#DamagedViaduct

:DamagedViaduct rdf:type owl:Class ;
                
                rdfs:label "Damaged Viaduct"^^xsd:string ;
                
                rdfs:subClassOf :InfrastructureDamageObstruction ;
                
                rdfs:comment "Damage to a viaduct that may cause traffic disruption. This concept and description are from the DATEX II concept damagedViaduct."^^xsd:string ;
                
                rdfs:seeAlso "http://datex2.eu/schema/2/2_0#DamagedViaduct" .



###  http://purl.org/td/transportdisruption#DamagingHail

:DamagingHail rdf:type owl:Class ;
              
              rdfs:label "Damaging Hail"^^xsd:string ;
              
              rdfs:subClassOf :EnvironmentalConditions ;
              
              rdfs:comment "Large falling ice pellets or frozen rain capable of causing injury or damage to property. This concept and description are from the DATEX II concept damagingHail."^^xsd:string ;
              
              rdfs:seeAlso "http://datex2.eu/schema/2/2_0#DamagingHail" .



###  http://purl.org/td/transportdisruption#DangerousSlowMovingVehicle

:DangerousSlowMovingVehicle rdf:type owl:Class ;
                            
                            rdfs:label "Dangerous Slow Moving Vehicle"^^xsd:string ;
                            
                            rdfs:subClassOf :VehicleObstruction ;
                            
                            rdfs:comment "Dangerous slow moving vehicles which may cause traffic disruption. This concept and description are from the DATEX II concept dangerousSlowMovingVehicle."^^xsd:string ;
                            
                            rdfs:seeAlso "http://datex2.eu/schema/2/2_0#DangerousSlowMovingVehicle" .



###  http://purl.org/td/transportdisruption#DeepSnow

:DeepSnow rdf:type owl:Class ;
          
          rdfs:label "Deep Snow"^^xsd:string ;
          
          rdfs:subClassOf :WeatherRelatedConditions ;
          
          rdfs:comment "Deep snow on the transport infrastructure. This concept and description are a generalised version of the DATEX II concept deepSnow."^^xsd:string ;
          
          rdfs:seeAlso "http://datex2.eu/schema/2/2_0#DeepSnow" .



###  http://purl.org/td/transportdisruption#DemolitionWork

:DemolitionWork rdf:type owl:Class ;
                
                rdfs:label "Demolition Work"^^xsd:string ;
                
                rdfs:subClassOf :InfrastructureConstruction ;
                
                rdfs:comment "Demolition work associated with the construction work. This concept and description are from the DATEX II concept demolitionWork."^^xsd:string ;
                
                rdfs:seeAlso "http://datex2.eu/schema/2/2_0#DemolitionWork" .



###  http://purl.org/td/transportdisruption#Demonstration

:Demonstration rdf:type owl:Class ;
               
               rdfs:label "Demonstration"^^xsd:string ;
               
               rdfs:subClassOf :DisturbanceActivity ;
               
               rdfs:comment "A public protest with the potential to disrupt traffic. This concept and description are from the DATEX II concept demonstration."^^xsd:string ;
               
               rdfs:seeAlso "http://datex2.eu/schema/2/2_0#Demonstration" .



###  http://purl.org/td/transportdisruption#DenseFog

:DenseFog rdf:type owl:Class ;
          
          rdfs:label "Dense Fog"^^xsd:string ;
          
          rdfs:subClassOf :EnvironmentalConditions ;
          
          rdfs:comment "Dense fog, limiting visibility to 50m or less. This concept and description are from the DATEX II concept denseFog."^^xsd:string ;
          
          rdfs:seeAlso "http://datex2.eu/schema/2/2_0#DenseFog" .



###  http://purl.org/td/transportdisruption#Derailment

:Derailment rdf:type owl:Class ;
            
            rdfs:label "Derailment"^^xsd:string ;
            
            rdfs:subClassOf :VehicleOffInfrastructure ;
            
            rdfs:comment "Includes all accidents where one or more vehicles have left the rails of a track."^^xsd:string .



###  http://purl.org/td/transportdisruption#DieselOnInfrastructure

:DieselOnInfrastructure rdf:type owl:Class ;
                        
                        rdfs:label "Diesel On Infrastructure"^^xsd:string ;
                        
                        rdfs:subClassOf :AdverseInfrastructureConditions ;
                        
                        rdfs:comment "Diesel on transport infrastructure. This concept and description are a generalised version of the DATEX II concept dieselOnRoad."^^xsd:string ;
                        
                        rdfs:seeAlso "http://datex2.eu/schema/2/2_0#DieselOnRoad" .



###  http://purl.org/td/transportdisruption#DisruptiveEvent

:DisruptiveEvent rdf:type owl:Class ;
                 
                 rdfs:label "Disruptive Event"^^xsd:string ;
                 
                 rdfs:subClassOf <http://purl.org/NET/c4dm/event.owl#Event> ,
                                 [ rdf:type owl:Restriction ;
                                   owl:onProperty :causeOf ;
                                   owl:onClass :DisruptiveImpact ;
                                   owl:minQualifiedCardinality "1"^^xsd:nonNegativeInteger
                                 ] ;
                 
                 rdfs:comment "An event that has caused a disruptive impact.  This class is designed to allow events of any type to be typed as disruptive; as such, it is not hte intention that this class is extended further."^^xsd:string .



###  http://purl.org/td/transportdisruption#DisruptiveImpact

:DisruptiveImpact rdf:type owl:Class ;
                  
                  rdfs:label "Disruptive Impact"^^xsd:string ;
                  
                  rdfs:subClassOf [ rdf:type owl:Restriction ;
                                    owl:onProperty :relevantTo ;
                                    owl:onClass <http://xmlns.com/foaf/0.1/Agent> ;
                                    owl:minQualifiedCardinality "1"^^xsd:nonNegativeInteger
                                  ] ,
                                  [ rdf:type owl:Restriction ;
                                    owl:onProperty :impactsOn ;
                                    owl:onClass :Plan ;
                                    owl:minQualifiedCardinality "1"^^xsd:nonNegativeInteger
                                  ] ,
                                  [ rdf:type owl:Restriction ;
                                    owl:onProperty :hasCause ;
                                    owl:onClass <http://purl.org/NET/c4dm/event.owl#Event> ;
                                    owl:minQualifiedCardinality "1"^^xsd:nonNegativeInteger
                                  ] ;
                  
                  rdfs:comment "A disruptive impact the action of one or more events causing or tending to prevent an agent's planned travel from continuing as expected."^^xsd:string .



###  http://purl.org/td/transportdisruption#DisturbanceActivity

:DisturbanceActivity rdf:type owl:Class ;
                     
                     rdfs:label "Disturbance Activity"^^xsd:string ;
                     
                     rdfs:subClassOf :Activity ;
                     
                     rdfs:comment "Deliberate human action of either a public disorder nature or of a situation alert type which could disrupt traffic. This concept and description are from the DATEX II concept DisturbanceActivity."^^xsd:string ;
                     
                     rdfs:seeAlso "http://datex2.eu/schema/2/2_0#DisturbanceActivity" .



###  http://purl.org/td/transportdisruption#DrivingCondition

:DrivingCondition rdf:type owl:Class ;
                  
                  rdfs:label "Travel Conditions"^^xsd:string ;
                  
                  rdfs:subClassOf :Conditions ;
                  
                  rdfs:comment "Types of the perceived conditions affecting travel. This concept and description are from the DATEX II concept DrivingConditionTypeEnum."^^xsd:string ;
                  
                  rdfs:seeAlso "http://datex2.eu/schema/2/2_0#DrivingConditionTypeEnum" .



###  http://purl.org/td/transportdisruption#Dry

:Dry rdf:type owl:Class ;
     
     rdfs:label "Dry"^^xsd:string ;
     
     rdfs:subClassOf :WeatherRelatedConditions ;
     
     rdfs:comment "The infrastructure surface is dry. This concept and description are a generalised version of the DATEX II concept dry."^^xsd:string ;
     
     rdfs:seeAlso "http://datex2.eu/schema/2/2_0#Dry" .



###  http://purl.org/td/transportdisruption#EarthquakeDamage

:EarthquakeDamage rdf:type owl:Class ;
                  
                  rdfs:label "Earthquake Damage"^^xsd:string ;
                  
                  rdfs:subClassOf :EnvironmentalObstruction ;
                  
                  rdfs:comment "The transport infrastructure obstructed or partially obstructed because of damage caused by an earthquake. This concept and description are a generalised version of the DATEX II concept earthquakeDamage."^^xsd:string ;
                  
                  rdfs:seeAlso "http://datex2.eu/schema/2/2_0#EarthquakeDamage" .



###  http://purl.org/td/transportdisruption#Eclipse

:Eclipse rdf:type owl:Class ;
         
         rdfs:label "Eclipse"^^xsd:string ;
         
         rdfs:subClassOf :EnvironmentalConditions ;
         
         rdfs:comment "Eclipse, either partial or full, of the sun causing low light levels during normal daylight period. This concept and description are from the DATEX II concept eclipse."^^xsd:string ;
         
         rdfs:seeAlso "http://datex2.eu/schema/2/2_0#Eclipse" .



###  http://purl.org/td/transportdisruption#EmergencyRoadsideTelephoneFailure

:EmergencyRoadsideTelephoneFailure rdf:type owl:Class ;
                                   
                                   rdfs:label "Emergency Roadside Telephone Failure"^^xsd:string ;
                                   
                                   rdfs:subClassOf :InfrastructureFailure ;
                                   
                                   rdfs:comment "Failure of emergency roadside telephones. This concept and description are based on the DATEX II concept emergencyRoadsideTelephones."^^xsd:string ;
                                   
                                   rdfs:seeAlso "http://datex2.eu/schema/2/2_0#EmergencyRoadsideTelephones" .



###  http://purl.org/td/transportdisruption#EmergencyRoadsideTelephoneFault

:EmergencyRoadsideTelephoneFault rdf:type owl:Class ;
                                 
                                 rdfs:label "Emergency Roadside Telephone Fault"^^xsd:string ;
                                 
                                 rdfs:subClassOf :InfrastructureFault ;
                                 
                                 rdfs:comment "Faulty or malfunctioning emergency roadside telephones. This concept and description are based on the DATEX II concept emergencyRoadsideTelephones."^^xsd:string ;
                                 
                                 rdfs:seeAlso "http://datex2.eu/schema/2/2_0#EmergencyRoadsideTelephones" .



###  http://purl.org/td/transportdisruption#EmergencyServices

:EmergencyServices rdf:type owl:Class ;
                   
                   rdfs:label "Emergency Services"^^xsd:string ;
                   
                   rdfs:subClassOf :InfrastructureSideAssistance ;
                   
                   rdfs:comment "Emergency services assistance. This concept and description are from the DATEX II concept emergencyServices."^^xsd:string ;
                   
                   rdfs:seeAlso "http://datex2.eu/schema/2/2_0#EmergencyServices" .



###  http://purl.org/td/transportdisruption#EmergencyVehicle

:EmergencyVehicle rdf:type owl:Class ;
                  
                  rdfs:label "Emergency Vehicle"^^xsd:string ;
                  
                  rdfs:subClassOf :VehicleObstruction ;
                  
                  rdfs:comment "Emergency service vehicles on some transport infrastructure in response to an emergency situation. This concept and description are a generalised version of the DATEX II concept emergencyVehicle."^^xsd:string ;
                  
                  rdfs:seeAlso "http://datex2.eu/schema/2/2_0#EmergencyVehicle" .



###  http://purl.org/td/transportdisruption#EnvironmentalConditions

:EnvironmentalConditions rdf:type owl:Class ;
                         
                         rdfs:label "Environmental Conditions"^^xsd:string ;
                         
                         rdfs:subClassOf :Conditions ;
                         
                         rdfs:comment "Types of environmental conditions that may affect the transport network. This concept and description are based on the DATEX II concept PoorEnvironmentConditions"^^xsd:string ;
                         
                         rdfs:seeAlso "http://datex2.eu/schema/2/2_0#PoorEnvironmentTypeEnum" .



###  http://purl.org/td/transportdisruption#EnvironmentalObstruction

:EnvironmentalObstruction rdf:type owl:Class ;
                          
                          rdfs:label "Environmental Obstruction"^^xsd:string ;
                          
                          rdfs:subClassOf :Obstruction ;
                          
                          rdfs:comment "An obstruction on transport infrastructure resulting from an environmental cause. This concept and description are a generalised version of the DATEX II concept EnvironmentalObstruction."^^xsd:string ;
                          
                          rdfs:seeAlso "http://datex2.eu/schema/2/2_0#EnvironmentalObstruction" .



###  http://purl.org/td/transportdisruption#Evacuation

:Evacuation rdf:type owl:Class ;
            
            rdfs:label "Evacuation"^^xsd:string ;
            
            rdfs:subClassOf :DisturbanceActivity ;
            
            rdfs:comment "A situation where a definite area is being cleared due to dangerous conditions or for security reasons. This concept and description are from the DATEX II concept evacuation."^^xsd:string ;
            
            rdfs:seeAlso "http://datex2.eu/schema/2/2_0#Evacuation" .



###  http://purl.org/td/transportdisruption#Exhibition

:Exhibition rdf:type owl:Class ;
            
            rdfs:label "Exhibition"^^xsd:string ;
            
            rdfs:subClassOf :PublicEvent ;
            
            rdfs:comment "Major display or trade show which could disrupt traffic. This concept and description are from the DATEX II concept exhibition."^^xsd:string ;
            
            rdfs:seeAlso "http://datex2.eu/schema/2/2_0#Exhibition" .



###  http://purl.org/td/transportdisruption#ExtremeCold

:ExtremeCold rdf:type owl:Class ;
             
             rdfs:label "Extreme Cold"^^xsd:string ;
             
             rdfs:subClassOf :EnvironmentalConditions ;
             
             rdfs:comment "Abnormally low temperatures. This concept and description are from the DATEX II concept extremeCold."^^xsd:string ;
             
             rdfs:seeAlso "http://datex2.eu/schema/2/2_0#ExtremeCold" .



###  http://purl.org/td/transportdisruption#ExtremeHeat

:ExtremeHeat rdf:type owl:Class ;
             
             rdfs:label "Extreme Heat"^^xsd:string ;
             
             rdfs:subClassOf :EnvironmentalConditions ;
             
             rdfs:comment "Abnormally high expected maximum temperature. This concept and description are from the DATEX II concept extremeHeat."^^xsd:string ;
             
             rdfs:seeAlso "http://datex2.eu/schema/2/2_0#ExtremeHeat" .



###  http://purl.org/td/transportdisruption#Fair

:Fair rdf:type owl:Class ;
      
      rdfs:label "Fair"^^xsd:string ;
      
      rdfs:subClassOf :PublicEvent ;
      
      rdfs:comment "Periodic (e.g. annual), often traditional, gathering for entertainment or trade promotion, which could disrupt traffic. This concept and description are from the DATEX II concept fair."^^xsd:string ;
      
      rdfs:seeAlso "http://datex2.eu/schema/2/2_0#Fair" .



###  http://purl.org/td/transportdisruption#FallenPowerCables

:FallenPowerCables rdf:type owl:Class ;
                   
                   rdfs:label "Fallen Power Cables"^^xsd:string ;
                   
                   rdfs:subClassOf :InfrastructureDamageObstruction ;
                   
                   rdfs:comment "Transport infrastructure is obstructed or partially obstructed by one or more fallen power cables. This concept and description are a generalised version of the DATEX II concept fallenPowerCables."^^xsd:string ;
                   
                   rdfs:seeAlso "http://datex2.eu/schema/2/2_0#FallenPowerCables" .



###  http://purl.org/td/transportdisruption#FallenTrees

:FallenTrees rdf:type owl:Class ;
             
             rdfs:label "Fallen Trees"^^xsd:string ;
             
             rdfs:subClassOf :EnvironmentalObstruction ;
             
             rdfs:comment "The transport infrastructure is obstructed or partially obstructed by one or more fallen trees. This concept and description are a generalised version of the DATEX II concept fallenTrees."^^xsd:string ;
             
             rdfs:seeAlso "http://datex2.eu/schema/2/2_0#FallenTrees" .



###  http://purl.org/td/transportdisruption#FallingIce

:FallingIce rdf:type owl:Class ;
            
            rdfs:label "Falling Ice"^^xsd:string ;
            
            rdfs:subClassOf :EnvironmentalObstruction ;
            
            rdfs:comment "Falling ice off trees, power lines or structures which may cause traffic disruption. This concept and description are from the DATEX II concept fallingIce."^^xsd:string ;
            
            rdfs:seeAlso "http://datex2.eu/schema/2/2_0#FallingIce" .



###  http://purl.org/td/transportdisruption#FallingLightIceOrSnow

:FallingLightIceOrSnow rdf:type owl:Class ;
                       
                       rdfs:label "Falling Light Ice Or Snow"^^xsd:string ;
                       
                       rdfs:subClassOf :EnvironmentalObstruction ;
                       
                       rdfs:comment "Falling light ice or snow off trees, power lines or structures which may cause traffic disruption. This concept and description are from the DATEX II concept fallingLightIceOrSnow."^^xsd:string ;
                       
                       rdfs:seeAlso "http://datex2.eu/schema/2/2_0#FallingLightIceOrSnow" .



###  http://purl.org/td/transportdisruption#Festival

:Festival rdf:type owl:Class ;
          
          rdfs:label "Festival"^^xsd:string ;
          
          rdfs:subClassOf :PublicEvent ;
          
          rdfs:comment "Celebratory event or series of events which could disrupt traffic. This concept and description are from the DATEX II concept festival."^^xsd:string ;
          
          rdfs:seeAlso "http://datex2.eu/schema/2/2_0#Festival" .



###  http://purl.org/td/transportdisruption#FilmTVMaking

:FilmTVMaking rdf:type owl:Class ;
              
              rdfs:label "Film TV Making"^^xsd:string ;
              
              rdfs:subClassOf :PublicEvent ;
              
              rdfs:comment "Film or TV making event which could disrupt traffic. This concept and description are from the DATEX II concept filmTVMaking."^^xsd:string ;
              
              rdfs:seeAlso "http://datex2.eu/schema/2/2_0#FilmTVMaking" .



###  http://purl.org/td/transportdisruption#FilterBlockade

:FilterBlockade rdf:type owl:Class ;
                
                rdfs:label "Filter Blockade"^^xsd:string ;
                
                rdfs:subClassOf :DisturbanceActivity ;
                
                rdfs:comment "A manned blockade of some transport infrasturcture where only certain vehicles are allowed through. This concept and description are a generalised version of the DATEX II concept filterBlockade."^^xsd:string ;
                
                rdfs:seeAlso "http://datex2.eu/schema/2/2_0#FilterBlockade" .



###  http://purl.org/td/transportdisruption#FirstAid

:FirstAid rdf:type owl:Class ;
          
          rdfs:label "First Aid"^^xsd:string ;
          
          rdfs:subClassOf :InfrastructureSideAssistance ;
          
          rdfs:comment "First aid assistance. This concept and description are from the DATEX II concept firstAid."^^xsd:string ;
          
          rdfs:seeAlso "http://datex2.eu/schema/2/2_0#FirstAid" .



###  http://purl.org/td/transportdisruption#FlashFloods

:FlashFloods rdf:type owl:Class ;
             
             rdfs:label "Flash Floods"^^xsd:string ;
             
             rdfs:subClassOf :EnvironmentalObstruction ;
             
             rdfs:comment "The transport infrastructure being quickly inundated by powerful floodwaters due to heavy rain nearby. This concept and description are a generalised version of the DATEX II concept flashFloods."^^xsd:string ;
             
             rdfs:seeAlso "http://datex2.eu/schema/2/2_0#FlashFloods" .



###  http://purl.org/td/transportdisruption#Flooding

:Flooding rdf:type owl:Class ;
          
          rdfs:label "Flooding"^^xsd:string ;
          
          rdfs:subClassOf :EnvironmentalObstruction ;
          
          rdfs:comment "The transport infrastructure is obstructed or partially obstructed by flood water. This concept and description are a generalised version of the DATEX II concept flooding."^^xsd:string ;
          
          rdfs:seeAlso "http://datex2.eu/schema/2/2_0#Flooding" .



###  http://purl.org/td/transportdisruption#Fog

:Fog rdf:type owl:Class ;
     
     rdfs:label "Fog"^^xsd:string ;
     
     rdfs:subClassOf :EnvironmentalConditions ;
     
     rdfs:comment "Fog, visibility more than 50m. This concept and description are from the DATEX II concept fog."^^xsd:string ;
     
     rdfs:seeAlso "http://datex2.eu/schema/2/2_0#Fog" .



###  http://purl.org/td/transportdisruption#FoodDelivery

:FoodDelivery rdf:type owl:Class ;
              
              rdfs:label "Food Delivery"^^xsd:string ;
              
              rdfs:subClassOf :InfrastructureSideAssistance ;
              
              rdfs:comment "Food delivery. This concept and description are from the DATEX II concept foodDelivery."^^xsd:string ;
              
              rdfs:seeAlso "http://datex2.eu/schema/2/2_0#FoodDelivery" .



###  http://purl.org/td/transportdisruption#FootballMatch

:FootballMatch rdf:type owl:Class ;
               
               rdfs:label "Football Match"^^xsd:string ;
               
               rdfs:subClassOf :PublicEvent ;
               
               rdfs:comment "Football match that could disrupt traffic. This concept and description are from the DATEX II concept footballMatch."^^xsd:string ;
               
               rdfs:seeAlso "http://datex2.eu/schema/2/2_0#FootballMatch" .



###  http://purl.org/td/transportdisruption#ForestFire

:ForestFire rdf:type owl:Class ;
            
            rdfs:label "Forest Fire"^^xsd:string ;
            
            rdfs:subClassOf :EnvironmentalObstruction ;
            
            rdfs:comment "Traffic may be disrupted due to a forest fire adjacent to some transport infrastructure. This concept and description are a generalised version of the DATEX II concept forestFire."^^xsd:string ;
            
            rdfs:seeAlso "http://datex2.eu/schema/2/2_0#ForestFire" .



###  http://purl.org/td/transportdisruption#FreezingFog

:FreezingFog rdf:type owl:Class ;
             
             rdfs:label "Freezing Fog"^^xsd:string ;
             
             rdfs:subClassOf :EnvironmentalConditions ;
             
             rdfs:comment "Fog, in conjunction with sub-zero air temperatures causing possible freezing of infrastructure such as road surface. This concept and description are a generalised version of the DATEX II concept freezingFog."^^xsd:string ;
             
             rdfs:seeAlso "http://datex2.eu/schema/2/2_0#FreezingFog" .



###  http://purl.org/td/transportdisruption#FreezingOfWetInfrastructureSurface

:FreezingOfWetInfrastructureSurface rdf:type owl:Class ;
                                    
                                    rdfs:label "Freezing Of Wet Infrastructure Surface"^^xsd:string ;
                                    
                                    rdfs:subClassOf :WeatherRelatedConditions ;
                                    
                                    rdfs:comment "The wet infrastructure surface is subject to freezing. This concept and description are a generalised version of the DATEX II concept freezingOfWetRoads."^^xsd:string ;
                                    
                                    rdfs:seeAlso "http://datex2.eu/schema/2/2_0#FreezingOfWetRoads" .



###  http://purl.org/td/transportdisruption#FreezingPavements

:FreezingPavements rdf:type owl:Class ;
                   
                   rdfs:label "Freezing Pavements"^^xsd:string ;
                   
                   rdfs:subClassOf :WeatherRelatedConditions ;
                   
                   rdfs:comment "The pavements for pedestrians are subject to freezing. This concept and description are from the DATEX II concept freezingPavements."^^xsd:string ;
                   
                   rdfs:seeAlso "http://datex2.eu/schema/2/2_0#FreezingPavements" .



###  http://purl.org/td/transportdisruption#FreezingRain

:FreezingRain rdf:type owl:Class ;
              
              rdfs:label "Freezing Rain"^^xsd:string ;
              
              rdfs:subClassOf :WeatherRelatedConditions ;
              
              rdfs:comment "Falling rain on sub-zero temperature infrastructure surfaces freezing. This concept and description are a generalised version of the DATEX II concept freezingRain."^^xsd:string ;
              
              rdfs:seeAlso "http://datex2.eu/schema/2/2_0#FreezingRain" .



###  http://purl.org/td/transportdisruption#FreshSnow

:FreshSnow rdf:type owl:Class ;
           
           rdfs:label "Fresh Snow"^^xsd:string ;
           
           rdfs:subClassOf :WeatherRelatedConditions ;
           
           rdfs:comment "Fresh snow on the infrastructure. This concept and description are a generalised version of the DATEX II concept freshSnow."^^xsd:string ;
           
           rdfs:seeAlso "http://datex2.eu/schema/2/2_0#FreshSnow" .



###  http://purl.org/td/transportdisruption#Frost

:Frost rdf:type owl:Class ;
       
       rdfs:label "Frost"^^xsd:string ;
       
       rdfs:subClassOf :EnvironmentalConditions ;
       
       rdfs:comment "Frost. This concept and description are adaptations of the DATEX II concept frost."^^xsd:string ;
       
       rdfs:seeAlso "http://datex2.eu/schema/2/2_0#Frost" .



###  http://purl.org/td/transportdisruption#FuelSpillageAccident

:FuelSpillageAccident rdf:type owl:Class ;
                      
                      rdfs:label "Fuel Spillage Accident"^^xsd:string ;
                      
                      rdfs:subClassOf :SpillageAccident ;
                      
                      rdfs:comment "Includes all situations resulting in a spillage of fuel. This concept and description are a generalised version of the DATEX II concept fuelSpillageAccident."^^xsd:string ;
                      
                      rdfs:seeAlso "http://datex2.eu/schema/2/2_0#FuelSpillageAccident" .



###  http://purl.org/td/transportdisruption#Funfair

:Funfair rdf:type owl:Class ;
         
         rdfs:label "Funfair"^^xsd:string ;
         
         rdfs:subClassOf :PublicEvent ;
         
         rdfs:comment "Periodic (e.g. annual), often traditional, gathering for entertainment, which could disrupt traffic. This concept and description are from the DATEX II concept funfair."^^xsd:string ;
         
         rdfs:seeAlso "http://datex2.eu/schema/2/2_0#Funfair" .



###  http://purl.org/td/transportdisruption#Gales

:Gales rdf:type owl:Class ;
       
       rdfs:label "Gales"^^xsd:string ;
       
       rdfs:subClassOf :EnvironmentalConditions ;
       
       rdfs:comment "Winds between 60 km/h and 90 km/h. This concept and description are from the DATEX II concept gales."^^xsd:string ;
       
       rdfs:seeAlso "http://datex2.eu/schema/2/2_0#Gales" .



###  http://purl.org/td/transportdisruption#GalleryLightsFailure

:GalleryLightsFailure rdf:type owl:Class ;
                      
                      rdfs:label "Gallery Lights Failure"^^xsd:string ;
                      
                      rdfs:subClassOf :InfrastructureFailure ;
                      
                      rdfs:comment "Failure of gallery lights. This concept and description are based on the DATEX II concept galleryLights."^^xsd:string ;
                      
                      rdfs:seeAlso "http://datex2.eu/schema/2/2_0#GalleryLights" .



###  http://purl.org/td/transportdisruption#GalleryLightsFault

:GalleryLightsFault rdf:type owl:Class ;
                    
                    rdfs:label "Gallery Lights Fault"^^xsd:string ;
                    
                    rdfs:subClassOf :InfrastructureFault ;
                    
                    rdfs:comment "Faulty or malfunctioning gallery lights. This concept and description are based on the DATEX II concept galleryLights."^^xsd:string ;
                    
                    rdfs:seeAlso "http://datex2.eu/schema/2/2_0#GalleryLights" .



###  http://purl.org/td/transportdisruption#GardeningOrFlowerShow

:GardeningOrFlowerShow rdf:type owl:Class ;
                       
                       rdfs:label "Gardening Or Flower Show"^^xsd:string ;
                       
                       rdfs:subClassOf :PublicEvent ;
                       
                       rdfs:comment "Gardening and/or flower show or event which could disrupt traffic. This concept and description are from the DATEX II concept gardeningOrFlowerShow."^^xsd:string ;
                       
                       rdfs:seeAlso "http://datex2.eu/schema/2/2_0#GardeningOrFlowerShow" .



###  http://purl.org/td/transportdisruption#GasLeak

:GasLeak rdf:type owl:Class ;
         
         rdfs:label "Gas Leak"^^xsd:string ;
         
         rdfs:subClassOf :InfrastructureDamageObstruction ;
         
         rdfs:comment "Traffic may be disrupted due to an explosion hazard from gas escaping in or near transport infrastructure. This concept and description are a generalised version of the DATEX II concept gasLeak."^^xsd:string ;
         
         rdfs:seeAlso "http://datex2.eu/schema/2/2_0#GasLeak" .



###  http://purl.org/td/transportdisruption#GeneralNetworkManagement

:GeneralNetworkManagement rdf:type owl:Class ;
                          
                          rdfs:label "General Network Management"^^xsd:string ;
                          
                          rdfs:subClassOf :NetworkManagement ;
                          
                          rdfs:comment "Network management action that is instigated either manually or automatically by the network operator.  Compliance with any resulting control may be advisory or mandatory. This concept and description are a generalised version the DATEX II concept GeneralNetworkManagement."^^xsd:string ;
                          
                          rdfs:seeAlso "http://datex2.eu/schema/2/2_0#GeneralNetworkManagement" .



###  http://purl.org/td/transportdisruption#GeneralObstruction

:GeneralObstruction rdf:type owl:Class ;
                    
                    rdfs:label "General Obstruction"^^xsd:string ;
                    
                    rdfs:subClassOf :Obstruction ;
                    
                    rdfs:comment "Any stationary or moving obstacle of a physical nature, other than of an animal, vehicle, environmental, or damaged equipment nature. This concept and description are from the DATEX II concept GeneralObstruction."^^xsd:string ;
                    
                    rdfs:seeAlso "http://datex2.eu/schema/2/2_0#GeneralObstruction" .



###  http://purl.org/td/transportdisruption#GoSlowOperation

:GoSlowOperation rdf:type owl:Class ;
                 
                 rdfs:label "Go Slow Operation"^^xsd:string ;
                 
                 rdfs:subClassOf :DisturbanceActivity ;
                 
                 rdfs:comment "As a form of protest, several vehicles are driving in a convoy at a low speed which is affecting the normal traffic flow. This concept and description are from the DATEX II concept goSlowOperation."^^xsd:string ;
                 
                 rdfs:seeAlso "http://datex2.eu/schema/2/2_0#GoSlowOperation" .



###  http://purl.org/td/transportdisruption#GolfTournament

:GolfTournament rdf:type owl:Class ;
                
                rdfs:label "Golf Tournament"^^xsd:string ;
                
                rdfs:subClassOf :PublicEvent ;
                
                rdfs:comment "Golf tournament event that could disrupt traffic. This concept and description are from the DATEX II concept golfTournament."^^xsd:string ;
                
                rdfs:seeAlso "http://datex2.eu/schema/2/2_0#GolfTournament" .



###  http://purl.org/td/transportdisruption#GrassCuttingWork

:GrassCuttingWork rdf:type owl:Class ;
                  
                  rdfs:label "Grass Cutting Work"^^xsd:string ;
                  
                  rdfs:subClassOf :InfrastructureMaintenance ;
                  
                  rdfs:comment "Grass cutting work. This concept and description are from the DATEX II concept grassCuttingWork."^^xsd:string ;
                  
                  rdfs:seeAlso "http://datex2.eu/schema/2/2_0#GrassCuttingWork" .



###  http://purl.org/td/transportdisruption#GrassFire

:GrassFire rdf:type owl:Class ;
           
           rdfs:label "Grass Fire"^^xsd:string ;
           
           rdfs:subClassOf :EnvironmentalObstruction ;
           
           rdfs:comment "Traffic may be disrupted due to a grass fire adjacent to some transport infrastructure. This concept and description are a generalised version of the DATEX II concept grassFire."^^xsd:string ;
           
           rdfs:seeAlso "http://datex2.eu/schema/2/2_0#GrassFire" .



###  http://purl.org/td/transportdisruption#GunfireOnRoadway

:GunfireOnRoadway rdf:type owl:Class ;
                  
                  rdfs:label "Gunfire On Roadway"^^xsd:string ;
                  
                  rdfs:subClassOf :DisturbanceActivity ;
                  
                  rdfs:comment "A situation involving gunfire, perceived or actual, on or near some transport infrastructure through an act of terrorism or crime, which could disrupt traffic. This concept and description are a generalised version of the DATEX II concept gunfireOnRoadway."^^xsd:string ;
                  
                  rdfs:seeAlso "http://datex2.eu/schema/2/2_0#GunfireOnRoadway" .



###  http://purl.org/td/transportdisruption#GustyWinds

:GustyWinds rdf:type owl:Class ;
            
            rdfs:label "Gusty Winds"^^xsd:string ;
            
            rdfs:subClassOf :EnvironmentalConditions ;
            
            rdfs:comment "Constantly varying winds, significant at times. This concept and description are from the DATEX II concept gustyWinds."^^xsd:string ;
            
            rdfs:seeAlso "http://datex2.eu/schema/2/2_0#GustyWinds" .



###  http://purl.org/td/transportdisruption#Hail

:Hail rdf:type owl:Class ;
      
      rdfs:label "Hail"^^xsd:string ;
      
      rdfs:subClassOf :EnvironmentalConditions ;
      
      rdfs:comment "Falling ice pellets or frozen rain. This concept and description are from the DATEX II concept hail."^^xsd:string ;
      
      rdfs:seeAlso "http://datex2.eu/schema/2/2_0#Hail" .



###  http://purl.org/td/transportdisruption#HardShoulderRunningInOperation

:HardShoulderRunningInOperation rdf:type owl:Class ;
                                
                                rdfs:label "Hard Shoulder Running In Operation"^^xsd:string ;
                                
                                rdfs:subClassOf :RoadOrCarriagewayOrLaneManagement ;
                                
                                rdfs:comment "The hard shoulder is open as an operational lane. This concept and description are from the DATEX II concept hardShoulderRunningInOperation."^^xsd:string ;
                                
                                rdfs:seeAlso "http://datex2.eu/schema/2/2_0#HardShoulderRunningInOperation" .



###  http://purl.org/td/transportdisruption#Hazardous

:Hazardous rdf:type owl:Class ;
           
           rdfs:label "Hazardous"^^xsd:string ;
           
           rdfs:subClassOf :DrivingCondition ;
           
           rdfs:comment "Driving conditions are hazardous due to environmental conditions. This concept and description are from the DATEX II concept hazardous."^^xsd:string ;
           
           rdfs:seeAlso "http://datex2.eu/schema/2/2_0#Hazardous" .



###  http://purl.org/td/transportdisruption#HeadOnCollision

:HeadOnCollision rdf:type owl:Class ;
                 
                 rdfs:label "Head On Collision"^^xsd:string ;
                 
                 rdfs:subClassOf :Collision ;
                 
                 rdfs:comment "Collision of vehicle with another vehicle head on. This concept and description are from the DATEX II concept headOnCollision."^^xsd:string ;
                 
                 rdfs:seeAlso "http://datex2.eu/schema/2/2_0#HeadOnCollision" .



###  http://purl.org/td/transportdisruption#HeadOnOrSideCollision

:HeadOnOrSideCollision rdf:type owl:Class ;
                       
                       rdfs:label "Head On Or Side Collision"^^xsd:string ;
                       
                       rdfs:subClassOf :Collision ;
                       
                       rdfs:comment "Collision of vehicle with another vehicle either head on or sideways. This concept and description are from the DATEX II concept headOnOrSideCollision."^^xsd:string ;
                       
                       rdfs:seeAlso "http://datex2.eu/schema/2/2_0#HeadOnOrSideCollision" .



###  http://purl.org/td/transportdisruption#HeavyFrost

:HeavyFrost rdf:type owl:Class ;
            
            rdfs:label "Heavy Frost"^^xsd:string ;
            
            rdfs:subClassOf :EnvironmentalConditions ;
            
            rdfs:comment "A thick coating of frost. This concept and description are adaptations of the DATEX II concept heavyFrost."^^xsd:string ;
            
            rdfs:seeAlso "http://datex2.eu/schema/2/2_0#HeavyFrost" .



###  http://purl.org/td/transportdisruption#HeavyRain

:HeavyRain rdf:type owl:Class ;
           
           rdfs:label "Heavy Rain"^^xsd:string ;
           
           rdfs:subClassOf :EnvironmentalConditions ;
           
           rdfs:comment "Heavy rainfall, limiting visibility to 50m or less. This concept and description are from the DATEX II concept heavyRain."^^xsd:string ;
           
           rdfs:seeAlso "http://datex2.eu/schema/2/2_0#HeavyRain" .



###  http://purl.org/td/transportdisruption#HeavySnowfall

:HeavySnowfall rdf:type owl:Class ;
               
               rdfs:label "Heavy Snowfall"^^xsd:string ;
               
               rdfs:subClassOf :EnvironmentalConditions ;
               
               rdfs:comment "Dense falling snow, limiting visibility to 50m or less. This concept and description are from the DATEX II concept heavySnowfall."^^xsd:string ;
               
               rdfs:seeAlso "http://datex2.eu/schema/2/2_0#HeavySnowfall" .



###  http://purl.org/td/transportdisruption#HeavyTraffic

:HeavyTraffic rdf:type owl:Class ;
              
              rdfs:label "Heavy Traffic"^^xsd:string ;
              
              rdfs:subClassOf :AbnormalTraffic ;
              
              rdfs:comment "Traffic is heavy at the specified location. For road traffic, DATEX II defines this as the average speed is between 75% and 90% of its free-flow level.  This concept and description are adaptations of the DATEX II concept heavyTraffic."^^xsd:string ;
              
              rdfs:seeAlso "http://datex2.eu/schema/2/2_0#HeavyTraffic" .



###  http://purl.org/td/transportdisruption#HeightRestrictionInOperation

:HeightRestrictionInOperation rdf:type owl:Class ;
                              
                              rdfs:label "Height Restriction In Operation"^^xsd:string ;
                              
                              rdfs:subClassOf :RoadOrCarriagewayOrLaneManagement ;
                              
                              rdfs:comment "A height restriction is in operation. This concept and description are from the DATEX II concept heightRestrictionInOperation."^^xsd:string ;
                              
                              rdfs:seeAlso "http://datex2.eu/schema/2/2_0#HeightRestrictionInOperation" .



###  http://purl.org/td/transportdisruption#HelicopterRescue

:HelicopterRescue rdf:type owl:Class ;
                  
                  rdfs:label "Helicopter Rescue"^^xsd:string ;
                  
                  rdfs:subClassOf :InfrastructureSideAssistance ;
                  
                  rdfs:comment "Helicopter rescue. This concept and description are from the DATEX II concept helicopterRescue."^^xsd:string ;
                  
                  rdfs:seeAlso "http://datex2.eu/schema/2/2_0#HelicopterRescue" .



###  http://purl.org/td/transportdisruption#HerdOfAnimalsOnTheInfrastructure

:HerdOfAnimalsOnTheInfrastructure rdf:type owl:Class ;
                                  
                                  rdfs:label "Herd Of Animals On The Infrastructure"^^xsd:string ;
                                  
                                  rdfs:subClassOf :AnimalPresenceObstruction ;
                                  
                                  rdfs:comment "Traffic may be disrupted due to a herd of animals on transport infrastructure. This concept and description a generalised version of the DATEX II concept herdOfAnimalsOnTheRoad."^^xsd:string ;
                                  
                                  rdfs:seeAlso "http://datex2.eu/schema/2/2_0#HerdOfAnimalsOnTheRoad" .



###  http://purl.org/td/transportdisruption#HighSpeedEmergencyVehicle

:HighSpeedEmergencyVehicle rdf:type owl:Class ;
                           
                           rdfs:label "High Speed Emergency Vehicle"^^xsd:string ;
                           
                           rdfs:subClassOf :VehicleObstruction ;
                           
                           rdfs:comment "Emergency service vehicles progressing at high speed along the roadway in response to or en route from an emergency situation. This concept and description are from the DATEX II concept highSpeedEmergencyVehicle."^^xsd:string ;
                           
                           rdfs:seeAlso "http://datex2.eu/schema/2/2_0#HighSpeedEmergencyVehicle" .



###  http://purl.org/td/transportdisruption#HockeyGame

:HockeyGame rdf:type owl:Class ;
            
            rdfs:label "Hockey Game"^^xsd:string ;
            
            rdfs:subClassOf :PublicEvent ;
            
            rdfs:comment "Hockey game event that could disrupt traffic. This concept and description are from the DATEX II concept hockeyGame."^^xsd:string ;
            
            rdfs:seeAlso "http://datex2.eu/schema/2/2_0#HockeyGame" .



###  http://purl.org/td/transportdisruption#HorseRaceMeeting

:HorseRaceMeeting rdf:type owl:Class ;
                  
                  rdfs:label "Horse Race Meeting"^^xsd:string ;
                  
                  rdfs:subClassOf :PublicEvent ;
                  
                  rdfs:comment "Horse race meeting that could disrupt traffic. This concept and description are from the DATEX II concept horseRaceMeeting."^^xsd:string ;
                  
                  rdfs:seeAlso "http://datex2.eu/schema/2/2_0#HorseRaceMeeting" .



###  http://purl.org/td/transportdisruption#HurricaneForceWinds

:HurricaneForceWinds rdf:type owl:Class ;
                     
                     rdfs:label "Hurricane Force Winds"^^xsd:string ;
                     
                     rdfs:subClassOf :EnvironmentalConditions ;
                     
                     rdfs:comment "Winds over 120 km/h. This concept and description are from the DATEX II concept hurricaneForceWinds."^^xsd:string ;
                     
                     rdfs:seeAlso "http://datex2.eu/schema/2/2_0#HurricaneForceWinds" .



###  http://purl.org/td/transportdisruption#Ice

:Ice rdf:type owl:Class ;
     
     rdfs:label "Ice"^^xsd:string ;
     
     rdfs:subClassOf :WeatherRelatedConditions ;
     
     rdfs:comment "Presence of ice (of any kind) on transport infrastructure. This concept and description are a generalised version of the DATEX II concept ice."^^xsd:string ;
     
     rdfs:seeAlso "http://datex2.eu/schema/2/2_0#Ice" .



###  http://purl.org/td/transportdisruption#IceBuildUp

:IceBuildUp rdf:type owl:Class ;
            
            rdfs:label "Ice Build Up"^^xsd:string ;
            
            rdfs:subClassOf :WeatherRelatedConditions ;
            
            rdfs:comment "Ice is building up on the infrastructure surface. This concept and description are a generalised version of the DATEX II concept iceBuildUp."^^xsd:string ;
            
            rdfs:seeAlso "http://datex2.eu/schema/2/2_0#IceBuildUp" .



###  http://purl.org/td/transportdisruption#IceWithWheelBarTracks

:IceWithWheelBarTracks rdf:type owl:Class ;
                       
                       rdfs:label "Ice With Wheel Bar Tracks"^^xsd:string ;
                       
                       rdfs:subClassOf :WeatherRelatedConditions ;
                       
                       rdfs:comment "Ice on the road frozen in the form of wheel tracks. This concept and description are from the DATEX II concept iceWithWheelBarTracks."^^xsd:string ;
                       
                       rdfs:seeAlso "http://datex2.eu/schema/2/2_0#IceWithWheelBarTracks" .



###  http://purl.org/td/transportdisruption#IcyPatches

:IcyPatches rdf:type owl:Class ;
            
            rdfs:label "Icy Patches"^^xsd:string ;
            
            rdfs:subClassOf :WeatherRelatedConditions ;
            
            rdfs:comment "Icy patches (i.e. intermittent ice on the surface of transport infrastructure). This concept and description are a generalised version of the DATEX II concept icyPatches."^^xsd:string ;
            
            rdfs:seeAlso "http://datex2.eu/schema/2/2_0#IcyPatches" .



###  http://purl.org/td/transportdisruption#IllVehicleOccupants

:IllVehicleOccupants rdf:type owl:Class ;
                     
                     rdfs:label "Ill Vehicle Occupants"^^xsd:string ;
                     
                     rdfs:subClassOf :DisturbanceActivity ;
                     
                     rdfs:comment "One or more occupants of a vehicle are seriously ill, possibly requiring specialist services or assistance. This may disrupt normal traffic flow. This concept and description are from the DATEX II concept illVehicleOccupants."^^xsd:string ;
                     
                     rdfs:seeAlso "http://datex2.eu/schema/2/2_0#IllVehicleOccupants" .



###  http://purl.org/td/transportdisruption#Impossible

:Impossible rdf:type owl:Class ;
            
            rdfs:label "Impossible"^^xsd:string ;
            
            rdfs:subClassOf :DrivingCondition ;
            
            rdfs:comment "Current conditions are making driving impossible. This concept and description are from the DATEX II concept impossible."^^xsd:string ;
            
            rdfs:seeAlso "http://datex2.eu/schema/2/2_0#Impossible" .



###  http://purl.org/td/transportdisruption#InfrastructureConstruction

:InfrastructureConstruction rdf:type owl:Class ;
                            
                            rdfs:label "Infrastructure Construction"^^xsd:string ;
                            
                            rdfs:subClassOf :InfrastructureWorks ;
                            
                            rdfs:comment "Work involving the construction of new infrastructure. This concept and description are from the DATEX II concept ConstructionWorks."^^xsd:string ;
                            
                            rdfs:seeAlso "http://datex2.eu/schema/2/2_0#ConstructionWorks" .



###  http://purl.org/td/transportdisruption#InfrastructureDamageObstruction

:InfrastructureDamageObstruction rdf:type owl:Class ;
                                 
                                 rdfs:label "Infrastructure Damage Obstruction"^^xsd:string ;
                                 
                                 rdfs:subClassOf :Obstruction ;
                                 
                                 rdfs:comment "An obstruction on some transport infrastructure resulting from the failure or damage of infrastructure on, under, above or nearby. This concept and description are a generalised version of the DATEX II concept InfrastructureDamageObstruction."^^xsd:string ;
                                 
                                 rdfs:seeAlso "http://datex2.eu/schema/2/2_0#InfrastructureDamageObstruction" .



###  http://purl.org/td/transportdisruption#InfrastructureFailure

:InfrastructureFailure rdf:type owl:Class ;
                       
                       rdfs:label "Infrastructure Failure"^^xsd:string ;
                       
                       rdfs:subClassOf :TrafficElementEvent ;
                       
                       rdfs:comment "Infrastructure, equipment or system which is not in an operational state. This concept and description are based on the DATEX II concept EquipmentOrSystemFault."^^xsd:string ;
                       
                       rdfs:seeAlso "http://datex2.eu/schema/2/2_0#EquipmentOrSystemFault" .



###  http://purl.org/td/transportdisruption#InfrastructureFault

:InfrastructureFault rdf:type owl:Class ;
                     
                     rdfs:label "Infrastructure Fault"^^xsd:string ;
                     
                     rdfs:subClassOf :TrafficElementEvent ;
                     
                     rdfs:comment "Infrastructure, equipment or system which is faulty, malfunctioning or not in a fully operational state. This concept and description are based on the DATEX II concept EquipmentOrSystemFault."^^xsd:string ;
                     
                     rdfs:seeAlso "http://datex2.eu/schema/2/2_0#EquipmentOrSystemFault" .



###  http://purl.org/td/transportdisruption#InfrastructureImprovementOrUpgrading

:InfrastructureImprovementOrUpgrading rdf:type owl:Class ;
                                      
                                      rdfs:label "Infrastructure Improvement Or Upgrading"^^xsd:string ;
                                      
                                      rdfs:subClassOf :InfrastructureConstruction ;
                                      
                                      rdfs:comment "Construction work associated with improvements to the infrastructure or its layout or with it upgrading. This concept and description are a generalised version of the DATEX II concept roadImprovementOrUpgrading."^^xsd:string ;
                                      
                                      rdfs:seeAlso "http://datex2.eu/schema/2/2_0#RoadImprovementOrUpgrading" .



###  http://purl.org/td/transportdisruption#InfrastructureMaintenance

:InfrastructureMaintenance rdf:type owl:Class ;
                           
                           rdfs:label "Infrastructure Maintenance"^^xsd:string ;
                           
                           rdfs:subClassOf :InfrastructureWorks ;
                           
                           rdfs:comment "Infrastructure work involving the maintenance or installation of infrastructure. concept and description are a generalised version of the DATEX II concept MaintenanceWorks."^^xsd:string ;
                           
                           rdfs:seeAlso "http://datex2.eu/schema/2/2_0#MaintenanceWorks" .



###  http://purl.org/td/transportdisruption#InfrastructureSideAssistance

:InfrastructureSideAssistance rdf:type owl:Class ;
                              
                              rdfs:label "Infrastructure Side Assistance"^^xsd:string ;
                              
                              rdfs:subClassOf :OperatorAction ;
                              
                              rdfs:comment "Details of assistance required or being given at the side of transport infrastructure. This concept and description are a generalised version of the DATEX II concept RoadsideAssistance."^^xsd:string ;
                              
                              rdfs:seeAlso "http://datex2.eu/schema/2/2_0#RoadsideAssistance" .



###  http://purl.org/td/transportdisruption#InfrastructureSideCommunicationsSystemFailure

:InfrastructureSideCommunicationsSystemFailure rdf:type owl:Class ;
                                               
                                               rdfs:label "Side of Infrastructure Communications System Failure"^^xsd:string ;
                                               
                                               rdfs:subClassOf :InfrastructureFailure ;
                                               
                                               rdfs:comment "Failure of communications system at the side of infrastucture which is used by one or more equipments or systems. This concept and description are based on the DATEX II concept roadsideCommunicationsSystem."^^xsd:string ;
                                               
                                               rdfs:seeAlso "http://datex2.eu/schema/2/2_0#RoadsideCommunicationsSystem" .



###  http://purl.org/td/transportdisruption#InfrastructureSideCommunicationsSystemFault

:InfrastructureSideCommunicationsSystemFault rdf:type owl:Class ;
                                             
                                             rdfs:label "Side of Infrastructure Communications System Fault"^^xsd:string ;
                                             
                                             rdfs:subClassOf :InfrastructureFault ;
                                             
                                             rdfs:comment "Faulty or malfunctioning communications system at side of infrastructure which is used by one or more roadside equipments or systems. This concept and description are based on the DATEX II concept roadsideCommunicationsSystem."^^xsd:string ;
                                             
                                             rdfs:seeAlso "http://datex2.eu/schema/2/2_0#RoadsideCommunicationsSystem" .



###  http://purl.org/td/transportdisruption#InfrastructureSidePowerSystemFailure

:InfrastructureSidePowerSystemFailure rdf:type owl:Class ;
                                      
                                      rdfs:label "Side of Infrastructure Power System Failure"^^xsd:string ;
                                      
                                      rdfs:subClassOf :InfrastructureFailure ;
                                      
                                      rdfs:comment "Failure of power system at the side of infrastructure which is used by one or more equipments or system. This concept and description are based on the DATEX II concept roadsidePowerSystem."^^xsd:string ;
                                      
                                      rdfs:seeAlso "http://datex2.eu/schema/2/2_0#RoadsidePowerSystem" .



###  http://purl.org/td/transportdisruption#InfrastructureSidePowerSystemFault

:InfrastructureSidePowerSystemFault rdf:type owl:Class ;
                                    
                                    rdfs:label "Side of Infrastructure Power System Fault"^^xsd:string ;
                                    
                                    rdfs:subClassOf :InfrastructureFault ;
                                    
                                    rdfs:comment "Faulty or malfunctioning power system at side of infrastructure which is used by one or more roadside equipments or systems. This concept and description are based on the DATEX II concept roadsidePowerSystem."^^xsd:string ;
                                    
                                    rdfs:seeAlso "http://datex2.eu/schema/2/2_0#RoadsidePowerSystem" .



###  http://purl.org/td/transportdisruption#InfrastructureSideWork

:InfrastructureSideWork rdf:type owl:Class ;
                        
                        rdfs:label "Infrastructure Side Work"^^xsd:string ;
                        
                        rdfs:subClassOf :InfrastructureMaintenance ;
                        
                        rdfs:comment "Work of an unspecified nature carried out at the side of transport infrastructure. This concept and description are a generalised version of the DATEX II concept roadsideWork."^^xsd:string ;
                        
                        rdfs:seeAlso "http://datex2.eu/schema/2/2_0#RoadsideWork" .



###  http://purl.org/td/transportdisruption#InfrastructureSurfaceInPoorCondition

:InfrastructureSurfaceInPoorCondition rdf:type owl:Class ;
                                      
                                      rdfs:label "Infrastructure Surface In Poor Condition"^^xsd:string ;
                                      
                                      rdfs:subClassOf :AdverseInfrastructureConditions ;
                                      
                                      rdfs:comment "The infrastructure surface is damaged, severely rutted or potholed (i.e. it is in a poor state of repair). This concept and description are a generalised version of the DATEX II concept roadSurfaceInPoorCondition."^^xsd:string ;
                                      
                                      rdfs:seeAlso "http://datex2.eu/schema/2/2_0#RoadSurfaceInPoorCondition" .



###  http://purl.org/td/transportdisruption#InfrastructureWorks

:InfrastructureWorks rdf:type owl:Class ;
                     
                     rdfs:label "Infrastructure Works"^^xsd:string ;
                     
                     rdfs:subClassOf :OperatorAction ;
                     
                     rdfs:comment "Infrastructure maintenance or improvement activity of an unspecified nature which may potentially cause disruption to travel. This concept and description are a generalised version of the DATEX II concept roadworks."^^xsd:string ;
                     
                     rdfs:seeAlso "http://datex2.eu/schema/2/2_0#Roadworks" .



###  http://purl.org/td/transportdisruption#InfrastructureWorksClearance

:InfrastructureWorksClearance rdf:type owl:Class ;
                              
                              rdfs:label "Inffrastructure Works Clearance"^^xsd:string ;
                              
                              rdfs:subClassOf :InfrastructureMaintenance ;
                              
                              rdfs:comment "Infrastructure works are completed and are being cleared. This concept and description are a generalised version the DATEX II concept roadworksClearance."^^xsd:string ;
                              
                              rdfs:seeAlso "http://datex2.eu/schema/2/2_0#RoadworksClearance" .



###  http://purl.org/td/transportdisruption#InstallationWork

:InstallationWork rdf:type owl:Class ;
                  
                  rdfs:label "Installation Work"^^xsd:string ;
                  
                  rdfs:subClassOf :InfrastructureMaintenance ;
                  
                  rdfs:comment "Installation of new equipments or systems on or along-side some infrastructure. This concept and description are a generalised version of the DATEX II concept installationWork."^^xsd:string ;
                  
                  rdfs:seeAlso "http://datex2.eu/schema/2/2_0#InstallationWork" .



###  http://purl.org/td/transportdisruption#IntermittentShortTermClosures

:IntermittentShortTermClosures rdf:type owl:Class ;
                               
                               rdfs:label "Intermittent Short Term Closures"^^xsd:string ;
                               
                               rdfs:subClassOf :RoadOrCarriagewayOrLaneManagement ;
                               
                               rdfs:comment "Road closures occur intermittently on a specified road in a given direction for short durations. This concept and description are adaptations of the DATEX II concept intermittentShortTermClosures."^^xsd:string ;
                               
                               rdfs:seeAlso "http://datex2.eu/schema/2/2_0#IntermittentShortTermClosures" .



###  http://purl.org/td/transportdisruption#InternationalSportsMeeting

:InternationalSportsMeeting rdf:type owl:Class ;
                            
                            rdfs:label "International Sports Meeting"^^xsd:string ;
                            
                            rdfs:subClassOf :PublicEvent ;
                            
                            rdfs:comment "Large sporting event of an international nature that could disrupt traffic. This concept and description are from the DATEX II concept internationalSportsMeeting."^^xsd:string ;
                            
                            rdfs:seeAlso "http://datex2.eu/schema/2/2_0#InternationalSportsMeeting" .



###  http://purl.org/td/transportdisruption#JackknifedArticulatedLorry

:JackknifedArticulatedLorry rdf:type owl:Class ;
                            
                            rdfs:label "Jackknifed Articulated Lorry"^^xsd:string ;
                            
                            rdfs:subClassOf :JackknifedVehicle ;
                            
                            rdfs:comment "Includes all situations resulting in a heavy goods vehicle folding together in an accidental skidding movement on the carriageway. This concept and description are from the DATEX II concept jackknifedArticulatedLorry."^^xsd:string ;
                            
                            rdfs:seeAlso "http://datex2.eu/schema/2/2_0#JackknifedArticulatedLorry" .



###  http://purl.org/td/transportdisruption#JackknifedCaravan

:JackknifedCaravan rdf:type owl:Class ;
                   
                   rdfs:label "Jackknifed Caravan"^^xsd:string ;
                   
                   rdfs:subClassOf :JackknifedVehicle ;
                   
                   rdfs:comment "Includes all situations resulting in a vehicle and caravan folding together in an accidental skidding movement on the carriageway. This concept and description are from the DATEX II concept jackknifedCaravan."^^xsd:string ;
                   
                   rdfs:seeAlso "http://datex2.eu/schema/2/2_0#JackknifedCaravan" .



###  http://purl.org/td/transportdisruption#JackknifedRailwayVehicle

:JackknifedRailwayVehicle rdf:type owl:Class ;
                          
                          rdfs:label "Jackknifed Railway Vehicle"^^xsd:string ;
                          
                          rdfs:subClassOf :JackknifedVehicle ;
                          
                          rdfs:comment "Includes all situations resulting in a rail vehicle (carrage, engine, etc.) folding together in an accidental movement."^^xsd:string .



###  http://purl.org/td/transportdisruption#JackknifedTrailer

:JackknifedTrailer rdf:type owl:Class ;
                   
                   rdfs:label "Jackknifed Trailer"^^xsd:string ;
                   
                   rdfs:subClassOf :JackknifedVehicle ;
                   
                   rdfs:comment "Includes all situations resulting in a vehicle and trailer folding together in an accidental skidding movement on the carriageway. This concept and description are from the DATEX II concept jackknifedTrailer."^^xsd:string ;
                   
                   rdfs:seeAlso "http://datex2.eu/schema/2/2_0#JackknifedTrailer" .



###  http://purl.org/td/transportdisruption#JackknifedVehicle

:JackknifedVehicle rdf:type owl:Class ;
                   
                   rdfs:label "Jackknifed Vehicle"^^xsd:string ;
                   
                   rdfs:subClassOf :Accident ;
                   
                   rdfs:comment "Includes all situations resulting in a vehicle folding together in an accidental  movement, such as skidding."^^xsd:string .



###  http://purl.org/td/transportdisruption#JuridicalReconstruction

:JuridicalReconstruction rdf:type owl:Class ;
                         
                         rdfs:label "Juridical Reconstruction"^^xsd:string ;
                         
                         rdfs:subClassOf :AuthorityOperation ;
                         
                         rdfs:comment "An operation involving the juridical reconstruction of events for the purposes of judicial or legal proceedings. This concept and description are from the DATEX II concept juridicalReconstruction."^^xsd:string ;
                         
                         rdfs:seeAlso "http://datex2.eu/schema/2/2_0#JuridicalReconstruction" .



###  http://purl.org/td/transportdisruption#Landslips

:Landslips rdf:type owl:Class ;
           
           rdfs:label "Landslips"^^xsd:string ;
           
           rdfs:subClassOf :EnvironmentalObstruction ;
           
           rdfs:comment "Transport infrastructure obstructed or partially obstructed due to landslides. This concept and description are a generalised version of the DATEX II concept landslips."^^xsd:string ;
           
           rdfs:seeAlso "http://datex2.eu/schema/2/2_0#Landslips" .



###  http://purl.org/td/transportdisruption#LaneClosure

:LaneClosure rdf:type owl:Class ;
             
             rdfs:label "Lane Closure"^^xsd:string ;
             
             rdfs:subClassOf :RoadOrCarriagewayOrLaneManagement ;
             
             rdfs:comment "Lane closure in operation at a location. This concept and description are adaptations of the DATEX II concept laneClosures."^^xsd:string ;
             
             rdfs:seeAlso "http://datex2.eu/schema/2/2_0#LaneClosures" .



###  http://purl.org/td/transportdisruption#LaneControlSignFailure

:LaneControlSignFailure rdf:type owl:Class ;
                        
                        rdfs:label "Lane Control Sign Failure"^^xsd:string ;
                        
                        rdfs:subClassOf :InfrastructureFailure ;
                        
                        rdfs:comment "Failure of signs used to control lane usage (e.g. in tidal flow systems or hard shoulder running). This concept and description are based on the DATEX II concept laneControlSigns."^^xsd:string ;
                        
                        rdfs:seeAlso "http://datex2.eu/schema/2/2_0#LaneControlSigns" .



###  http://purl.org/td/transportdisruption#LaneControlSignFault

:LaneControlSignFault rdf:type owl:Class ;
                      
                      rdfs:label "Lane Control Sign Fault"^^xsd:string ;
                      
                      rdfs:subClassOf :InfrastructureFault ;
                      
                      rdfs:comment "Faulty or malfunctioning signs used to control lane usage (e.g. in tidal flow systems or hard shoulder running). This concept and description are based on the DATEX II concept laneControlSigns."^^xsd:string ;
                      
                      rdfs:seeAlso "http://datex2.eu/schema/2/2_0#LaneControlSigns" .



###  http://purl.org/td/transportdisruption#LanesDeviated

:LanesDeviated rdf:type owl:Class ;
               
               rdfs:label "Lanes Deviated"^^xsd:string ;
               
               rdfs:subClassOf :RoadOrCarriagewayOrLaneManagement ;
               
               rdfs:comment "Lane deviations are in operation at the specified location. This concept and description are from the DATEX II concept lanesDeviated."^^xsd:string ;
               
               rdfs:seeAlso "http://datex2.eu/schema/2/2_0#LanesDeviated" .



###  http://purl.org/td/transportdisruption#LargeAnimalsOnTheInfrastructure

:LargeAnimalsOnTheInfrastructure rdf:type owl:Class ;
                                 
                                 rdfs:label "Large Animals On The Infrastructure"^^xsd:string ;
                                 
                                 rdfs:subClassOf :AnimalPresenceObstruction ;
                                 
                                 rdfs:comment "Traffic may be disrupted due to large animals on transport infrastructure. This concept and description are a generalised version of the DATEX II concept largeAnimalsOnTheRoad."^^xsd:string ;
                                 
                                 rdfs:seeAlso "http://datex2.eu/schema/2/2_0#LargeAnimalsOnTheRoad" .



###  http://purl.org/td/transportdisruption#LeavesOnInfrastructure

:LeavesOnInfrastructure rdf:type owl:Class ;
                        
                        rdfs:label "Leaves On Infrastructure"^^xsd:string ;
                        
                        rdfs:subClassOf :AdverseInfrastructureConditions ;
                        
                        rdfs:comment "Leaves lying on transport infrastructure. This concept and description are a generalised version of the DATEX II concept leavesOnRoad."^^xsd:string ;
                        
                        rdfs:seeAlso "http://datex2.eu/schema/2/2_0#LeavesOnRoad" .



###  http://purl.org/td/transportdisruption#LevelCrossingFailure

:LevelCrossingFailure rdf:type owl:Class ;
                      
                      rdfs:label "Level Crossing Failure"^^xsd:string ;
                      
                      rdfs:subClassOf :InfrastructureFailure ;
                      
                      rdfs:comment "Failure of a level crossing (barriers and signals). This concept and description are based on the DATEX II concept levelCrossing."^^xsd:string ;
                      
                      rdfs:seeAlso "http://datex2.eu/schema/2/2_0#LevelCrossing" .



###  http://purl.org/td/transportdisruption#LevelCrossingFault

:LevelCrossingFault rdf:type owl:Class ;
                    
                    rdfs:label "Level Crossing Fault"^^xsd:string ;
                    
                    rdfs:subClassOf :InfrastructureFault ;
                    
                    rdfs:comment "Faulty or malfunctioning level crossing (barriers and signals). This concept and description are based on the DATEX II concept levelCrossing."^^xsd:string ;
                    
                    rdfs:seeAlso "http://datex2.eu/schema/2/2_0#LevelCrossing" .



###  http://purl.org/td/transportdisruption#LitterClearance

:LitterClearance rdf:type owl:Class ;
                 
                 rdfs:label "Litter Clearance"^^xsd:string ;
                 
                 rdfs:subClassOf :InfrastructureMaintenance ;
                 
                 rdfs:comment "Work to collect litter from the transport infrastructure and/or adjacent verges. This concept and description are a generalised version of the DATEX II concept litterClearance."^^xsd:string ;
                 
                 rdfs:seeAlso "http://datex2.eu/schema/2/2_0#LitterClearance" .



###  http://purl.org/td/transportdisruption#LongLoad

:LongLoad rdf:type owl:Class ;
          
          rdfs:label "Long Load"^^xsd:string ;
          
          rdfs:subClassOf :VehicleObstruction ;
          
          rdfs:comment "A vehicle of length greater than that normally allowed which may cause traffic disruption. This concept and description are from the DATEX II concept longLoad."^^xsd:string ;
          
          rdfs:seeAlso "http://datex2.eu/schema/2/2_0#LongLoad" .



###  http://purl.org/td/transportdisruption#LooseChippings

:LooseChippings rdf:type owl:Class ;
                
                rdfs:label "Loose Chippings"^^xsd:string ;
                
                rdfs:subClassOf :AdverseInfrastructureConditions ;
                
                rdfs:comment "Loose chippings transport infrastructure. This concept and description are a generalised version of the DATEX II concept looseChippings."^^xsd:string ;
                
                rdfs:seeAlso "http://datex2.eu/schema/2/2_0#LooseChippings" .



###  http://purl.org/td/transportdisruption#LooseSandOnInfrastructure

:LooseSandOnInfrastructure rdf:type owl:Class ;
                           
                           rdfs:label "Loose Sand On Infrastructure"^^xsd:string ;
                           
                           rdfs:subClassOf :AdverseInfrastructureConditions ;
                           
                           rdfs:comment "Loose sand on transport infrastructure. This concept and description are a generalised version of the DATEX II concept looseSandOnRoad."^^xsd:string ;
                           
                           rdfs:seeAlso "http://datex2.eu/schema/2/2_0#LooseSandOnRoad" .



###  http://purl.org/td/transportdisruption#LooseSnow

:LooseSnow rdf:type owl:Class ;
           
           rdfs:label "Loose Snow"^^xsd:string ;
           
           rdfs:subClassOf :WeatherRelatedConditions ;
           
           rdfs:comment "Powdery snow on the infrastructure which is subject to being blown by the wind. This concept and description are a generalised version of the DATEX II concept looseSnow."^^xsd:string ;
           
           rdfs:seeAlso "http://datex2.eu/schema/2/2_0#LooseSnow" .



###  http://purl.org/td/transportdisruption#LowSunGlare

:LowSunGlare rdf:type owl:Class ;
             
             rdfs:label "Low Sun Glare"^^xsd:string ;
             
             rdfs:subClassOf :EnvironmentalConditions ;
             
             rdfs:comment "Difficult visibility conditions created by low elevation sunlight. This concept and description are from the DATEX II concept lowSunGlare."^^xsd:string ;
             
             rdfs:seeAlso "http://datex2.eu/schema/2/2_0#LowSunGlare" .



###  http://purl.org/td/transportdisruption#MaintenanceWork

:MaintenanceWork rdf:type owl:Class ;
                 
                 rdfs:label "Maintenance Work"^^xsd:string ;
                 
                 rdfs:subClassOf :InfrastructureMaintenance ;
                 
                 rdfs:comment "Maintenance of transport and associated infrastructure or equipments. This concept and description are a generalised version of the the DATEX II concept maintenanceWork."^^xsd:string ;
                 
                 rdfs:seeAlso "http://datex2.eu/schema/2/2_0#MaintenanceWork" .



###  http://purl.org/td/transportdisruption#MajorEvent

:MajorEvent rdf:type owl:Class ;
            
            rdfs:label "Major Event"^^xsd:string ;
            
            rdfs:subClassOf :PublicEvent ;
            
            rdfs:comment "Significant organised event either on or near some transport infrastructure which could disrupt traffic. This concept and description are a generalised version of the DATEX II concept majorEvent."^^xsd:string ;
            
            rdfs:seeAlso "http://datex2.eu/schema/2/2_0#MajorEvent" .



###  http://purl.org/td/transportdisruption#Marathon

:Marathon rdf:type owl:Class ;
          
          rdfs:label "Marathon"^^xsd:string ;
          
          rdfs:subClassOf :PublicEvent ;
          
          rdfs:comment "Marathon, cross-country or road running event that could disrupt traffic. This concept and description are from the DATEX II concept marathon."^^xsd:string ;
          
          rdfs:seeAlso "http://datex2.eu/schema/2/2_0#Marathon" .



###  http://purl.org/td/transportdisruption#March

:March rdf:type owl:Class ;
       
       rdfs:label "March"^^xsd:string ;
       
       rdfs:subClassOf :DisturbanceActivity ;
       
       rdfs:comment "A situation where people are walking together in large groups for a common purpose, with potential to disrupt traffic. This concept and description are from the DATEX II concept march."^^xsd:string ;
       
       rdfs:seeAlso "http://datex2.eu/schema/2/2_0#March" .



###  http://purl.org/td/transportdisruption#Market

:Market rdf:type owl:Class ;
        
        rdfs:label "Market"^^xsd:string ;
        
        rdfs:subClassOf :PublicEvent ;
        
        rdfs:comment "Periodic (e.g. weekly) gathering for buying and selling, which could disrupt traffic. This concept and description are from the DATEX II concept market."^^xsd:string ;
        
        rdfs:seeAlso "http://datex2.eu/schema/2/2_0#Market" .



###  http://purl.org/td/transportdisruption#Match

:Match rdf:type owl:Class ;
       
       rdfs:label "Match"^^xsd:string ;
       
       rdfs:subClassOf :PublicEvent ;
       
       rdfs:comment "Sports match of unspecified type that could disrupt traffic. This concept and description are from the DATEX II concept match."^^xsd:string ;
       
       rdfs:seeAlso "http://datex2.eu/schema/2/2_0#Match" .



###  http://purl.org/td/transportdisruption#MatrixSignFailure

:MatrixSignFailure rdf:type owl:Class ;
                   
                   rdfs:label "Matrix Signs Failure"^^xsd:string ;
                   
                   rdfs:subClassOf :InfrastructureFailure ;
                   
                   rdfs:comment "Failure of matrix signs. These normally comprise a symbol display area surrounded by four lights (usually amber) which flash when a symbol is displayed.  This concept and description are based on the DATEX II concept matrixSigns."^^xsd:string ;
                   
                   rdfs:seeAlso "http://datex2.eu/schema/2/2_0#MatrixSigns" .



###  http://purl.org/td/transportdisruption#MatrixSignFault

:MatrixSignFault rdf:type owl:Class ;
                 
                 rdfs:label "Matrix Sign Fault"^^xsd:string ;
                 
                 rdfs:subClassOf :InfrastructureFault ;
                 
                 rdfs:comment "Faulty or malfunctioning matrix signs. These normally comprise a symbol display area surrounded by four lights (usually amber) which flash when a symbol is displayed.  This concept and description are based on the DATEX II concept matrixSigns."^^xsd:string ;
                 
                 rdfs:seeAlso "http://datex2.eu/schema/2/2_0#MatrixSigns" .



###  http://purl.org/td/transportdisruption#MilitaryConvoy

:MilitaryConvoy rdf:type owl:Class ;
                
                rdfs:label "Military Convoy"^^xsd:string ;
                
                rdfs:subClassOf :VehicleObstruction ;
                
                rdfs:comment "A group of military vehicles moving together in formation which may cause traffic disruption. This concept and description are from the DATEX II concept militaryConvoy."^^xsd:string ;
                
                rdfs:seeAlso "http://datex2.eu/schema/2/2_0#MilitaryConvoy" .



###  http://purl.org/td/transportdisruption#ModerateFog

:ModerateFog rdf:type owl:Class ;
             
             rdfs:label "Moderate Fog"^^xsd:string ;
             
             rdfs:subClassOf :EnvironmentalConditions ;
             
             rdfs:comment "Misty conditions impairing vision over 100m. This concept and description are from the DATEX II concept moderateFog."^^xsd:string ;
             
             rdfs:seeAlso "http://datex2.eu/schema/2/2_0#ModerateFog" .



###  http://purl.org/td/transportdisruption#MotorShow

:MotorShow rdf:type owl:Class ;
           
           rdfs:label "Motor Show"^^xsd:string ;
           
           rdfs:subClassOf :PublicEvent ;
           
           rdfs:comment "Motor show which could disrupt traffic. This concept and description are from the DATEX II concept motorShow."^^xsd:string ;
           
           rdfs:seeAlso "http://datex2.eu/schema/2/2_0#MotorShow" .



###  http://purl.org/td/transportdisruption#MotorSportRaceMeeting

:MotorSportRaceMeeting rdf:type owl:Class ;
                       
                       rdfs:label "Motor Sport Race Meeting"^^xsd:string ;
                       
                       rdfs:subClassOf :PublicEvent ;
                       
                       rdfs:comment "Motor sport race meeting that could disrupt traffic. This concept and description are from the DATEX II concept motorSportRaceMeeting."^^xsd:string ;
                       
                       rdfs:seeAlso "http://datex2.eu/schema/2/2_0#MotorSportRaceMeeting" .



###  http://purl.org/td/transportdisruption#MudOnInfrastructure

:MudOnInfrastructure rdf:type owl:Class ;
                     
                     rdfs:label "Mud On Infrastructure"^^xsd:string ;
                     
                     rdfs:subClassOf :AdverseInfrastructureConditions ;
                     
                     rdfs:comment "Mud on transport infrastructure. This concept and description are a generalised version of the DATEX II concept mudOnRoad."^^xsd:string ;
                     
                     rdfs:seeAlso "http://datex2.eu/schema/2/2_0#MudOnRoad" .



###  http://purl.org/td/transportdisruption#MudSlide

:MudSlide rdf:type owl:Class ;
          
          rdfs:label "Mud Slide"^^xsd:string ;
          
          rdfs:subClassOf :EnvironmentalObstruction ;
          
          rdfs:comment "Transport infrastructure obstructed or partially obstructed due to mudslides. This concept and description are a generalised version of the DATEX II concept mudSlide."^^xsd:string ;
          
          rdfs:seeAlso "http://datex2.eu/schema/2/2_0#MudSlide" .



###  http://purl.org/td/transportdisruption#MultipleVehicleCollision

:MultipleVehicleCollision rdf:type owl:Class ;
                          
                          rdfs:label "Multiple Vehicle Collision"^^xsd:string ;
                          
                          rdfs:subClassOf :Collision ;
                          
                          rdfs:comment "Multiple vehicles involved in a collision. This concept and description are from the DATEX II concept multipleVehicleCollision."^^xsd:string ;
                          
                          rdfs:seeAlso "http://datex2.eu/schema/2/2_0#MultipleVehicleCollision" .



###  http://purl.org/td/transportdisruption#MultivehicleAccident

:MultivehicleAccident rdf:type owl:Class ;
                      
                      rdfs:label "Multivehicle Accident"^^xsd:string ;
                      
                      rdfs:subClassOf :Accident ;
                      
                      rdfs:comment "Includes all accidents involving three or more vehicles. This concept and description are from the DATEX II concept multivehicleAccident."^^xsd:string ;
                      
                      rdfs:seeAlso "http://datex2.eu/schema/2/2_0#MultivehicleAccident" .



###  http://purl.org/td/transportdisruption#NarrowLanes

:NarrowLanes rdf:type owl:Class ;
             
             rdfs:label "Narrow Lanes"^^xsd:string ;
             
             rdfs:subClassOf :RoadOrCarriagewayOrLaneManagement ;
             
             rdfs:comment "Normal lane widths are temporarily reduced. This concept and description are from the DATEX II concept narrowLanes."^^xsd:string ;
             
             rdfs:seeAlso "http://datex2.eu/schema/2/2_0#NarrowLanes" .



###  http://purl.org/td/transportdisruption#NetworkManagement

:NetworkManagement rdf:type owl:Class ;
                   
                   rdfs:label "Network Management"^^xsd:string ;
                   
                   rdfs:subClassOf :OperatorAction ;
                   
                   rdfs:comment "Network management action which is applicable to the transport network and its users. This concept and description are a generalised version the DATEX II concept NetworkManagement."^^xsd:string ;
                   
                   rdfs:seeAlso "http://datex2.eu/schema/2/2_0#NetworkManagement" .



###  http://purl.org/td/transportdisruption#NewRoadworksLayout

:NewRoadworksLayout rdf:type owl:Class ;
                    
                    rdfs:label "New Roadworks Layout"^^xsd:string ;
                    
                    rdfs:subClassOf :RoadOrCarriagewayOrLaneManagement ;
                    
                    rdfs:comment "A new layout of lanes/carriageway has been implemented associated with roadworks. This concept and description are from the DATEX II concept newRoadworksLayout."^^xsd:string ;
                    
                    rdfs:seeAlso "http://datex2.eu/schema/2/2_0#NewRoadworksLayout" .



###  http://purl.org/td/transportdisruption#Normal

:Normal rdf:type owl:Class ;
        
        rdfs:label "Normal"^^xsd:string ;
        
        rdfs:subClassOf :DrivingCondition ;
        
        rdfs:comment "Driving conditions are normal. This concept and description are from the DATEX II concept normal."^^xsd:string ;
        
        rdfs:seeAlso "http://datex2.eu/schema/2/2_0#Normal" .



###  http://purl.org/td/transportdisruption#NormalWinterConditionsForPedestrians

:NormalWinterConditionsForPedestrians rdf:type owl:Class ;
                                      
                                      rdfs:label "Normal Winter Conditions For Pedestrians"^^xsd:string ;
                                      
                                      rdfs:subClassOf :WeatherRelatedConditions ;
                                      
                                      rdfs:comment "Conditions for pedestrians are consistent with those normally expected in winter. This concept and description are from the DATEX II concept normalWinterConditionsForPedestrians."^^xsd:string ;
                                      
                                      rdfs:seeAlso "http://datex2.eu/schema/2/2_0#NormalWinterConditionsForPedestrians" .



###  http://purl.org/td/transportdisruption#ObstacleSignalling

:ObstacleSignalling rdf:type owl:Class ;
                    
                    rdfs:label "Obstacle Signalling"^^xsd:string ;
                    
                    rdfs:subClassOf :GeneralNetworkManagement ;
                    
                    rdfs:comment "Signs are being put out before or around an obstacle to protect drivers. This concept and description are from the DATEX II concept obstacleSignalling."^^xsd:string ;
                    
                    rdfs:seeAlso "http://datex2.eu/schema/2/2_0#ObstacleSignalling" .



###  http://purl.org/td/transportdisruption#Obstruction

:Obstruction rdf:type owl:Class ;
             
             rdfs:label "Obstruction"^^xsd:string ;
             
             rdfs:subClassOf :TrafficElementEvent ;
             
             rdfs:comment "Any stationary or moving obstacle of a physical nature (e.g. obstacles or vehicles from an earlier accident, shed loads on carriageway, rock fall, abnormal or dangerous loads, or animals etc.) which could disrupt or endanger traffic. This concept and description are from the DATEX II concept Obstruction."^^xsd:string ;
             
             rdfs:seeAlso "http://datex2.eu/schema/2/2_0#Obstruction" .



###  http://purl.org/td/transportdisruption#OilOnInfrastructure

:OilOnInfrastructure rdf:type owl:Class ;
                     
                     rdfs:label "Oil On Infrastructure"^^xsd:string ;
                     
                     rdfs:subClassOf :AdverseInfrastructureConditions ;
                     
                     rdfs:comment "Oil on infrastructure. This concept and description are a generalised version of the DATEX II concept oilOnRoad."^^xsd:string ;
                     
                     rdfs:seeAlso "http://datex2.eu/schema/2/2_0#OilOnRoad" .



###  http://purl.org/td/transportdisruption#OilSpillageAccident

:OilSpillageAccident rdf:type owl:Class ;
                     
                     rdfs:label "Oil Spillage Accident"^^xsd:string ;
                     
                     rdfs:subClassOf :SpillageAccident ;
                     
                     rdfs:comment "Includes all situations resulting in a spillage of oil. This concept and description are a generalised version the DATEX II concept oilSpillageAccident."^^xsd:string ;
                     
                     rdfs:seeAlso "http://datex2.eu/schema/2/2_0#OilSpillageAccident" .



###  http://purl.org/td/transportdisruption#OperatorAction

:OperatorAction rdf:type owl:Class ;
                
                rdfs:label "Operator Action"^^xsd:string ;
                
                rdfs:subClassOf <http://purl.org/NET/c4dm/event.owl#Event> ;
                
                rdfs:comment "Actions that an operator can decide to implement to prevent or help correct dangerous or poor transport or travel conditions. This concept and description is based on the DATEX II concept OperatorAction."^^xsd:string ;
                
                rdfs:seeAlso "http://datex2.eu/schema/2/2_0#OperatorAction" .



###  http://purl.org/td/transportdisruption#OverheadWorks

:OverheadWorks rdf:type owl:Class ;
               
               rdfs:label "Overhead Works"^^xsd:string ;
               
               rdfs:subClassOf :InfrastructureMaintenance ;
               
               rdfs:comment "Works which are overhead of the transport infrastructure. This concept and description are a generalised version of the DATEX II concept overheadWorks."^^xsd:string ;
               
               rdfs:seeAlso "http://datex2.eu/schema/2/2_0#OverheadWorks" .



###  http://purl.org/td/transportdisruption#OverheightVehicle

:OverheightVehicle rdf:type owl:Class ;
                   
                   rdfs:label "Overheight Vehicle"^^xsd:string ;
                   
                   rdfs:subClassOf :VehicleObstruction ;
                   
                   rdfs:comment "Vehicles of height greater than normally allowed which may cause traffic disruption. This concept and description are from the DATEX II concept overheightVehicle."^^xsd:string ;
                   
                   rdfs:seeAlso "http://datex2.eu/schema/2/2_0#OverheightVehicle" .



###  http://purl.org/td/transportdisruption#OvernightClosures

:OvernightClosures rdf:type owl:Class ;
                   
                   rdfs:label "Overnight Closures"^^xsd:string ;
                   
                   rdfs:subClassOf :RoadOrCarriagewayOrLaneManagement ;
                   
                   rdfs:comment "Every night the road is closed to vehicles, either all or those with specified characteristics by decision of the appropriate authorities. This concept and description are adaptations of the DATEX II concept overnightClosures."^^xsd:string ;
                   
                   rdfs:seeAlso "http://datex2.eu/schema/2/2_0#OvernightClosures" .



###  http://purl.org/td/transportdisruption#OverturnedHeavyLorry

:OverturnedHeavyLorry rdf:type owl:Class ;
                      
                      rdfs:label "Overturned Heavy Lorry"^^xsd:string ;
                      
                      rdfs:subClassOf :OverturnedVehicle ;
                      
                      rdfs:comment "Includes all situations resulting in the overturning of a heavy goods vehicle on the carriageway. This concept and description are from the DATEX II concept overturnedHeavyLorry."^^xsd:string ;
                      
                      rdfs:seeAlso "http://datex2.eu/schema/2/2_0#OverturnedHeavyLorry" .



###  http://purl.org/td/transportdisruption#OverturnedTrailer

:OverturnedTrailer rdf:type owl:Class ;
                   
                   rdfs:label "Overturned Trailer"^^xsd:string ;
                   
                   rdfs:subClassOf :OverturnedVehicle ;
                   
                   rdfs:comment "Includes all situations resulting in the overturning of a trailer. This concept and description are from the DATEX II concept overturnedTrailer."^^xsd:string ;
                   
                   rdfs:seeAlso "http://datex2.eu/schema/2/2_0#OverturnedTrailer" .



###  http://purl.org/td/transportdisruption#OverturnedVehicle

:OverturnedVehicle rdf:type owl:Class ;
                   
                   rdfs:label "Overturned Vehicle"^^xsd:string ;
                   
                   rdfs:subClassOf :Accident ;
                   
                   rdfs:comment "Includes all situations resulting in the overturning of a vehicle (of unspecified type) on the carriageway. This concept and description are from the DATEX II concept overturnedVehicle."^^xsd:string ;
                   
                   rdfs:seeAlso "http://datex2.eu/schema/2/2_0#OverturnedVehicle" .



###  http://purl.org/td/transportdisruption#OzonePollution

:OzonePollution rdf:type owl:Class ;
                
                rdfs:label "Ozone Pollution"^^xsd:string ;
                
                rdfs:subClassOf :EnvironmentalConditions ;
                
                rdfs:comment "High concentrations of ozone are present. This concept and description are from the DATEX II concept ozonePollution."^^xsd:string ;
                
                rdfs:seeAlso "http://datex2.eu/schema/2/2_0#OzonePollution" .



###  http://purl.org/td/transportdisruption#PackedSnow

:PackedSnow rdf:type owl:Class ;
            
            rdfs:label "Packed Snow"^^xsd:string ;
            
            rdfs:subClassOf :WeatherRelatedConditions ;
            
            rdfs:comment "Packed snow (heavily trafficked) on the transport infrastructure. This concept and description are a generalised version of the DATEX II concept packedSnow."^^xsd:string ;
            
            rdfs:seeAlso "http://datex2.eu/schema/2/2_0#PackedSnow" .



###  http://purl.org/td/transportdisruption#Parade

:Parade rdf:type owl:Class ;
        
        rdfs:label "Parade"^^xsd:string ;
        
        rdfs:subClassOf :PublicEvent ;
        
        rdfs:comment "Formal display or organised procession which could disrupt traffic. This concept and description are from the DATEX II concept parade."^^xsd:string ;
        
        rdfs:seeAlso "http://datex2.eu/schema/2/2_0#Parade" .



###  http://purl.org/td/transportdisruption#PassableWithCare

:PassableWithCare rdf:type owl:Class ;
                  
                  rdfs:label "Passable With Care"^^xsd:string ;
                  
                  rdfs:subClassOf :DrivingCondition ;
                  
                  rdfs:comment "The roadway is passable to vehicles with driver care. This concept and description are from the DATEX II concept passableWithCare."^^xsd:string ;
                  
                  rdfs:seeAlso "http://datex2.eu/schema/2/2_0#PassableWithCare" .



###  http://purl.org/td/transportdisruption#PassengerAssistance

:PassengerAssistance rdf:type owl:Class ;
                     
                     rdfs:label "Passenger Assistance"^^xsd:string ;
                     
                     rdfs:subClassOf :InfrastructureSideAssistance ;
                     
                     rdfs:comment "Bus, rail, ferry, etc. passenger assistance. This concept and description are a generalised version of the DATEX II concept busPassengerAssistance."^^xsd:string ;
                     
                     rdfs:seeAlso "http://datex2.eu/schema/2/2_0#BusPassengerAssistance" .



###  http://purl.org/td/transportdisruption#PatchyFog

:PatchyFog rdf:type owl:Class ;
           
           rdfs:label "Patchy Fog"^^xsd:string ;
           
           rdfs:subClassOf :EnvironmentalConditions ;
           
           rdfs:comment "Fog, in which intermittent areas of dense fog may be encountered. This concept and description are from the DATEX II concept patchyFog."^^xsd:string ;
           
           rdfs:seeAlso "http://datex2.eu/schema/2/2_0#PatchyFog" .



###  http://purl.org/td/transportdisruption#PetrolOnInfrastructure

:PetrolOnInfrastructure rdf:type owl:Class ;
                        
                        rdfs:label "Petrol On Infrastructure"^^xsd:string ;
                        
                        rdfs:subClassOf :AdverseInfrastructureConditions ;
                        
                        rdfs:comment "Petrol on infrascture. This concept and description are a generalised version of the DATEX II concept petrolOnRoad."^^xsd:string ;
                        
                        rdfs:seeAlso "http://datex2.eu/schema/2/2_0#PetrolOnRoad" .



###  http://purl.org/td/transportdisruption#Plan

:Plan rdf:type owl:Class ;
      
      rdfs:label "Plan"^^xsd:string ;
      
      rdfs:comment "Plan provides an extension point for users of the ontology to describe an agent's plan that may be impacted by an event."^^xsd:string .



###  http://purl.org/td/transportdisruption#PoliceCheckPoint

:PoliceCheckPoint rdf:type owl:Class ;
                  
                  rdfs:label "Police Check Point"^^xsd:string ;
                  
                  rdfs:subClassOf :AuthorityOperation ;
                  
                  rdfs:comment "A permanent or temporary operation established on or adjacent to the transport infrastructure for use by police or other authorities. This concept and description are a generalised version of the DATEX II concept policeCheckPoint."^^xsd:string ;
                  
                  rdfs:seeAlso "http://datex2.eu/schema/2/2_0#PoliceCheckPoint" .



###  http://purl.org/td/transportdisruption#PoliceInvestigation

:PoliceInvestigation rdf:type owl:Class ;
                     
                     rdfs:label "Police Investigation"^^xsd:string ;
                     
                     rdfs:subClassOf :AuthorityOperation ;
                     
                     rdfs:comment "A temporary operation established on or adjacent to the transport infrastructure by the police associated with an ongoing investigation. This concept and description are a generalised version of the DATEX II concept policeInvestigation."^^xsd:string ;
                     
                     rdfs:seeAlso "http://datex2.eu/schema/2/2_0#PoliceInvestigation" .



###  http://purl.org/td/transportdisruption#PoliceSpeedChecksInOperation

:PoliceSpeedChecksInOperation rdf:type owl:Class ;
                              
                              rdfs:label "Police Speed Checks In Operation"^^xsd:string ;
                              
                              rdfs:subClassOf :SpeedManagement ;
                              
                              rdfs:comment "Police speed checks are in operation. This concept and description are from the DATEX II concept policeSpeedChecksInOperation."^^xsd:string ;
                              
                              rdfs:seeAlso "http://datex2.eu/schema/2/2_0#PoliceSpeedChecksInOperation" .



###  http://purl.org/td/transportdisruption#Pollution

:Pollution rdf:type owl:Class ;
           
           rdfs:label "Pollution"^^xsd:string ;
           
           rdfs:subClassOf :EnvironmentalConditions ;
           
           rdfs:comment "Pollution of an unspecified nature. This concept and description are from the DATEX II concept pollution."^^xsd:string ;
           
           rdfs:seeAlso "http://datex2.eu/schema/2/2_0#Pollution" .



###  http://purl.org/td/transportdisruption#PrecipitationInTheArea

:PrecipitationInTheArea rdf:type owl:Class ;
                        
                        rdfs:label "Precipitation In The Area"^^xsd:string ;
                        
                        rdfs:subClassOf :EnvironmentalConditions ;
                        
                        rdfs:comment "Unspecified precipitation is falling on the area. This concept and description are from the DATEX II concept precipitationInTheArea."^^xsd:string ;
                        
                        rdfs:seeAlso "http://datex2.eu/schema/2/2_0#PrecipitationInTheArea" .



###  http://purl.org/td/transportdisruption#Procession

:Procession rdf:type owl:Class ;
            
            rdfs:label "Procession"^^xsd:string ;
            
            rdfs:subClassOf :PublicEvent ;
            
            rdfs:comment "An organised procession which could disrupt traffic. This concept and description are from the DATEX II concept procession."^^xsd:string ;
            
            rdfs:seeAlso "http://datex2.eu/schema/2/2_0#Procession" .



###  http://purl.org/td/transportdisruption#ProhibitedVehicleOnTheRoadway

:ProhibitedVehicleOnTheRoadway rdf:type owl:Class ;
                               
                               rdfs:label "Prohibited Vehicle On The Roadway"^^xsd:string ;
                               
                               rdfs:subClassOf :VehicleObstruction ;
                               
                               rdfs:comment "Vehicles not normally permitted on the highway are present which may cause traffic disruption. This concept and description are from the DATEX II concept prohibitedVehicleOnTheRoadway."^^xsd:string ;
                               
                               rdfs:seeAlso "http://datex2.eu/schema/2/2_0#ProhibitedVehicleOnTheRoadway" .



###  http://purl.org/td/transportdisruption#PublicDisturbance

:PublicDisturbance rdf:type owl:Class ;
                   
                   rdfs:label "Public Disturbance"^^xsd:string ;
                   
                   rdfs:subClassOf :DisturbanceActivity ;
                   
                   rdfs:comment "A situation of public disorder, with potential to disrupt traffic. This concept and description are from the DATEX II concept publicDisturbance."^^xsd:string ;
                   
                   rdfs:seeAlso "http://datex2.eu/schema/2/2_0#PublicDisturbance" .



###  http://purl.org/td/transportdisruption#PublicEvent

:PublicEvent rdf:type owl:Class ;
             
             rdfs:label "Public Event"^^xsd:string ;
             
             rdfs:subClassOf :Activity ;
             
             rdfs:comment "Organised public event which could disrupt traffic. This concept and description are from the DATEX II concept PublicEvent."^^xsd:string ;
             
             rdfs:seeAlso "http://datex2.eu/schema/2/2_0#PublicEvent" .



###  http://purl.org/td/transportdisruption#PublicTransportCancellation

:PublicTransportCancellation rdf:type owl:Class ;
                             
                             rdfs:label "Public Transport Cancellation"^^xsd:string ;
                             
                             rdfs:subClassOf :PublicTransportEvent ;
                             
                             rdfs:comment "A cancellation of a public transport service, route, trip, etc."^^xsd:string .



###  http://purl.org/td/transportdisruption#PublicTransportDelay

:PublicTransportDelay rdf:type owl:Class ;
                      
                      rdfs:label "Public Transport Delay"^^xsd:string ;
                      
                      rdfs:subClassOf :PublicTransportEvent ;
                      
                      rdfs:comment "A delay to a public transport service, trip, route, etc."^^xsd:string .



###  http://purl.org/td/transportdisruption#PublicTransportDiversion

:PublicTransportDiversion rdf:type owl:Class ;
                          
                          rdfs:label "Public Transport Diversion"^^xsd:string ;
                          
                          rdfs:subClassOf :PublicTransportEvent ;
                          
                          rdfs:comment "A diversion to the typical route of a public transport service, trip, etc."^^xsd:string .



###  http://purl.org/td/transportdisruption#PublicTransportEvent

:PublicTransportEvent rdf:type owl:Class ;
                      
                      rdfs:label "Public Transport Event"^^xsd:string ;
                      
                      rdfs:subClassOf <http://purl.org/NET/c4dm/event.owl#Event> ;
                      
                      rdfs:comment "A public transport event is an event that features some form of public transport: bus, rail, air, ferry, etc."^^xsd:string .



###  http://purl.org/td/transportdisruption#QueuingTraffic

:QueuingTraffic rdf:type owl:Class ;
                
                rdfs:label "Queuing Traffic"^^xsd:string ;
                
                rdfs:subClassOf :AbnormalTraffic ;
                
                rdfs:comment "Traffic is queuing at the specified location, although there is still some traffic movement.  For road traffic, DATEX II defines this as i.e. average speed is between 10% and 25% of its free-flow level). This concept and description are adaptations of the DATEX II concept queuingTraffic."^^xsd:string ;
                
                rdfs:seeAlso "http://datex2.eu/schema/2/2_0#QueuingTraffic" .



###  http://purl.org/td/transportdisruption#RaceMeeting

:RaceMeeting rdf:type owl:Class ;
             
             rdfs:label "Race Meeting"^^xsd:string ;
             
             rdfs:subClassOf :PublicEvent ;
             
             rdfs:comment "Race meeting (other than horse or motor sport) that could disrupt traffic. This concept and description are from the DATEX II concept raceMeeting."^^xsd:string ;
             
             rdfs:seeAlso "http://datex2.eu/schema/2/2_0#RaceMeeting" .



###  http://purl.org/td/transportdisruption#RadioactiveLeakAlert

:RadioactiveLeakAlert rdf:type owl:Class ;
                      
                      rdfs:label "Radioactive Leak Alert"^^xsd:string ;
                      
                      rdfs:subClassOf :DisturbanceActivity ;
                      
                      rdfs:comment "An alert to a radioactive leak which may endanger the public and hence may cause traffic disruption. This concept and description are from the DATEX II concept radioactiveLeakAlert."^^xsd:string ;
                      
                      rdfs:seeAlso "http://datex2.eu/schema/2/2_0#RadioactiveLeakAlert" .



###  http://purl.org/td/transportdisruption#Rain

:Rain rdf:type owl:Class ;
      
      rdfs:label "Rain"^^xsd:string ;
      
      rdfs:subClassOf :EnvironmentalConditions ;
      
      rdfs:comment "Rain, visibility more than 50m. This concept and description are from the DATEX II concept rain."^^xsd:string ;
      
      rdfs:seeAlso "http://datex2.eu/schema/2/2_0#Rain" .



###  http://purl.org/td/transportdisruption#RainChangingToSnow

:RainChangingToSnow rdf:type owl:Class ;
                    
                    rdfs:label "Rain Changing To Snow"^^xsd:string ;
                    
                    rdfs:subClassOf :EnvironmentalConditions ;
                    
                    rdfs:comment "Falling rain is changing to snow. This concept and description are from the DATEX II concept rainChangingToSnow."^^xsd:string ;
                    
                    rdfs:seeAlso "http://datex2.eu/schema/2/2_0#RainChangingToSnow" .



###  http://purl.org/td/transportdisruption#RampControlFailure

:RampControlFailure rdf:type owl:Class ;
                    
                    rdfs:label "Ramp Control Failure"^^xsd:string ;
                    
                    rdfs:subClassOf :InfrastructureFailure ;
                    
                    rdfs:comment "Failure of ramp control equipment. This concept and description are based on the DATEX II concept rampControls."^^xsd:string ;
                    
                    rdfs:seeAlso "http://datex2.eu/schema/2/2_0#RampControls" .



###  http://purl.org/td/transportdisruption#RampControlFault

:RampControlFault rdf:type owl:Class ;
                  
                  rdfs:label "Ramp Control Fault"^^xsd:string ;
                  
                  rdfs:subClassOf :InfrastructureFault ;
                  
                  rdfs:comment "Faulty or malfunctioning ramp control equipment. This concept and description are based on the DATEX II concept rampControls."^^xsd:string ;
                  
                  rdfs:seeAlso "http://datex2.eu/schema/2/2_0#RampControls" .



###  http://purl.org/td/transportdisruption#RampMeteringInOperation

:RampMeteringInOperation rdf:type owl:Class ;
                         
                         rdfs:label "Ramp Metering In Operation"^^xsd:string ;
                         
                         rdfs:subClassOf :GeneralNetworkManagement ;
                         
                         rdfs:comment "Ramp metering is now active at the specified location. This concept and description are from the DATEX II concept rampMeteringInOperation."^^xsd:string ;
                         
                         rdfs:seeAlso "http://datex2.eu/schema/2/2_0#RampMeteringInOperation" .



###  http://purl.org/td/transportdisruption#RearCollision

:RearCollision rdf:type owl:Class ;
               
               rdfs:label "Rear Collision"^^xsd:string ;
               
               rdfs:subClassOf :Collision ;
               
               rdfs:comment "Includes all accidents where one or more vehicles have collided with the rear of one or more other vehicles. This concept and description are from the DATEX II concept rearCollision."^^xsd:string ;
               
               rdfs:seeAlso "http://datex2.eu/schema/2/2_0#RearCollision" .



###  http://purl.org/td/transportdisruption#RepairWork

:RepairWork rdf:type owl:Class ;
            
            rdfs:label "Repair Work"^^xsd:string ;
            
            rdfs:subClassOf :InfrastructureMaintenance ;
            
            rdfs:comment "Repair work to infrastructure or equipments. This concept and description are a generalised version of the DATEX II concept repairWork."^^xsd:string ;
            
            rdfs:seeAlso "http://datex2.eu/schema/2/2_0#RepairWork" .



###  http://purl.org/td/transportdisruption#ResurfacingWork

:ResurfacingWork rdf:type owl:Class ;
                 
                 rdfs:label "Resurfacing Work"^^xsd:string ;
                 
                 rdfs:subClassOf :InfrastructureMaintenance ;
                 
                 rdfs:comment "Work associated with relaying or renewal of road, runway, or similar infrastructure. This concept and description are a generalised version of the DATEX II concept resurfacingWork."^^xsd:string ;
                 
                 rdfs:seeAlso "http://datex2.eu/schema/2/2_0#ResurfacingWork" .



###  http://purl.org/td/transportdisruption#Riot

:Riot rdf:type owl:Class ;
      
      rdfs:label "Riot"^^xsd:string ;
      
      rdfs:subClassOf :DisturbanceActivity ;
      
      rdfs:comment "A situation of public disorder involving violent behaviour and/or destruction of property with the potential to disrupt traffic. This concept and description are from the DATEX II concept riot."^^xsd:string ;
      
      rdfs:seeAlso "http://datex2.eu/schema/2/2_0#Riot" .



###  http://purl.org/td/transportdisruption#RoadCleared

:RoadCleared rdf:type owl:Class ;
             
             rdfs:label "Road Cleared"^^xsd:string ;
             
             rdfs:subClassOf :RoadOrCarriagewayOrLaneManagement ;
             
             rdfs:comment "The road has been cleared of earlier reported problems. This concept and description are from the DATEX II concept roadCleared."^^xsd:string ;
             
             rdfs:seeAlso "http://datex2.eu/schema/2/2_0#RoadCleared" .



###  http://purl.org/td/transportdisruption#RoadClosure

:RoadClosure rdf:type owl:Class ;
             
             rdfs:label "Road Closure"^^xsd:string ;
             
             rdfs:subClassOf :RoadOrCarriagewayOrLaneManagement ;
             
             rdfs:comment "A road is closed to vehicles with the specified characteristics or all, if none defined, in the specified direction. This concept and description are adaptions of the DATEX II concept roadClosed."^^xsd:string ;
             
             rdfs:seeAlso "http://datex2.eu/schema/2/2_0#RoadClosed" .



###  http://purl.org/td/transportdisruption#RoadMarkingWork

:RoadMarkingWork rdf:type owl:Class ;
                 
                 rdfs:label "Road Marking Work"^^xsd:string ;
                 
                 rdfs:subClassOf :InfrastructureMaintenance ;
                 
                 rdfs:comment "Striping and repainting of road markings, plus placement or replacement of reflecting studs (cats' eyes). This concept and description are from the DATEX II concept roadMarkingWork."^^xsd:string ;
                 
                 rdfs:seeAlso "http://datex2.eu/schema/2/2_0#RoadMarkingWork" .



###  http://purl.org/td/transportdisruption#RoadOperatorCheckPoint

:RoadOperatorCheckPoint rdf:type owl:Class ;
                        
                        rdfs:label "Road Operator Check Point"^^xsd:string ;
                        
                        rdfs:subClassOf :AuthorityOperation ;
                        
                        rdfs:comment "A permanent or temporary operation established on or adjacent to the carriageway for use by the road operator, such as for survey or inspection purposes, but not for traffic management purposes. This concept and description are from the DATEX II concept roadOperatorCheckPoint."^^xsd:string ;
                        
                        rdfs:seeAlso "http://datex2.eu/schema/2/2_0#RoadOperatorCheckPoint" .



###  http://purl.org/td/transportdisruption#RoadOrCarriagewayOrLaneManagement

:RoadOrCarriagewayOrLaneManagement rdf:type owl:Class ;
                                   
                                   rdfs:label "Road Or Carriageway Or Lane Management"^^xsd:string ;
                                   
                                   rdfs:subClassOf :NetworkManagement ;
                                   
                                   rdfs:comment "Road, carriageway or lane management action that is instigated by the network/road operator. This concept and description are from the DATEX II concept RoadOrCarriagewayOrLaneManagement."^^xsd:string ;
                                   
                                   rdfs:seeAlso "http://datex2.eu/schema/2/2_0#RoadOrCarriagewayOrLaneManagement" .



###  http://purl.org/td/transportdisruption#RoadSurfaceMelting

:RoadSurfaceMelting rdf:type owl:Class ;
                    
                    rdfs:label "Road Surface Melting"^^xsd:string ;
                    
                    rdfs:subClassOf :WeatherRelatedConditions ;
                    
                    rdfs:comment "The infrastructure surface is melting, or has melted due to abnormally high temperatures. This concept and description are a generalised version of the DATEX II concept roadSurfaceMelting."^^xsd:string ;
                    
                    rdfs:seeAlso "http://datex2.eu/schema/2/2_0#RoadSurfaceMelting" .



###  http://purl.org/td/transportdisruption#RoadWideningWork

:RoadWideningWork rdf:type owl:Class ;
                  
                  rdfs:label "Road Widening Work"^^xsd:string ;
                  
                  rdfs:subClassOf :InfrastructureConstruction ;
                  
                  rdfs:comment "Road widening work at the specified location. This concept and description are from the DATEX II concept roadWideningWork."^^xsd:string ;
                  
                  rdfs:seeAlso "http://datex2.eu/schema/2/2_0#RoadWideningWork" .



###  http://purl.org/td/transportdisruption#RoadWorks

:RoadWorks rdf:type owl:Class ;
           
           rdfs:label "Roadworks"^^xsd:string ;
           
           rdfs:subClassOf :InfrastructureMaintenance ;
           
           rdfs:comment "Road maintenance or improvement activity of an unspecified nature which may potentially cause disruption to travel. This concept and description are from the DATEX II concept roadworks."^^xsd:string .



###  http://purl.org/td/transportdisruption#RockFallPreventativeMaintenance

:RockFallPreventativeMaintenance rdf:type owl:Class ;
                                 
                                 rdfs:label "Rock Fall Preventative Maintenance"^^xsd:string ;
                                 
                                 rdfs:subClassOf :InfrastructureMaintenance ;
                                 
                                 rdfs:comment "Rock fall preventative maintenance. This concept and description are from the DATEX II concept rockFallPreventativeMaintenance."^^xsd:string ;
                                 
                                 rdfs:seeAlso "http://datex2.eu/schema/2/2_0#RockFallPreventativeMaintenance" .



###  http://purl.org/td/transportdisruption#Rockfalls

:Rockfalls rdf:type owl:Class ;
           
           rdfs:label "Rockfalls"^^xsd:string ;
           
           rdfs:subClassOf :EnvironmentalObstruction ;
           
           rdfs:comment "Transport infrastructure obstructed or partially obstructed due to fallen rocks. This concept and description are a generalised version of the DATEX II concept rockfalls."^^xsd:string ;
           
           rdfs:seeAlso "http://datex2.eu/schema/2/2_0#Rockfalls" .



###  http://purl.org/td/transportdisruption#RollingRoadBlock

:RollingRoadBlock rdf:type owl:Class ;
                  
                  rdfs:label "Rolling Road Block"^^xsd:string ;
                  
                  rdfs:subClassOf :RoadOrCarriagewayOrLaneManagement ;
                  
                  rdfs:comment "Traffic officers or police are driving slowly in front of a queue of traffic to create a gap in the traffic to allow for clearance activities to take place in safety on the road ahead. This concept and description are from the DATEX II concept rollingRoadBlock."^^xsd:string ;
                  
                  rdfs:seeAlso "http://datex2.eu/schema/2/2_0#RollingRoadBlock" .



###  http://purl.org/td/transportdisruption#RugbyMatch

:RugbyMatch rdf:type owl:Class ;
            
            rdfs:label "Rugby Match"^^xsd:string ;
            
            rdfs:subClassOf :PublicEvent ;
            
            rdfs:comment "Rugby match that could disrupt traffic. This concept and description are from the DATEX II concept rugbyMatch."^^xsd:string ;
            
            rdfs:seeAlso "http://datex2.eu/schema/2/2_0#RugbyMatch" .



###  http://purl.org/td/transportdisruption#RushHourLaneInOperation

:RushHourLaneInOperation rdf:type owl:Class ;
                         
                         rdfs:label "Rush Hour Lane In Operation"^^xsd:string ;
                         
                         rdfs:subClassOf :RoadOrCarriagewayOrLaneManagement ;
                         
                         rdfs:comment "Dedicated rush (peak) hour lane(s) are in operation. This concept and description are from the DATEX II concept rushHourLaneInOperation."^^xsd:string ;
                         
                         rdfs:seeAlso "http://datex2.eu/schema/2/2_0#RushHourLaneInOperation" .



###  http://purl.org/td/transportdisruption#Sabotage

:Sabotage rdf:type owl:Class ;
          
          rdfs:label "Sabotage"^^xsd:string ;
          
          rdfs:subClassOf :DisturbanceActivity ;
          
          rdfs:comment "A situation resulting from any act of sabotage. This concept and description are from the DATEX II concept sabotage."^^xsd:string ;
          
          rdfs:seeAlso "http://datex2.eu/schema/2/2_0#Sabotage" .



###  http://purl.org/td/transportdisruption#SaltingInProgress

:SaltingInProgress rdf:type owl:Class ;
                   
                   rdfs:label "Salting In Progress"^^xsd:string ;
                   
                   rdfs:subClassOf :InfrastructureMaintenance ;
                   
                   rdfs:comment "Spreading of salt and / or grit on the road surface to prevent or melt snow or ice. This concept and description are from the DATEX II concept saltingInProgress."^^xsd:string ;
                   
                   rdfs:seeAlso "http://datex2.eu/schema/2/2_0#SaltingInProgress" .



###  http://purl.org/td/transportdisruption#SaltingOrGrittingVehicleInUse

:SaltingOrGrittingVehicleInUse rdf:type owl:Class ;
                               
                               rdfs:label "Salting Or Gritting Vehicle In Use"^^xsd:string ;
                               
                               rdfs:subClassOf :VehicleObstruction ;
                               
                               rdfs:comment "Salting and gritting vehicles are in use which may cause traffic disruption. This concept and description are from the DATEX II concept saltingOrGrittingVehicleInUse."^^xsd:string ;
                               
                               rdfs:seeAlso "http://datex2.eu/schema/2/2_0#SaltingOrGrittingVehicleInUse" .



###  http://purl.org/td/transportdisruption#SandStorms

:SandStorms rdf:type owl:Class ;
            
            rdfs:label "Sand Storms"^^xsd:string ;
            
            rdfs:subClassOf :EnvironmentalConditions ;
            
            rdfs:comment "Sand blowing across some transport infrasturcture causing significantly reduced visibility. This concept and description are a generalised version of the DATEX II concept sandStorms."^^xsd:string ;
            
            rdfs:seeAlso "http://datex2.eu/schema/2/2_0#SandStorms" .



###  http://purl.org/td/transportdisruption#SecurityAlert

:SecurityAlert rdf:type owl:Class ;
               
               rdfs:label "Security Alert"^^xsd:string ;
               
               rdfs:subClassOf :DisturbanceActivity ;
               
               rdfs:comment "An official alert to a perceived or actual threat of crime or terrorism, which could disrupt traffic. This concept and description are from the DATEX II concept securityAlert."^^xsd:string ;
               
               rdfs:seeAlso "http://datex2.eu/schema/2/2_0#SecurityAlert" .



###  http://purl.org/td/transportdisruption#SecurityIncident

:SecurityIncident rdf:type owl:Class ;
                  
                  rdfs:label "Security Incident"^^xsd:string ;
                  
                  rdfs:subClassOf :DisturbanceActivity ;
                  
                  rdfs:comment "A situation related to a perceived or actual threat of crime or terrorism, which could disrupt traffic. This concept and description are from the DATEX II concept securityIncident."^^xsd:string ;
                  
                  rdfs:seeAlso "http://datex2.eu/schema/2/2_0#SecurityIncident" .



###  http://purl.org/td/transportdisruption#SeriousAccident

:SeriousAccident rdf:type owl:Class ;
                 
                 rdfs:label "Serious Accident"^^xsd:string ;
                 
                 rdfs:subClassOf :Accident ;
                 
                 rdfs:comment "Includes all accidents believed to involve fatality or injury expected to require overnight hospitalisation. This concept and description are from the DATEX II concept seriousAccident."^^xsd:string ;
                 
                 rdfs:seeAlso "http://datex2.eu/schema/2/2_0#SeriousAccident" .



###  http://purl.org/td/transportdisruption#SeriousFire

:SeriousFire rdf:type owl:Class ;
             
             rdfs:label "Serious Fire"^^xsd:string ;
             
             rdfs:subClassOf :EnvironmentalObstruction ;
             
             rdfs:comment "Traffic may be disrupted due to a fire (other than a vehicle fire) adjacent to some transport infrastructure. This concept and description are a generalised version of the DATEX II concept seriousFire."^^xsd:string ;
             
             rdfs:seeAlso "http://datex2.eu/schema/2/2_0#SeriousFire" .



###  http://purl.org/td/transportdisruption#SeveralMajorEvents

:SeveralMajorEvents rdf:type owl:Class ;
                    
                    rdfs:label "Several Major Events"^^xsd:string ;
                    
                    rdfs:subClassOf :PublicEvent ;
                    
                    rdfs:comment "A series of significant organised events either on or near some transport infrastructure which could disrupt traffic. This concept and description are a generalised version of the DATEX II concept severalMajorEvents."^^xsd:string ;
                    
                    rdfs:seeAlso "http://datex2.eu/schema/2/2_0#SeveralMajorEvents" .



###  http://purl.org/td/transportdisruption#SevereExhaustPollution

:SevereExhaustPollution rdf:type owl:Class ;
                        
                        rdfs:label "Severe Exhaust Pollution"^^xsd:string ;
                        
                        rdfs:subClassOf :EnvironmentalConditions ;
                        
                        rdfs:comment "Pollution from exhaust fumes has reached a level sufficient to cause concern. This concept and description are from the DATEX II concept severeExhaustPollution."^^xsd:string ;
                        
                        rdfs:seeAlso "http://datex2.eu/schema/2/2_0#SevereExhaustPollution" .



###  http://purl.org/td/transportdisruption#SevereSmog

:SevereSmog rdf:type owl:Class ;
            
            rdfs:label "Severe Smog"^^xsd:string ;
            
            rdfs:subClassOf :EnvironmentalConditions ;
            
            rdfs:comment "Very poor air quality resulting from smog. This concept and description are adaptations of the DATEX II concept severeSmog."^^xsd:string ;
            
            rdfs:seeAlso "http://datex2.eu/schema/2/2_0#SevereSmog" .



###  http://purl.org/td/transportdisruption#SewerOverflow

:SewerOverflow rdf:type owl:Class ;
               
               rdfs:label "Sewer Overflow"^^xsd:string ;
               
               rdfs:subClassOf :EnvironmentalObstruction ;
               
               rdfs:comment "Transport infrastructure is obstructed or partially obstructed by overflows from one or more sewers. This concept and description are a generalised version of the DATEX II concept sewerOverflow."^^xsd:string ;
               
               rdfs:seeAlso "http://datex2.eu/schema/2/2_0#SewerOverflow" .



###  http://purl.org/td/transportdisruption#Show

:Show rdf:type owl:Class ;
      
      rdfs:label "Show"^^xsd:string ;
      
      rdfs:subClassOf :PublicEvent ;
      
      rdfs:comment "Entertainment event that could disrupt traffic. This concept and description are from the DATEX II concept show."^^xsd:string ;
      
      rdfs:seeAlso "http://datex2.eu/schema/2/2_0#Show" .



###  http://purl.org/td/transportdisruption#ShowJumping

:ShowJumping rdf:type owl:Class ;
             
             rdfs:label "Show Jumping"^^xsd:string ;
             
             rdfs:subClassOf :PublicEvent ;
             
             rdfs:comment "Horse showing jumping and tournament event that could disrupt traffic. This concept and description are from the DATEX II concept showJumping."^^xsd:string ;
             
             rdfs:seeAlso "http://datex2.eu/schema/2/2_0#ShowJumping" .



###  http://purl.org/td/transportdisruption#Showers

:Showers rdf:type owl:Class ;
         
         rdfs:label "Showers"^^xsd:string ;
         
         rdfs:subClassOf :EnvironmentalConditions ;
         
         rdfs:comment "Light rain or intermittent rain. This concept and description are from the DATEX II concept showers."^^xsd:string ;
         
         rdfs:seeAlso "http://datex2.eu/schema/2/2_0#Showers" .



###  http://purl.org/td/transportdisruption#SideCollision

:SideCollision rdf:type owl:Class ;
               
               rdfs:label "Side Collision"^^xsd:string ;
               
               rdfs:subClassOf :Collision ;
               
               rdfs:comment "Includes all accidents where one or more vehicles have collided with the side of one or more other vehicles. This concept and description are from the DATEX II concept sideCollision."^^xsd:string ;
               
               rdfs:seeAlso "http://datex2.eu/schema/2/2_0#SideCollision" .



###  http://purl.org/td/transportdisruption#SightseersObstructingAccess

:SightseersObstructingAccess rdf:type owl:Class ;
                             
                             rdfs:label "Sightseers Obstructing Access"^^xsd:string ;
                             
                             rdfs:subClassOf :DisturbanceActivity ;
                             
                             rdfs:comment "Attendees or sightseers to reported event(s) causing obstruction to access. This concept and description are from the DATEX II concept sightseersObstructingAccess."^^xsd:string ;
                             
                             rdfs:seeAlso "http://datex2.eu/schema/2/2_0#SightseersObstructingAccess" .



###  http://purl.org/td/transportdisruption#SingleAlternateLineTraffic

:SingleAlternateLineTraffic rdf:type owl:Class ;
                            
                            rdfs:label "Single Alternate Line Traffic"^^xsd:string ;
                            
                            rdfs:subClassOf :RoadOrCarriagewayOrLaneManagement ;
                            
                            rdfs:comment "Traffic is being controlled to move in alternate single lines. This control may be undertaken by traffic lights or flagman. This concept and description are from the DATEX II concept singleAlternateLineTraffic."^^xsd:string ;
                            
                            rdfs:seeAlso "http://datex2.eu/schema/2/2_0#SingleAlternateLineTraffic" .



###  http://purl.org/td/transportdisruption#Sleet

:Sleet rdf:type owl:Class ;
       
       rdfs:label "Sleet"^^xsd:string ;
       
       rdfs:subClassOf :EnvironmentalConditions ;
       
       rdfs:comment "Rain mingled with snow or hail. This concept and description are from the DATEX II concept sleet."^^xsd:string ;
       
       rdfs:seeAlso "http://datex2.eu/schema/2/2_0#Sleet" .



###  http://purl.org/td/transportdisruption#SlipperyRoad

:SlipperyRoad rdf:type owl:Class ;
              
              rdfs:label "Slippery Road"^^xsd:string ;
              
              rdfs:subClassOf :AdverseInfrastructureConditions ,
                              :WeatherRelatedConditions ;
              
              rdfs:comment "The road surface is slippery due to an unspecified non-weather related cause. This concept and description are from the DATEX II concept slipperyRoad."^^xsd:string ;
              
              rdfs:seeAlso "http://datex2.eu/schema/2/2_0#SlipperyRoad" .



###  http://purl.org/td/transportdisruption#SlowMovingMaintenanceVehicle

:SlowMovingMaintenanceVehicle rdf:type owl:Class ;
                              
                              rdfs:label "Slow Moving Maintenance Vehicle"^^xsd:string ;
                              
                              rdfs:subClassOf :VehicleObstruction ;
                              
                              rdfs:comment "Slow moving vehicles undertaking maintenance work may pose a hazard to other vehicles. This concept and description are a generalised version of the DATEX II concept slowMovingMaintenanceVehicle."^^xsd:string ;
                              
                              rdfs:seeAlso "http://datex2.eu/schema/2/2_0#SlowMovingMaintenanceVehicle" .



###  http://purl.org/td/transportdisruption#SlowTraffic

:SlowTraffic rdf:type owl:Class ;
             
             rdfs:label "Slow Traffic"^^xsd:string ;
             
             rdfs:subClassOf :AbnormalTraffic ;
             
             rdfs:comment "Traffic is slow moving at the specified location, but not yet forming queues.  For road traffic, DATEX II defines this as  average speed is between 25% and 75% of its free-flow level. This concept and description are adaptations of the DATEX II concept slowTraffic."^^xsd:string ;
             
             rdfs:seeAlso "http://datex2.eu/schema/2/2_0#SlowTraffic" .



###  http://purl.org/td/transportdisruption#SlowVehicle

:SlowVehicle rdf:type owl:Class ;
             
             rdfs:label "Slow Vehicle"^^xsd:string ;
             
             rdfs:subClassOf :VehicleObstruction ;
             
             rdfs:comment "A vehicle travelling at well below normal speeds which may cause traffic disruption. This concept and description are a generalised version of the DATEX II concept slowVehicle."^^xsd:string ;
             
             rdfs:seeAlso "http://datex2.eu/schema/2/2_0#SlowVehicle" .



###  http://purl.org/td/transportdisruption#SlushOnRoad

:SlushOnRoad rdf:type owl:Class ;
             
             rdfs:label "Slush On Road"^^xsd:string ;
             
             rdfs:subClassOf :WeatherRelatedConditions ;
             
             rdfs:comment "Melting snow (slush) on road. This concept and description are adaptations of the DATEX II concept slushOnRoad."^^xsd:string ;
             
             rdfs:seeAlso "http://datex2.eu/schema/2/2_0#SlushOnRoad" .



###  http://purl.org/td/transportdisruption#SlushStrings

:SlushStrings rdf:type owl:Class ;
              
              rdfs:label "Slush Strings"^^xsd:string ;
              
              rdfs:subClassOf :WeatherRelatedConditions ;
              
              rdfs:comment "Melting snow (slush) on the roadway is formed into wheel tracks. This concept and description are from the DATEX II concept slushStrings."^^xsd:string ;
              
              rdfs:seeAlso "http://datex2.eu/schema/2/2_0#SlushStrings" .



###  http://purl.org/td/transportdisruption#SmogAlert

:SmogAlert rdf:type owl:Class ;
           
           rdfs:label "Smog Alert"^^xsd:string ;
           
           rdfs:subClassOf :EnvironmentalConditions ;
           
           rdfs:comment "Environmental warning of poor air quality resulting from smog. This concept and description are from the DATEX II concept smogAlert."^^xsd:string ;
           
           rdfs:seeAlso "http://datex2.eu/schema/2/2_0#SmogAlert" .



###  http://purl.org/td/transportdisruption#SmokeHazard

:SmokeHazard rdf:type owl:Class ;
             
             rdfs:label "Smoke Hazard"^^xsd:string ;
             
             rdfs:subClassOf :EnvironmentalConditions ;
             
             rdfs:comment "Smoke drifting across transport infrastructure causing significantly reduced visibility. This concept and description are adaptations of the DATEX II concept smokeHazard."^^xsd:string ;
             
             rdfs:seeAlso "http://datex2.eu/schema/2/2_0#SmokeHazard" .



###  http://purl.org/td/transportdisruption#SmokeOrFumes

:SmokeOrFumes rdf:type owl:Class ;
              
              rdfs:label "Smoke Or Fumes"^^xsd:string ;
              
              rdfs:subClassOf :EnvironmentalObstruction ;
              
              rdfs:comment "Smoke or fumes which may hinder driving conditions or distract drivers. This concept and description are from the DATEX II concept smokeOrFumes."^^xsd:string ;
              
              rdfs:seeAlso "http://datex2.eu/schema/2/2_0#SmokeOrFumes" .



###  http://purl.org/td/transportdisruption#SnowChangingToRain

:SnowChangingToRain rdf:type owl:Class ;
                    
                    rdfs:label "Snow Changing To Rain"^^xsd:string ;
                    
                    rdfs:subClassOf :EnvironmentalConditions ;
                    
                    rdfs:comment "Falling snow is changing to rain. This concept and description are from the DATEX II concept snowChangingToRain."^^xsd:string ;
                    
                    rdfs:seeAlso "http://datex2.eu/schema/2/2_0#SnowChangingToRain" .



###  http://purl.org/td/transportdisruption#SnowDrifts

:SnowDrifts rdf:type owl:Class ;
            
            rdfs:label "Snow Drifts"^^xsd:string ;
            
            rdfs:subClassOf :WeatherRelatedConditions ;
            
            rdfs:comment "Snow drifting is in progress or patches of deep snow are present due to earlier drifting. This concept and description are from the DATEX II concept snowDrifts."^^xsd:string ;
            
            rdfs:seeAlso "http://datex2.eu/schema/2/2_0#SnowDrifts" .



###  http://purl.org/td/transportdisruption#SnowOnPavement

:SnowOnPavement rdf:type owl:Class ;
                
                rdfs:label "Snow On Pavement"^^xsd:string ;
                
                rdfs:subClassOf :WeatherRelatedConditions ;
                
                rdfs:comment "Snow is on the pedestrian pavement. This concept and description are from the DATEX II concept snowOnPavement."^^xsd:string ;
                
                rdfs:seeAlso "http://datex2.eu/schema/2/2_0#SnowOnPavement" .



###  http://purl.org/td/transportdisruption#SnowOnTheInfrastructure

:SnowOnTheInfrastructure rdf:type owl:Class ;
                         
                         rdfs:label "Snow On The Infrastructure"^^xsd:string ;
                         
                         rdfs:subClassOf :WeatherRelatedConditions ;
                         
                         rdfs:comment "Snow is lying on the inftrastructure surface. This concept and description are a generalised version of the DATEX II concept snowOnTheRoad."^^xsd:string ;
                         
                         rdfs:seeAlso "http://datex2.eu/schema/2/2_0#SnowOnTheRoad" .



###  http://purl.org/td/transportdisruption#Snowfall

:Snowfall rdf:type owl:Class ;
          
          rdfs:label "Snowfall"^^xsd:string ;
          
          rdfs:subClassOf :EnvironmentalConditions ;
          
          rdfs:comment "Falling snow, visibility more than 50m. This concept and description are from the DATEX II concept snowfall."^^xsd:string ;
          
          rdfs:seeAlso "http://datex2.eu/schema/2/2_0#Snowfall" .



###  http://purl.org/td/transportdisruption#Snowplough

:Snowplough rdf:type owl:Class ;
            
            rdfs:label "Snowplough"^^xsd:string ;
            
            rdfs:subClassOf :VehicleObstruction ;
            
            rdfs:comment "Snowploughs are in use which may cause traffic disruption. This concept and description are from the DATEX II concept snowplough."^^xsd:string ;
            
            rdfs:seeAlso "http://datex2.eu/schema/2/2_0#Snowplough" .



###  http://purl.org/td/transportdisruption#SnowploughsInUse

:SnowploughsInUse rdf:type owl:Class ;
                  
                  rdfs:label "Snowploughs In Use"^^xsd:string ;
                  
                  rdfs:subClassOf :InfrastructureMaintenance ;
                  
                  rdfs:comment "Snowploughs or other similar mechanical devices in use to clear snow from the road. This concept and description are from the DATEX II concept snowploughsInUse."^^xsd:string ;
                  
                  rdfs:seeAlso "http://datex2.eu/schema/2/2_0#SnowploughsInUse" .



###  http://purl.org/td/transportdisruption#SpeedControlSignFailure

:SpeedControlSignFailure rdf:type owl:Class ;
                         
                         rdfs:label "Speed Control Signs Failure"^^xsd:string ;
                         
                         rdfs:subClassOf :InfrastructureFailure ;
                         
                         rdfs:comment "Failure of signs used to control traffic speed. This concept and description are based on the DATEX II concept speedControlSigns."^^xsd:string ;
                         
                         rdfs:seeAlso "http://datex2.eu/schema/2/2_0#SpeedControlSigns" .



###  http://purl.org/td/transportdisruption#SpeedControlSignFault

:SpeedControlSignFault rdf:type owl:Class ;
                       
                       rdfs:label "Speed Control Sign Fault"^^xsd:string ;
                       
                       rdfs:subClassOf :InfrastructureFault ;
                       
                       rdfs:comment "Faulty or malfunctioning signs used to control traffic speed. This concept and description are based on the DATEX II concept speedControlSigns."^^xsd:string ;
                       
                       rdfs:seeAlso "http://datex2.eu/schema/2/2_0#SpeedControlSigns" .



###  http://purl.org/td/transportdisruption#SpeedManagement

:SpeedManagement rdf:type owl:Class ;
                 
                 rdfs:label "Speed Management"^^xsd:string ;
                 
                 rdfs:subClassOf :NetworkManagement ;
                 
                 rdfs:comment "Speed management action that is instigated by the network/road operator. This concept and description are from the DATEX II concept SpeedManagement."^^xsd:string ;
                 
                 rdfs:seeAlso "http://datex2.eu/schema/2/2_0#SpeedManagement" .



###  http://purl.org/td/transportdisruption#SpeedRestriction

:SpeedRestriction rdf:type owl:Class ;
                  
                  rdfs:label "Speed Restriction"^^xsd:string ;
                  
                  rdfs:subClassOf :SpeedManagement ;
                  
                  rdfs:comment "A speed restriction is in operation. This concept and description are from the DATEX II concept speedRestrictionInOperation."^^xsd:string ;
                  
                  rdfs:seeAlso "http://datex2.eu/schema/2/2_0#SpeedRestrictionInOperation" .



###  http://purl.org/td/transportdisruption#SpillageAccident

:SpillageAccident rdf:type owl:Class ;
                  
                  rdfs:label "Spillage Accident"^^xsd:string ;
                  
                  rdfs:subClassOf :Accident ;
                  
                  rdfs:comment "Includes all situations resulting in a spillage of some substance on transport infrastructure."^^xsd:string .



###  http://purl.org/td/transportdisruption#SportsMeeting

:SportsMeeting rdf:type owl:Class ;
               
               rdfs:label "Sports Meeting"^^xsd:string ;
               
               rdfs:subClassOf :PublicEvent ;
               
               rdfs:comment "Sports event of unspecified type that could disrupt traffic. This concept and description are from the DATEX II concept sportsMeeting."^^xsd:string ;
               
               rdfs:seeAlso "http://datex2.eu/schema/2/2_0#SportsMeeting" .



###  http://purl.org/td/transportdisruption#SprayHazard

:SprayHazard rdf:type owl:Class ;
             
             rdfs:label "Spray Hazard"^^xsd:string ;
             
             rdfs:subClassOf :EnvironmentalConditions ;
             
             rdfs:comment "Reduced visibility resulting from spray created by moving vehicles on a wet roadway. This concept and description are from the DATEX II concept sprayHazard."^^xsd:string ;
             
             rdfs:seeAlso "http://datex2.eu/schema/2/2_0#SprayHazard" .



###  http://purl.org/td/transportdisruption#StateOccasion

:StateOccasion rdf:type owl:Class ;
               
               rdfs:label "State Occasion"^^xsd:string ;
               
               rdfs:subClassOf :PublicEvent ;
               
               rdfs:comment "Public ceremony or visit of national or international significance which could disrupt traffic. This concept and description are from the DATEX II concept stateOccasion."^^xsd:string ;
               
               rdfs:seeAlso "http://datex2.eu/schema/2/2_0#StateOccasion" .



###  http://purl.org/td/transportdisruption#StationaryTraffic

:StationaryTraffic rdf:type owl:Class ;
                   
                   rdfs:label "Stationary Traffic"^^xsd:string ;
                   
                   rdfs:subClassOf :AbnormalTraffic ;
                   
                   rdfs:comment "Traffic is stationary, or very near stationary, at the specified locatio.  For road traffic, DATEX II defines this as average speed is less than 10% of its free-flow level. This concept and description are adaptations of the DATEX II concept stationaryTraffic."^^xsd:string ;
                   
                   rdfs:seeAlso "http://datex2.eu/schema/2/2_0#StationaryTraffic" .



###  http://purl.org/td/transportdisruption#StormDamage

:StormDamage rdf:type owl:Class ;
             
             rdfs:label "Storm Damage"^^xsd:string ;
             
             rdfs:subClassOf :EnvironmentalObstruction ;
             
             rdfs:comment "Transport infrastructure obstructed or partially obstructed by debris caused by strong winds. This concept and description are a generalised version of the DATEX II concept stormDamage."^^xsd:string ;
             
             rdfs:seeAlso "http://datex2.eu/schema/2/2_0#StormDamage" .



###  http://purl.org/td/transportdisruption#StormForceWinds

:StormForceWinds rdf:type owl:Class ;
                 
                 rdfs:label "Storm Force Winds"^^xsd:string ;
                 
                 rdfs:subClassOf :EnvironmentalConditions ;
                 
                 rdfs:comment "Winds between 90 km/h and 120 km/h. This concept and description are from the DATEX II concept stormForceWinds."^^xsd:string ;
                 
                 rdfs:seeAlso "http://datex2.eu/schema/2/2_0#StormForceWinds" .



###  http://purl.org/td/transportdisruption#StreetLightingFailure

:StreetLightingFailure rdf:type owl:Class ;
                       
                       rdfs:label "Street Lighting Failure"^^xsd:string ;
                       
                       rdfs:subClassOf :InfrastructureFailure ;
                       
                       rdfs:comment "Failure of street or road lighting. This concept and description are based on the DATEX II concept streetLighting."^^xsd:string ;
                       
                       rdfs:seeAlso "http://datex2.eu/schema/2/2_0#StreetLighting" .



###  http://purl.org/td/transportdisruption#StreetLightingFault

:StreetLightingFault rdf:type owl:Class ;
                     
                     rdfs:label "Street Lighting Fault"^^xsd:string ;
                     
                     rdfs:subClassOf :InfrastructureFault ;
                     
                     rdfs:comment "Faulty or malfunctioning street or road lighting. This concept and description are based on the DATEX II concept streetLighting."^^xsd:string ;
                     
                     rdfs:seeAlso "http://datex2.eu/schema/2/2_0#StreetLighting" .



###  http://purl.org/td/transportdisruption#Strike

:Strike rdf:type owl:Class ;
        
        rdfs:label "Strike"^^xsd:string ;
        
        rdfs:subClassOf :DisturbanceActivity ;
        
        rdfs:comment "A situation resulting from industrial action that could disrupt traffic. This concept and description are from the DATEX II concept strike."^^xsd:string ;
        
        rdfs:seeAlso "http://datex2.eu/schema/2/2_0#Strike" .



###  http://purl.org/td/transportdisruption#StrongGustsOfWind

:StrongGustsOfWind rdf:type owl:Class ;
                   
                   rdfs:label "Strong Gusts Of Wind"^^xsd:string ;
                   
                   rdfs:subClassOf :EnvironmentalConditions ;
                   
                   rdfs:comment "Constantly varying winds, strong at times. This concept and description are from the DATEX II concept strongGustsOfWind."^^xsd:string ;
                   
                   rdfs:seeAlso "http://datex2.eu/schema/2/2_0#StrongGustsOfWind" .



###  http://purl.org/td/transportdisruption#StrongWinds

:StrongWinds rdf:type owl:Class ;
             
             rdfs:label "Strong Winds"^^xsd:string ;
             
             rdfs:subClassOf :EnvironmentalConditions ;
             
             rdfs:comment "Winds between 40 km/h and 60 km/h. This concept and description are from the DATEX II concept strongWinds."^^xsd:string ;
             
             rdfs:seeAlso "http://datex2.eu/schema/2/2_0#StrongWinds" .



###  http://purl.org/td/transportdisruption#Subsidence

:Subsidence rdf:type owl:Class ;
            
            rdfs:label "Subsidence"^^xsd:string ;
            
            rdfs:subClassOf :EnvironmentalObstruction ;
            
            rdfs:comment "The surface of some ransport infrastructure has sunken or collapsed in places. This concept and description are a generalised version of the DATEX II concept subsidence."^^xsd:string ;
            
            rdfs:seeAlso "http://datex2.eu/schema/2/2_0#Subsidence" .



###  http://purl.org/td/transportdisruption#SurfaceWater

:SurfaceWater rdf:type owl:Class ;
              
              rdfs:label "Surface Water"^^xsd:string ;
              
              rdfs:subClassOf :WeatherRelatedConditions ;
              
              rdfs:comment "Water is resting on the roadway which provides an increased hazard to vehicles. This concept and description are from the DATEX II concept surfaceWater."^^xsd:string ;
              
              rdfs:seeAlso "http://datex2.eu/schema/2/2_0#SurfaceWater" .



###  http://purl.org/td/transportdisruption#Survey

:Survey rdf:type owl:Class ;
        
        rdfs:label "Survey"^^xsd:string ;
        
        rdfs:subClassOf :AuthorityOperation ;
        
        rdfs:comment "A permanent or temporary operation established by authorities on or adjacent to the transport infrastructure for the purpose of gathering statistics or other traffic related information. This concept and description are a generalised version of the DATEX II concept survey."^^xsd:string ;
        
        rdfs:seeAlso "http://datex2.eu/schema/2/2_0#Survey" .



###  http://purl.org/td/transportdisruption#SwarmsOfInsects

:SwarmsOfInsects rdf:type owl:Class ;
                 
                 rdfs:label "Swarms Of Insects"^^xsd:string ;
                 
                 rdfs:subClassOf :EnvironmentalConditions ;
                 
                 rdfs:comment "Large numbers of insects which create a hazard through reduced visibility. This concept and description are adaptations of the DATEX II concept swarmsOfInsects."^^xsd:string ;
                 
                 rdfs:seeAlso "http://datex2.eu/schema/2/2_0#SwarmsOfInsects" .



###  http://purl.org/td/transportdisruption#SweepingOfRoad

:SweepingOfRoad rdf:type owl:Class ;
                
                rdfs:label "Sweeping Of Road"^^xsd:string ;
                
                rdfs:subClassOf :InfrastructureMaintenance ;
                
                rdfs:comment "Sweeping of the roadway. This concept and description are from the DATEX II concept sweepingOfRoad."^^xsd:string ;
                
                rdfs:seeAlso "http://datex2.eu/schema/2/2_0#SweepingOfRoad" .



###  http://purl.org/td/transportdisruption#TemperatureFalling

:TemperatureFalling rdf:type owl:Class ;
                    
                    rdfs:label "Temperature Falling"^^xsd:string ;
                    
                    rdfs:subClassOf :EnvironmentalConditions ;
                    
                    rdfs:comment "The temperature is falling significantly. This concept and description are from the DATEX II concept temperatureFalling."^^xsd:string ;
                    
                    rdfs:seeAlso "http://datex2.eu/schema/2/2_0#TemperatureFalling" .



###  http://purl.org/td/transportdisruption#TemporaryTrafficLights

:TemporaryTrafficLights rdf:type owl:Class ;
                        
                        rdfs:label "Temporary Traffic Lights"^^xsd:string ;
                        
                        rdfs:subClassOf :GeneralNetworkManagement ;
                        
                        rdfs:comment "Traffic is being controlled by temporary traffic lights (red-yellow-green or red-green). This concept and description are from the DATEX II concept temporaryTrafficLights."^^xsd:string ;
                        
                        rdfs:seeAlso "http://datex2.eu/schema/2/2_0#TemporaryTrafficLights" .



###  http://purl.org/td/transportdisruption#TemporaryTrafficLightsFailure

:TemporaryTrafficLightsFailure rdf:type owl:Class ;
                               
                               rdfs:label "Temporary Traffic Lights Failure"^^xsd:string ;
                               
                               rdfs:subClassOf :InfrastructureFailure ;
                               
                               rdfs:comment "Failure of a set of temporary traffic lights (red-yellow-green or red-green). This concept and description are based on the DATEX II concept temporaryTrafficLights."^^xsd:string ;
                               
                               rdfs:seeAlso "http://datex2.eu/schema/2/2_0#TemporaryTrafficLights" .



###  http://purl.org/td/transportdisruption#TemporaryTrafficLightsFault

:TemporaryTrafficLightsFault rdf:type owl:Class ;
                             
                             rdfs:label "Temporary Traffic Lights Fault"^^xsd:string ;
                             
                             rdfs:subClassOf :InfrastructureFault ;
                             
                             rdfs:comment "Faulty or malfunctioning temporary traffic lights (red-yellow-green or red-green). This concept and description are based on the DATEX II concept temporaryTrafficLights."^^xsd:string ;
                             
                             rdfs:seeAlso "http://datex2.eu/schema/2/2_0#TemporaryTrafficLights" .



###  http://purl.org/td/transportdisruption#TennisTournament

:TennisTournament rdf:type owl:Class ;
                  
                  rdfs:label "Tennis Tournament"^^xsd:string ;
                  
                  rdfs:subClassOf :PublicEvent ;
                  
                  rdfs:comment "Tennis tournament that could disrupt traffic. This concept and description are from the DATEX II concept tennisTournament."^^xsd:string ;
                  
                  rdfs:seeAlso "http://datex2.eu/schema/2/2_0#TennisTournament" .



###  http://purl.org/td/transportdisruption#TerroristIncident

:TerroristIncident rdf:type owl:Class ;
                   
                   rdfs:label "Terrorist Incident"^^xsd:string ;
                   
                   rdfs:subClassOf :DisturbanceActivity ;
                   
                   rdfs:comment "A situation related to a perceived or actual threat of terrorism, which could disrupt traffic. This concept and description are from the DATEX II concept terroristIncident."^^xsd:string ;
                   
                   rdfs:seeAlso "http://datex2.eu/schema/2/2_0#TerroristIncident" .



###  http://purl.org/td/transportdisruption#Theft

:Theft rdf:type owl:Class ;
       
       rdfs:label "Theft"^^xsd:string ;
       
       rdfs:subClassOf :DisturbanceActivity ;
       
       rdfs:comment "A situation where assets of one or more persons or authorities have been stolen. This concept and description are from the DATEX II concept theft."^^xsd:string ;
       
       rdfs:seeAlso "http://datex2.eu/schema/2/2_0#Theft" .



###  http://purl.org/td/transportdisruption#Thunderstorms

:Thunderstorms rdf:type owl:Class ;
               
               rdfs:label "Thunderstorms"^^xsd:string ;
               
               rdfs:subClassOf :EnvironmentalConditions ;
               
               rdfs:comment "Electrical storms, generally with heavy rain. This concept and description are from the DATEX II concept thunderstorms."^^xsd:string ;
               
               rdfs:seeAlso "http://datex2.eu/schema/2/2_0#Thunderstorms" .



###  http://purl.org/td/transportdisruption#TidalFlowLaneInOperation

:TidalFlowLaneInOperation rdf:type owl:Class ;
                          
                          rdfs:label "Tidal Flow Lane In Operation"^^xsd:string ;
                          
                          rdfs:subClassOf :RoadOrCarriagewayOrLaneManagement ;
                          
                          rdfs:comment "Dedicated tidal flow lane(s) are in operation in the specified direction. This concept and description are from the DATEX II concept tidalFlowLaneInOperation."^^xsd:string ;
                          
                          rdfs:seeAlso "http://datex2.eu/schema/2/2_0#TidalFlowLaneInOperation" .



###  http://purl.org/td/transportdisruption#TollGatesFailure

:TollGatesFailure rdf:type owl:Class ;
                  
                  rdfs:label "Toll Gates Failure"^^xsd:string ;
                  
                  rdfs:subClassOf :InfrastructureFailure ;
                  
                  rdfs:comment "Failure of toll gates. This concept and description are based on the DATEX II concept tollGates."^^xsd:string ;
                  
                  rdfs:seeAlso "http://datex2.eu/schema/2/2_0#TollGates" .



###  http://purl.org/td/transportdisruption#TollGatesFault

:TollGatesFault rdf:type owl:Class ;
                
                rdfs:label "Toll Gates Fault"^^xsd:string ;
                
                rdfs:subClassOf :InfrastructureFault ;
                
                rdfs:comment "Faulty or malfunctioning toll gates. This concept and description are based on the DATEX II concept tollGates."^^xsd:string ;
                
                rdfs:seeAlso "http://datex2.eu/schema/2/2_0#TollGates" .



###  http://purl.org/td/transportdisruption#TollGatesOpen

:TollGatesOpen rdf:type owl:Class ;
               
               rdfs:label "Toll Gates Open"^^xsd:string ;
               
               rdfs:subClassOf :GeneralNetworkManagement ;
               
               rdfs:comment "Toll gates are open with no fee collection at the specified location. This concept and description are from the DATEX II concept tollGatesOpen."^^xsd:string ;
               
               rdfs:seeAlso "http://datex2.eu/schema/2/2_0#TollGatesOpen" .



###  http://purl.org/td/transportdisruption#Tornadoes

:Tornadoes rdf:type owl:Class ;
           
           rdfs:label "Tornadoes"^^xsd:string ;
           
           rdfs:subClassOf :EnvironmentalConditions ;
           
           rdfs:comment "Very violent, whirling windstorms affecting narrow strips of country. This concept and description are from the DATEX II concept tornadoes."^^xsd:string ;
           
           rdfs:seeAlso "http://datex2.eu/schema/2/2_0#Tornadoes" .



###  http://purl.org/td/transportdisruption#Tournament

:Tournament rdf:type owl:Class ;
            
            rdfs:label "Tournament"^^xsd:string ;
            
            rdfs:subClassOf :PublicEvent ;
            
            rdfs:comment "Sporting event or series of events of unspecified type lasting more than one day which could disrupt traffic. This concept and description are from the DATEX II concept tournament."^^xsd:string ;
            
            rdfs:seeAlso "http://datex2.eu/schema/2/2_0#Tournament" .



###  http://purl.org/td/transportdisruption#ToxicCloudAlert

:ToxicCloudAlert rdf:type owl:Class ;
                 
                 rdfs:label "Toxic Cloud Alert"^^xsd:string ;
                 
                 rdfs:subClassOf :DisturbanceActivity ;
                 
                 rdfs:comment "An alert to a toxic release of gases and/or particulates into the environment which may endanger the public and hence may cause traffic disruption. This concept and description are from the DATEX II concept toxicCloudAlert."^^xsd:string ;
                 
                 rdfs:seeAlso "http://datex2.eu/schema/2/2_0#ToxicCloudAlert" .



###  http://purl.org/td/transportdisruption#TrackLayingVehicle

:TrackLayingVehicle rdf:type owl:Class ;
                    
                    rdfs:label "Track Laying Vehicle"^^xsd:string ;
                    
                    rdfs:subClassOf :VehicleObstruction ;
                    
                    rdfs:comment "Track laying vehicles are in use which may cause traffic disruption. This concept and description are from the DATEX II concept trackLayingVehicle."^^xsd:string ;
                    
                    rdfs:seeAlso "http://datex2.eu/schema/2/2_0#TrackLayingVehicle" .



###  http://purl.org/td/transportdisruption#TradeFair

:TradeFair rdf:type owl:Class ;
           
           rdfs:label "Trade Fair"^^xsd:string ;
           
           rdfs:subClassOf :PublicEvent ;
           
           rdfs:comment "A periodic (e.g. annual), often traditional, gathering for trade promotion, which could disrupt traffic. This concept and description are from the DATEX II concept tradeFair."^^xsd:string ;
           
           rdfs:seeAlso "http://datex2.eu/schema/2/2_0#TradeFair" .



###  http://purl.org/td/transportdisruption#TrafficBeingManuallyDirected

:TrafficBeingManuallyDirected rdf:type owl:Class ;
                              
                              rdfs:label "Traffic Being Manually Directed"^^xsd:string ;
                              
                              rdfs:subClassOf :GeneralNetworkManagement ;
                              
                              rdfs:comment "Traffic is being manually directed. This concept and description are from the DATEX II concept trafficBeingManuallyDirected."^^xsd:string ;
                              
                              rdfs:seeAlso "http://datex2.eu/schema/2/2_0#TrafficBeingManuallyDirected" .



###  http://purl.org/td/transportdisruption#TrafficElementEvent

:TrafficElementEvent rdf:type owl:Class ;
                     
                     rdfs:label "Traffic Element Event"^^xsd:string ;
                     
                     rdfs:subClassOf <http://purl.org/NET/c4dm/event.owl#Event> ;
                     
                     rdfs:comment "An event which is not planned by the network operator, which is affecting, or has the potential to affect traffic flow. This concept and description are from the DATEX II concept TrafficElement."^^xsd:string ;
                     
                     rdfs:seeAlso "http://datex2.eu/schema/2/2_0#TrafficElement" .



###  http://purl.org/td/transportdisruption#TrafficHeld

:TrafficHeld rdf:type owl:Class ;
             
             rdfs:label "Traffic Held"^^xsd:string ;
             
             rdfs:subClassOf :GeneralNetworkManagement ;
             
             rdfs:comment "Traffic in the specified direction is temporarily held up due to an unplanned event (e.g. for clearance of wreckage following an accident). This concept and description are from the DATEX II concept trafficHeld."^^xsd:string ;
             
             rdfs:seeAlso "http://datex2.eu/schema/2/2_0#TrafficHeld" .



###  http://purl.org/td/transportdisruption#TrafficLightSetFailure

:TrafficLightSetFailure rdf:type owl:Class ;
                        
                        rdfs:label "Traffic Light Set Failure"^^xsd:string ;
                        
                        rdfs:subClassOf :InfrastructureFailure ;
                        
                        rdfs:comment "Failure of a set of traffic lights. This concept and description are based on the DATEX II concept trafficLightSets."^^xsd:string ;
                        
                        rdfs:seeAlso "http://datex2.eu/schema/2/2_0#TrafficLightSets" .



###  http://purl.org/td/transportdisruption#TrafficLightSetFault

:TrafficLightSetFault rdf:type owl:Class ;
                      
                      rdfs:label "Traffic Light Set Fault"^^xsd:string ;
                      
                      rdfs:subClassOf :InfrastructureFault ;
                      
                      rdfs:comment "Faulty or malfunctioning set of traffic lights. This concept and description are based on the DATEX II concept trafficLightSets."^^xsd:string ;
                      
                      rdfs:seeAlso "http://datex2.eu/schema/2/2_0#TrafficLightSets" .



###  http://purl.org/td/transportdisruption#TrafficSignalsFailure

:TrafficSignalsFailure rdf:type owl:Class ;
                       
                       rdfs:label "Traffic Signals Failure"^^xsd:string ;
                       
                       rdfs:subClassOf :InfrastructureFailure ;
                       
                       rdfs:comment "Failure of traffic signals. This concept and description are based on the DATEX II concept trafficSignals."^^xsd:string ;
                       
                       rdfs:seeAlso "http://datex2.eu/schema/2/2_0#TrafficSignals" .



###  http://purl.org/td/transportdisruption#TrafficSignalsFault

:TrafficSignalsFault rdf:type owl:Class ;
                     
                     rdfs:label "Traffic Signals Fault"^^xsd:string ;
                     
                     rdfs:subClassOf :InfrastructureFault ;
                     
                     rdfs:comment "Faulty or malfunctioning traffic signals. This concept and description are based on the DATEX II concept trafficSignals."^^xsd:string ;
                     
                     rdfs:seeAlso "http://datex2.eu/schema/2/2_0#TrafficSignals" .



###  http://purl.org/td/transportdisruption#TransportOfVip

:TransportOfVip rdf:type owl:Class ;
                
                rdfs:label "Transport Of Vip"^^xsd:string ;
                
                rdfs:subClassOf :AuthorityOperation ;
                
                rdfs:comment "An operation to transport one or more VIPs. This concept and description are from the DATEX II concept transportOfVip."^^xsd:string ;
                
                rdfs:seeAlso "http://datex2.eu/schema/2/2_0#TransportOfVip" .



###  http://purl.org/td/transportdisruption#TreeAndVegetationCuttingWork

:TreeAndVegetationCuttingWork rdf:type owl:Class ;
                              
                              rdfs:label "Tree And Vegetation Cutting Work"^^xsd:string ;
                              
                              rdfs:subClassOf :InfrastructureMaintenance ;
                              
                              rdfs:comment "Tree and vegetation cutting work near transport infrastructure. This concept and description are a generalised version the DATEX II concept treeAndVegetationCuttingWork."^^xsd:string ;
                              
                              rdfs:seeAlso "http://datex2.eu/schema/2/2_0#TreeAndVegetationCuttingWork" .



###  http://purl.org/td/transportdisruption#TunnelLightFailure

:TunnelLightFailure rdf:type owl:Class ;
                    
                    rdfs:label "Tunnel Light Failure"^^xsd:string ;
                    
                    rdfs:subClassOf :InfrastructureFailure ;
                    
                    rdfs:comment "Failure of tunnel lights. This concept and description are based on the DATEX II concept tunnelLights."^^xsd:string ;
                    
                    rdfs:seeAlso "http://datex2.eu/schema/2/2_0#TunnelLights" .



###  http://purl.org/td/transportdisruption#TunnelLightFault

:TunnelLightFault rdf:type owl:Class ;
                  
                  rdfs:label "Tunnel Lights Fault"^^xsd:string ;
                  
                  rdfs:subClassOf :InfrastructureFault ;
                  
                  rdfs:comment "Faulty or malfunctioning tunnel lights. This concept and description are based on the DATEX II concept tunnelLights."^^xsd:string ;
                  
                  rdfs:seeAlso "http://datex2.eu/schema/2/2_0#TunnelLights" .



###  http://purl.org/td/transportdisruption#TunnelVentilationFailure

:TunnelVentilationFailure rdf:type owl:Class ;
                          
                          rdfs:label "Tunnel Ventilation Failure"^^xsd:string ;
                          
                          rdfs:subClassOf :InfrastructureFailure ;
                          
                          rdfs:comment "Failure of a tunnel ventilation system. This concept and description are based on the DATEX II concept tunnelVentilation."^^xsd:string ;
                          
                          rdfs:seeAlso "http://datex2.eu/schema/2/2_0#TunnelVentilation" .



###  http://purl.org/td/transportdisruption#TunnelVentilationFault

:TunnelVentilationFault rdf:type owl:Class ;
                        
                        rdfs:label "Tunnel Ventilation Fault"^^xsd:string ;
                        
                        rdfs:subClassOf :InfrastructureFault ;
                        
                        rdfs:comment "Faulty or malfunctioning tunnel ventilation system. This concept and description are based on the DATEX II concept tunnelVentilation."^^xsd:string ;
                        
                        rdfs:seeAlso "http://datex2.eu/schema/2/2_0#TunnelVentilation" .



###  http://purl.org/td/transportdisruption#TurnAroundInOperation

:TurnAroundInOperation rdf:type owl:Class ;
                       
                       rdfs:label "Turn Around In Operation"^^xsd:string ;
                       
                       rdfs:subClassOf :RoadOrCarriagewayOrLaneManagement ;
                       
                       rdfs:comment "Traffic is being directed back down the opposite carriageway, possibly requiring the temporary removal of the central crash barrier. This concept and description are from the DATEX II concept turnAroundInOperation."^^xsd:string ;
                       
                       rdfs:seeAlso "http://datex2.eu/schema/2/2_0#TurnAroundInOperation" .



###  http://purl.org/td/transportdisruption#UndefinedAuthorityActivity

:UndefinedAuthorityActivity rdf:type owl:Class ;
                            
                            rdfs:label "Undefined Authority Activity"^^xsd:string ;
                            
                            rdfs:subClassOf :AuthorityOperation ;
                            
                            rdfs:comment "An authority activity of undefined type. This concept and description are from the DATEX II concept undefinedAuthorityActivity."^^xsd:string ;
                            
                            rdfs:seeAlso "http://datex2.eu/schema/2/2_0#UndefinedAuthorityActivity" .



###  http://purl.org/td/transportdisruption#Unknown

:Unknown rdf:type owl:Class ;
         
         rdfs:label "Unknown"^^xsd:string ;
         
         rdfs:subClassOf :DrivingCondition ;
         
         rdfs:comment "Driving conditions are unknown. This concept and description are from the DATEX II concept unknown."^^xsd:string ;
         
         rdfs:seeAlso "http://datex2.eu/schema/2/2_0#Unknown" .



###  http://purl.org/td/transportdisruption#UnlitVehicleOnTheRoad

:UnlitVehicleOnTheRoad rdf:type owl:Class ;
                       
                       rdfs:label "Unlit Vehicle On The Road"^^xsd:string ;
                       
                       rdfs:subClassOf :VehicleObstruction ;
                       
                       rdfs:comment "Vehicles without lights are in use which may present a hazard to infrastructure users. This concept and description are a generalised version of the DATEX II concept unlitVehicleOnTheRoad."^^xsd:string ;
                       
                       rdfs:seeAlso "http://datex2.eu/schema/2/2_0#UnlitVehicleOnTheRoad" .



###  http://purl.org/td/transportdisruption#UnspecifiedAbnormalTraffic

:UnspecifiedAbnormalTraffic rdf:type owl:Class ;
                            
                            rdfs:label "Unspecified Abnormal Traffic"^^xsd:string ;
                            
                            rdfs:subClassOf :AbnormalTraffic ;
                            
                            rdfs:comment "There are abnormal traffic conditions of an unspecified nature at the specified location. This concept and description are from the DATEX II concept unspecifiedAbnormalTraffic."^^xsd:string ;
                            
                            rdfs:seeAlso "http://datex2.eu/schema/2/2_0#UnspecifiedAbnormalTraffic" .



###  http://purl.org/td/transportdisruption#UnspecifiedAlert

:UnspecifiedAlert rdf:type owl:Class ;
                  
                  rdfs:label "Unspecified Alert"^^xsd:string ;
                  
                  rdfs:subClassOf :DisturbanceActivity ;
                  
                  rdfs:comment "An alert to a perceived or actual threat of an unspecified nature, which could disrupt traffic. This concept and description are from the DATEX II concept unspecifiedAlert."^^xsd:string ;
                  
                  rdfs:seeAlso "http://datex2.eu/schema/2/2_0#UnspecifiedAlert" .



###  http://purl.org/td/transportdisruption#UseOfSpecifiedLanesOrCarriagewaysAllowed

:UseOfSpecifiedLanesOrCarriagewaysAllowed rdf:type owl:Class ;
                                          
                                          rdfs:label "Use Of Specified Lanes Or Carriageways Allowed"^^xsd:string ;
                                          
                                          rdfs:subClassOf :RoadOrCarriagewayOrLaneManagement ;
                                          
                                          rdfs:comment "The specified lane(s) or carriageway(s) may be used. The normal lane(s) or carriageway(s) restrictions are not currently in force. This concept and description are from the DATEX II concept useOfSpecifiedLanesOrCarriagewaysAllowed."^^xsd:string ;
                                          
                                          rdfs:seeAlso "http://datex2.eu/schema/2/2_0#UseOfSpecifiedLanesOrCarriagewaysAllowed" .



###  http://purl.org/td/transportdisruption#VariableMessageSignFailure

:VariableMessageSignFailure rdf:type owl:Class ;
                            
                            rdfs:label "Variable Message Sign Failure"^^xsd:string ;
                            
                            rdfs:subClassOf :InfrastructureFailure ;
                            
                            rdfs:comment "Failure of a variable message sign. This concept and description are based on the DATEX II concept variableMessageSigns."^^xsd:string ;
                            
                            rdfs:seeAlso "http://datex2.eu/schema/2/2_0#VariableMessageSigns" .



###  http://purl.org/td/transportdisruption#VariableMessageSignFault

:VariableMessageSignFault rdf:type owl:Class ;
                          
                          rdfs:label "Variable Message Sign Fault"^^xsd:string ;
                          
                          rdfs:subClassOf :InfrastructureFault ;
                          
                          rdfs:comment "Faulty or malfunctioning variable message sign. This concept and description are based on the DATEX II concept variableMessageSigns."^^xsd:string ;
                          
                          rdfs:seeAlso "http://datex2.eu/schema/2/2_0#VariableMessageSigns" .



###  http://purl.org/td/transportdisruption#VehicleCarryingHazardousMaterials

:VehicleCarryingHazardousMaterials rdf:type owl:Class ;
                                   
                                   rdfs:label "Vehicle Carrying Hazardous Materials"^^xsd:string ;
                                   
                                   rdfs:subClassOf :VehicleObstruction ;
                                   
                                   rdfs:comment "Vehicles carrying materials of a hazardous nature are present and these could expose others to additional hazards. This concept and description are a generalised version of the DATEX II concept vehicleCarryingHazardousMaterials."^^xsd:string ;
                                   
                                   rdfs:seeAlso "http://datex2.eu/schema/2/2_0#VehicleCarryingHazardousMaterials" .



###  http://purl.org/td/transportdisruption#VehicleInDifficulty

:VehicleInDifficulty rdf:type owl:Class ;
                     
                     rdfs:label "Vehicle In Difficulty"^^xsd:string ;
                     
                     rdfs:subClassOf :VehicleObstruction ;
                     
                     rdfs:comment "A vehicle is experiencing difficulties (e.g. manoeuvring or propulsion difficulties) which may cause traffic disruption. This concept and description are from the DATEX II concept vehicleInDifficulty."^^xsd:string ;
                     
                     rdfs:seeAlso "http://datex2.eu/schema/2/2_0#VehicleInDifficulty" .



###  http://purl.org/td/transportdisruption#VehicleInspectionCheckPoint

:VehicleInspectionCheckPoint rdf:type owl:Class ;
                             
                             rdfs:label "Vehicle Inspection Check Point"^^xsd:string ;
                             
                             rdfs:subClassOf :AuthorityOperation ;
                             
                             rdfs:comment "A permanent or temporary operation established on or adjacent to the transport infrastructure for inspection of vehicles by authorities (e.g. vehicle safety checks and tachograph checks). This concept and description are a generalised version of the DATEX II concept vehicleInspectionCheckPoint."^^xsd:string ;
                             
                             rdfs:seeAlso "http://datex2.eu/schema/2/2_0#VehicleInspectionCheckPoint" .



###  http://purl.org/td/transportdisruption#VehicleObstruction

:VehicleObstruction rdf:type owl:Class ;
                    
                    rdfs:label "Vehicle Obstruction"^^xsd:string ;
                    
                    rdfs:subClassOf :Obstruction ;
                    
                    rdfs:comment "An obstruction on some infrastructure caused by one or more vehicles. This concept and description are a generalised version of the DATEX II concept VehicleObstruction."^^xsd:string ;
                    
                    rdfs:seeAlso "http://datex2.eu/schema/2/2_0#VehicleObstruction" .



###  http://purl.org/td/transportdisruption#VehicleOffInfrastructure

:VehicleOffInfrastructure rdf:type owl:Class ;
                          
                          rdfs:label "Vehicle Off Infrastructure"^^xsd:string ;
                          
                          rdfs:subClassOf :Accident ;
                          
                          rdfs:comment "Includes all accidents where one or more vehicles have left the transport infrastructure."^^xsd:string .



###  http://purl.org/td/transportdisruption#VehicleOffRoad

:VehicleOffRoad rdf:type owl:Class ;
                
                rdfs:label "Vehicle Off Road"^^xsd:string ;
                
                rdfs:subClassOf :VehicleOffInfrastructure ;
                
                rdfs:comment "Includes all accidents where one or more vehicles have left the roadway. This concept and description are from the DATEX II concept vehicleOffRoad."^^xsd:string ;
                
                rdfs:seeAlso "http://datex2.eu/schema/2/2_0#VehicleOffRoad" .



###  http://purl.org/td/transportdisruption#VehicleOnFire

:VehicleOnFire rdf:type owl:Class ;
               
               rdfs:label "Vehicle On Fire"^^xsd:string ;
               
               rdfs:subClassOf :VehicleObstruction ;
               
               rdfs:comment "A vehicle is or has been on fire and may cause traffic disruption. This concept and description are from the DATEX II concept vehicleOnFire."^^xsd:string ;
               
               rdfs:seeAlso "http://datex2.eu/schema/2/2_0#VehicleOnFire" .



###  http://purl.org/td/transportdisruption#VehicleOnWrongCarriageway

:VehicleOnWrongCarriageway rdf:type owl:Class ;
                           
                           rdfs:label "Vehicle On Wrong Carriageway"^^xsd:string ;
                           
                           rdfs:subClassOf :VehicleObstruction ;
                           
                           rdfs:comment "A vehicle is travelling the wrong way along a divided highway (i.e. on the wrong side). This concept and description are from the DATEX II concept vehicleOnWrongCarriageway."^^xsd:string ;
                           
                           rdfs:seeAlso "http://datex2.eu/schema/2/2_0#VehicleOnWrongCarriageway" .



###  http://purl.org/td/transportdisruption#VehicleRecovery

:VehicleRecovery rdf:type owl:Class ;
                 
                 rdfs:label "Vehicle Recovery"^^xsd:string ;
                 
                 rdfs:subClassOf :InfrastructureSideAssistance ;
                 
                 rdfs:comment "Vehicle recovery. This concept and description are from the DATEX II concept vehicleRecovery."^^xsd:string ;
                 
                 rdfs:seeAlso "http://datex2.eu/schema/2/2_0#VehicleRecovery" .



###  http://purl.org/td/transportdisruption#VehicleRepair

:VehicleRepair rdf:type owl:Class ;
               
               rdfs:label "Vehicle Repair"^^xsd:string ;
               
               rdfs:subClassOf :InfrastructureSideAssistance ;
               
               rdfs:comment "Vehicle repair assistance. This concept and description are from the DATEX II concept vehicleRepair."^^xsd:string ;
               
               rdfs:seeAlso "http://datex2.eu/schema/2/2_0#VehicleRepair" .



###  http://purl.org/td/transportdisruption#VehicleSpunAround

:VehicleSpunAround rdf:type owl:Class ;
                   
                   rdfs:label "Vehicle Spun Around"^^xsd:string ;
                   
                   rdfs:subClassOf :Accident ;
                   
                   rdfs:comment "Includes all accidents where a vehicle has skidded and has come to rest not facing its intended line of travel. This concept and description are from the DATEX II concept vehicleSpunAround."^^xsd:string ;
                   
                   rdfs:seeAlso "http://datex2.eu/schema/2/2_0#VehicleSpunAround" .



###  http://purl.org/td/transportdisruption#VehicleStorageInOperation

:VehicleStorageInOperation rdf:type owl:Class ;
                           
                           rdfs:label "Vehicle Storage In Operation"^^xsd:string ;
                           
                           rdfs:subClassOf :RoadOrCarriagewayOrLaneManagement ;
                           
                           rdfs:comment "Vehicles are being stored on the roadway and/or at a rest area or service area at the specified location. This concept and description are from the DATEX II concept vehicleStorageInOperation."^^xsd:string ;
                           
                           rdfs:seeAlso "http://datex2.eu/schema/2/2_0#VehicleStorageInOperation" .



###  http://purl.org/td/transportdisruption#VehicleStuck

:VehicleStuck rdf:type owl:Class ;
              
              rdfs:label "Vehicle Stuck"^^xsd:string ;
              
              rdfs:subClassOf :VehicleObstruction ;
              
              rdfs:comment "One or more vehicles are stuck (i.e. unable to move). This concept and description are adaptations of the DATEX II concept vehicleStuck."^^xsd:string ;
              
              rdfs:seeAlso "http://datex2.eu/schema/2/2_0#VehicleStuck" .



###  http://purl.org/td/transportdisruption#VehicleStuckUnderBridge

:VehicleStuckUnderBridge rdf:type owl:Class ;
                         
                         rdfs:label "Vehicle Stuck Under Bridge"^^xsd:string ;
                         
                         rdfs:subClassOf :VehicleStuck ;
                         
                         rdfs:comment "A vehicle is stuck under a bridge. This concept and description are from the DATEX II concept vehicleStuckUnderBridge."^^xsd:string ;
                         
                         rdfs:seeAlso "http://datex2.eu/schema/2/2_0#VehicleStuckUnderBridge" .



###  http://purl.org/td/transportdisruption#VehicleWeighing

:VehicleWeighing rdf:type owl:Class ;
                 
                 rdfs:label "Vehicle Weighing"^^xsd:string ;
                 
                 rdfs:subClassOf :AuthorityOperation ;
                 
                 rdfs:comment "A permanent or temporary operation established on or adjacent to the transport infrastructure for weighing of vehicles by authorities. This concept and description are a generalised version of the DATEX II concept vehicleWeighing."^^xsd:string ;
                 
                 rdfs:seeAlso "http://datex2.eu/schema/2/2_0#VehicleWeighing" .



###  http://purl.org/td/transportdisruption#VehicleWithOverheightLoad

:VehicleWithOverheightLoad rdf:type owl:Class ;
                           
                           rdfs:label "Vehicle With Overheight Load"^^xsd:string ;
                           
                           rdfs:subClassOf :VehicleObstruction ;
                           
                           rdfs:comment "An over-height vehicle which may present a hazard to road users. This concept and description are from the DATEX II concept vehicleWithOverheightLoad."^^xsd:string ;
                           
                           rdfs:seeAlso "http://datex2.eu/schema/2/2_0#VehicleWithOverheightLoad" .



###  http://purl.org/td/transportdisruption#VehicleWithOverwideLoad

:VehicleWithOverwideLoad rdf:type owl:Class ;
                         
                         rdfs:label "Vehicle With Overwide Load"^^xsd:string ;
                         
                         rdfs:subClassOf :VehicleObstruction ;
                         
                         rdfs:comment "A vehicle of width greater than that normally allowed which may cause traffic disruption. This concept and description are from the DATEX II concept vehicleWithOverwideLoad."^^xsd:string ;
                         
                         rdfs:seeAlso "http://datex2.eu/schema/2/2_0#VehicleWithOverwideLoad" .



###  http://purl.org/td/transportdisruption#VeryHazardous

:VeryHazardous rdf:type owl:Class ;
               
               rdfs:label "Very Hazardous"^^xsd:string ;
               
               rdfs:subClassOf :DrivingCondition ;
               
               rdfs:comment "Driving conditions are very hazardous due to environmental conditions. This concept and description are from the DATEX II concept veryHazardous."^^xsd:string ;
               
               rdfs:seeAlso "http://datex2.eu/schema/2/2_0#VeryHazardous" .



###  http://purl.org/td/transportdisruption#VeryStrongGustsOfWind

:VeryStrongGustsOfWind rdf:type owl:Class ;
                       
                       rdfs:label "Very Strong Gusts Of Wind"^^xsd:string ;
                       
                       rdfs:subClassOf :EnvironmentalConditions ;
                       
                       rdfs:comment "Constantly varying winds, very strong at times. This concept and description are from the DATEX II concept veryStrongGustsOfWind."^^xsd:string ;
                       
                       rdfs:seeAlso "http://datex2.eu/schema/2/2_0#VeryStrongGustsOfWind" .



###  http://purl.org/td/transportdisruption#VisibilityReduced

:VisibilityReduced rdf:type owl:Class ;
                   
                   rdfs:label "Visibility Reduced"^^xsd:string ;
                   
                   rdfs:subClassOf :EnvironmentalConditions ;
                   
                   rdfs:comment "Environmental conditions causing reduced visibility. This concept and description are from the DATEX II concept visibilityReduced."^^xsd:string ;
                   
                   rdfs:seeAlso "http://datex2.eu/schema/2/2_0#VisibilityReduced" .



###  http://purl.org/td/transportdisruption#WaterSportsMeeting

:WaterSportsMeeting rdf:type owl:Class ;
                    
                    rdfs:label "Water Sports Meeting"^^xsd:string ;
                    
                    rdfs:subClassOf :PublicEvent ;
                    
                    rdfs:comment "Water sports meeting that could disrupt traffic. This concept and description are from the DATEX II concept waterSportsMeeting."^^xsd:string ;
                    
                    rdfs:seeAlso "http://datex2.eu/schema/2/2_0#WaterSportsMeeting" .



###  http://purl.org/td/transportdisruption#WeakBridge

:WeakBridge rdf:type owl:Class ;
            
            rdfs:label "Weak Bridge"^^xsd:string ;
            
            rdfs:subClassOf :InfrastructureDamageObstruction ;
            
            rdfs:comment "Weak bridge capable of carrying a reduced load, typically with a reduced weight limit restriction imposed. This concept and description are from the DATEX II concept weakBridge."^^xsd:string ;
            
            rdfs:seeAlso "http://datex2.eu/schema/2/2_0#WeakBridge" .



###  http://purl.org/td/transportdisruption#WeatherRelatedConditions

:WeatherRelatedConditions rdf:type owl:Class ;
                          
                          rdfs:label "Weather Related Road Conditions"^^xsd:string ;
                          
                          rdfs:subClassOf :Conditions ;
                          
                          rdfs:comment "Conditions of infrastructure, for example road surfaces, that are related to the weather which may affect the transport conditions, such as ice, snow or water. This concept and description are a generalised version of the DATEX II concept WeatherRelatedRoadConditions."^^xsd:string ;
                          
                          rdfs:seeAlso "http://datex2.eu/schema/2/2_0#WeatherRelatedRoadConditions" .



###  http://purl.org/td/transportdisruption#WeighInMotion

:WeighInMotion rdf:type owl:Class ;
               
               rdfs:label "Weigh In Motion"^^xsd:string ;
               
               rdfs:subClassOf :AuthorityOperation ;
               
               rdfs:comment "A permanent or temporary facility established by authorities on the carriageway for weighing vehicles while in motion. This concept and description are from the DATEX II concept weighInMotion."^^xsd:string ;
               
               rdfs:seeAlso "http://datex2.eu/schema/2/2_0#WeighInMotion" .



###  http://purl.org/td/transportdisruption#WeightRestrictionInOperation

:WeightRestrictionInOperation rdf:type owl:Class ;
                              
                              rdfs:label "Weight Restriction In Operation"^^xsd:string ;
                              
                              rdfs:subClassOf :RoadOrCarriagewayOrLaneManagement ;
                              
                              rdfs:comment "A weight restriction is in operation. This concept and description are from the DATEX II concept weightRestrictionInOperation."^^xsd:string ;
                              
                              rdfs:seeAlso "http://datex2.eu/schema/2/2_0#WeightRestrictionInOperation" .



###  http://purl.org/td/transportdisruption#Wet

:Wet rdf:type owl:Class ;
     
     rdfs:label "Wet"^^xsd:string ;
     
     rdfs:subClassOf :WeatherRelatedConditions ;
     
     rdfs:comment "Road surface is wet. This concept and description are from the DATEX II concept wet."^^xsd:string ;
     
     rdfs:seeAlso "http://datex2.eu/schema/2/2_0#Wet" .



###  http://purl.org/td/transportdisruption#WetAndIcyRoad

:WetAndIcyRoad rdf:type owl:Class ;
               
               rdfs:label "Wet And Icy Road"^^xsd:string ;
               
               rdfs:subClassOf :WeatherRelatedConditions ;
               
               rdfs:comment "Increased skid risk due to partly thawed, wet road with packed snow and ice, or rain falling on packed snow and ice. This concept and description are from the DATEX II concept wetAndIcyRoad."^^xsd:string ;
               
               rdfs:seeAlso "http://datex2.eu/schema/2/2_0#WetAndIcyRoad" .



###  http://purl.org/td/transportdisruption#WetIcyPavement

:WetIcyPavement rdf:type owl:Class ;
                
                rdfs:label "Wet Icy Pavement"^^xsd:string ;
                
                rdfs:subClassOf :WeatherRelatedConditions ;
                
                rdfs:comment "Partly thawed, wet pedestrian pavement with packed snow and ice, or rain falling on packed snow and ice. This concept and description are from the DATEX II concept wetIcyPavement."^^xsd:string ;
                
                rdfs:seeAlso "http://datex2.eu/schema/2/2_0#WetIcyPavement" .



###  http://purl.org/td/transportdisruption#WhiteOut

:WhiteOut rdf:type owl:Class ;
          
          rdfs:label "White Out"^^xsd:string ;
          
          rdfs:subClassOf :EnvironmentalConditions ;
          
          rdfs:comment "Falling snow in blizzard conditions resulting in very reduced visibility. This concept and description are from the DATEX II concept whiteOut."^^xsd:string ;
          
          rdfs:seeAlso "http://datex2.eu/schema/2/2_0#WhiteOut" .



###  http://purl.org/td/transportdisruption#WinterConditions

:WinterConditions rdf:type owl:Class ;
                  
                  rdfs:label "Winter Conditions"^^xsd:string ;
                  
                  rdfs:subClassOf :DrivingCondition ;
                  
                  rdfs:comment "Driving conditions are consistent with those expected in winter. This concept and description are from the DATEX II concept winterConditions."^^xsd:string ;
                  
                  rdfs:seeAlso "http://datex2.eu/schema/2/2_0#WinterConditions" .



###  http://purl.org/td/transportdisruption#WinterSportsMeeting

:WinterSportsMeeting rdf:type owl:Class ;
                     
                     rdfs:label "Winter Sports Meeting"^^xsd:string ;
                     
                     rdfs:subClassOf :PublicEvent ;
                     
                     rdfs:comment "Winter sports meeting or event (e.g. skiing, ski jumping, skating) that could disrupt traffic. This concept and description are from the DATEX II concept winterSportsMeeting."^^xsd:string ;
                     
                     rdfs:seeAlso "http://datex2.eu/schema/2/2_0#WinterSportsMeeting" .



###  http://purl.org/td/transportdisruption#WinterStorm

:WinterStorm rdf:type owl:Class ;
             
             rdfs:label "Winter Storm"^^xsd:string ;
             
             rdfs:subClassOf :EnvironmentalConditions ;
             
             rdfs:comment "Heavy rain, sleet, hail and/or snow in combination with strong winds, limiting visibility to 50m or less. This concept and description are from the DATEX II concept winterStorm."^^xsd:string ;
             
             rdfs:seeAlso "http://datex2.eu/schema/2/2_0#WinterStorm" .





#################################################################
#
#    Annotations
#
#################################################################


dc:coverage rdfs:label "Coverage"@en ;
            
            terms:issued "1999-07-02"^^xsd:date ;
            
            terms:modified "2008-01-14"^^xsd:date ;
            
            skos:note "A second property with the same name as this property has been declared in the dcterms: namespace (http://purl.org/dc/terms/).  See the Introduction to the document \"DCMI Metadata Terms\" (http://dublincore.org/documents/dcmi-terms/) for an explanation."@en ;
            
            rdfs:comment "Spatial topic and spatial applicability may be a named place or a location specified by its geographic coordinates. Temporal topic may be a named period, date, or date range. A jurisdiction may be a named administrative entity or a geographic place to which the resource applies. Recommended best practice is to use a controlled vocabulary such as the Thesaurus of Geographic Names [TGN]. Where appropriate, named places or time periods can be used in preference to numeric identifiers such as sets of coordinates or date ranges."@en ,
                         "The spatial or temporal topic of the resource, the spatial applicability of the resource, or the jurisdiction under which the resource is relevant."@en ;
            
            terms:hasVersion <http://dublincore.org/usage/terms/history/#coverage-006> ;
            
            rdfs:isDefinedBy dc: .



dc: terms:modified "2012-06-14"^^xsd:date ;
    
    terms:title "Dublin Core Metadata Element Set, Version 1.1"@en ;
    
    terms:publisher <http://purl.org/dc/aboutdcmi#DCMI> .



dc:subject rdfs:label "Subject"@en ;
           
           terms:issued "1999-07-02"^^xsd:date ;
           
           terms:modified "2012-06-14"^^xsd:date ;
           
           skos:note "A second property with the same name as this property has been declared in the dcterms: namespace (http://purl.org/dc/terms/).  See the Introduction to the document \"DCMI Metadata Terms\" (http://dublincore.org/documents/dcmi-terms/) for an explanation."@en ;
           
           rdfs:comment "The topic of the resource."@en ,
                        "Typically, the subject will be represented using keywords, key phrases, or classification codes. Recommended best practice is to use a controlled vocabulary."@en ;
           
           terms:hasVersion <http://dublincore.org/usage/terms/history/#subject-007> ;
           
           rdfs:isDefinedBy dc: .



dc:type rdfs:label "Type"@en ;
        
        terms:issued "1999-07-02"^^xsd:date ;
        
        terms:modified "2008-01-14"^^xsd:date ;
        
        skos:note "A second property with the same name as this property has been declared in the dcterms: namespace (http://purl.org/dc/terms/).  See the Introduction to the document \"DCMI Metadata Terms\" (http://dublincore.org/documents/dcmi-terms/) for an explanation."@en ;
        
        rdfs:comment "Recommended best practice is to use a controlled vocabulary such as the DCMI Type Vocabulary [DCMITYPE]. To describe the file format, physical medium, or dimensions of the resource, use the Format element."@en ,
                     "The nature or genre of the resource."@en ;
        
        terms:hasVersion <http://dublincore.org/usage/terms/history/#type-006> ;
        
        rdfs:isDefinedBy dc: .



dc:contributor rdfs:label "Contributor"@en ;
               
               terms:issued "1999-07-02"^^xsd:date ;
               
               terms:modified "2008-01-14"^^xsd:date ;
               
               skos:note "A second property with the same name as this property has been declared in the dcterms: namespace (http://purl.org/dc/terms/).  See the Introduction to the document \"DCMI Metadata Terms\" (http://dublincore.org/documents/dcmi-terms/) for an explanation."@en ;
               
               rdfs:comment "An entity responsible for making contributions to the resource."@en ,
                            "Examples of a Contributor include a person, an organization, or a service. Typically, the name of a Contributor should be used to indicate the entity."@en ;
               
               terms:hasVersion <http://dublincore.org/usage/terms/history/#contributor-006> ;
               
               rdfs:isDefinedBy dc: .



dc:publisher rdfs:label "Publisher"@en ;
             
             terms:issued "1999-07-02"^^xsd:date ;
             
             terms:modified "2008-01-14"^^xsd:date ;
             
             skos:note "A second property with the same name as this property has been declared in the dcterms: namespace (http://purl.org/dc/terms/).  See the Introduction to the document \"DCMI Metadata Terms\" (http://dublincore.org/documents/dcmi-terms/) for an explanation."@en ;
             
             rdfs:comment "An entity responsible for making the resource available."@en ,
                          "Examples of a Publisher include a person, an organization, or a service. Typically, the name of a Publisher should be used to indicate the entity."@en ;
             
             terms:hasVersion <http://dublincore.org/usage/terms/history/#publisher-006> ;
             
             rdfs:isDefinedBy dc: .



dc:identifier rdfs:label "Identifier"@en ;
              
              terms:issued "1999-07-02"^^xsd:date ;
              
              terms:modified "2008-01-14"^^xsd:date ;
              
              skos:note "A second property with the same name as this property has been declared in the dcterms: namespace (http://purl.org/dc/terms/).  See the Introduction to the document \"DCMI Metadata Terms\" (http://dublincore.org/documents/dcmi-terms/) for an explanation."@en ;
              
              rdfs:comment "An unambiguous reference to the resource within a given context."@en ,
                           "Recommended best practice is to identify the resource by means of a string conforming to a formal identification system. "@en ;
              
              terms:hasVersion <http://dublincore.org/usage/terms/history/#identifier-006> ;
              
              rdfs:isDefinedBy dc: .



dc:relation rdfs:label "Relation"@en ;
            
            terms:issued "1999-07-02"^^xsd:date ;
            
            terms:modified "2008-01-14"^^xsd:date ;
            
            rdfs:comment "A related resource."@en ;
            
            skos:note "A second property with the same name as this property has been declared in the dcterms: namespace (http://purl.org/dc/terms/).  See the Introduction to the document \"DCMI Metadata Terms\" (http://dublincore.org/documents/dcmi-terms/) for an explanation."@en ;
            
            rdfs:comment "Recommended best practice is to identify the related resource by means of a string conforming to a formal identification system. "@en ;
            
            terms:hasVersion <http://dublincore.org/usage/terms/history/#relation-006> ;
            
            rdfs:isDefinedBy dc: .



dc:format rdfs:label "Format"@en ;
          
          terms:issued "1999-07-02"^^xsd:date ;
          
          terms:modified "2008-01-14"^^xsd:date ;
          
          skos:note "A second property with the same name as this property has been declared in the dcterms: namespace (http://purl.org/dc/terms/).  See the Introduction to the document \"DCMI Metadata Terms\" (http://dublincore.org/documents/dcmi-terms/) for an explanation."@en ;
          
          rdfs:comment "Examples of dimensions include size and duration. Recommended best practice is to use a controlled vocabulary such as the list of Internet Media Types [MIME]."@en ,
                       "The file format, physical medium, or dimensions of the resource."@en ;
          
          terms:hasVersion <http://dublincore.org/usage/terms/history/#format-007> ;
          
          rdfs:isDefinedBy dc: .



dc:source rdfs:label "Source"@en ;
          
          terms:issued "1999-07-02"^^xsd:date ;
          
          terms:modified "2008-01-14"^^xsd:date ;
          
          rdfs:comment "A related resource from which the described resource is derived."@en ;
          
          skos:note "A second property with the same name as this property has been declared in the dcterms: namespace (http://purl.org/dc/terms/).  See the Introduction to the document \"DCMI Metadata Terms\" (http://dublincore.org/documents/dcmi-terms/) for an explanation."@en ;
          
          rdfs:comment "The described resource may be derived from the related resource in whole or in part. Recommended best practice is to identify the related resource by means of a string conforming to a formal identification system."@en ;
          
          terms:hasVersion <http://dublincore.org/usage/terms/history/#source-006> ;
          
          rdfs:isDefinedBy dc: .



dc:language rdfs:label "Language"@en ;
            
            terms:issued "1999-07-02"^^xsd:date ;
            
            terms:modified "2008-01-14"^^xsd:date ;
            
            rdfs:comment "A language of the resource."@en ;
            
            skos:note "A second property with the same name as this property has been declared in the dcterms: namespace (http://purl.org/dc/terms/).  See the Introduction to the document \"DCMI Metadata Terms\" (http://dublincore.org/documents/dcmi-terms/) for an explanation."@en ;
            
            rdfs:comment "Recommended best practice is to use a controlled vocabulary such as RFC 4646 [RFC4646]."@en ;
            
            terms:hasVersion <http://dublincore.org/usage/terms/history/#language-007> ;
            
            rdfs:isDefinedBy dc: ;
            
            rdfs:seeAlso <http://www.ietf.org/rfc/rfc4646.txt> .




###  Generated by the OWL API (version 3.5.1) http://owlapi.sourceforge.net

